aspec+access: Access arch split
Signed-off-by: Ryan Barry <ryan.barry@unsw.edu.au>

proof/access-control/Access.thy
@@ -5,150 +5,8 @@
  *)
 
 theory Access
-imports Deterministic_AC
+imports ArchAccess
 begin
-
-context begin interpretation Arch . (*FIXME: arch_split*)
-
-section \<open>Policy and policy refinement\<close>
-
-subsection \<open>Policy definition\<close>
-
-text\<open>
-
-The goal is to place limits on what untrusted agents can do while the
-trusted agents are not running. This supports a framing constraint in
-the descriptions (Hoare triples) of syscalls. Roughly the existing
-proofs show the effect of the syscall, and this proof summarises what
-doesn't (or isn't allowed to) change.
-
-The basic intuition is to map all object references to the agent they
-belong to and show that changes to the object reference graph are
-allowed by the policy specified by the user. The policy is a labelled
-graph amongst agents independent of the current state, i.e. a static
-external summary of what should be talking to what and how.
-
-The interesting cases occur between trusted and untrusted components:
-e.g. we assume that it is unsafe for untrusted components (UT)
-to send capabilities to trusted components (T), and so T must ensure
-that all endpoints it shares with UT that it receives on do not have
-the grant bit set.
-
-\<close>
-
-type_synonym 'a agent_map = "obj_ref \<Rightarrow> 'a"
-type_synonym 'a agent_asid_map = "asid \<Rightarrow> 'a"
-type_synonym 'a agent_irq_map = "irq \<Rightarrow> 'a"
-type_synonym 'a agent_domain_map = "domain \<Rightarrow> 'a set"
-
-text\<open>
-
-What one agent can do to another. We allow multiple edges between
-agents in the graph.
-
-Control is special. It implies the ability to do pretty much anything,
-including get access the other rights, create, remove, etc.
-
-DeleteDerived allows you to delete a cap derived from a cap you own
-\<close>
-
-datatype auth = Control | Receive | SyncSend | Notify
-                    | Reset | Grant | Call | Reply | Write | Read
-                    | ASIDPoolMapsASID | DeleteDerived
-
-text\<open>
-
-The interesting case is for endpoints.
-
-Consider an EP between T and UT (across a trust boundary). We want to
-be able to say that all EPs and tcbs that T does not expose to UT do
-not change when it is not running. If UT had a direct Send right to T
-then integrity (see below) could not guarantee this, as it doesn't
-know which EP can be changed by UT. Thus we set things up like this
-(all distinct labels):
-
-T -Receive-> EP <-Send- UT
-
-Now UT can interfere with EP and all of T's tcbs blocked for receive on EP,
-but not endpoints internal to T, or tcbs blocked on other (suitably
-labelled) EPs, etc.
-
-\<close>
-
-type_synonym 'a auth_graph = "('a \<times> auth \<times> 'a) set"
-
-text \<open>
-
-Each global namespace will need a labeling function.
-
-We map each scheduling domain to a single label; concretely, each tcb
-in a scheduling domain has to have the same label. We will want to
-weaken this in the future.
-
-The booleans @{text pasMayActivate} and @{text pasMayEditReadyQueues}
-are used to weaken the integrity property. When @{const True},
-@{text pasMayActivate} causes the integrity property to permit
-activation of newly-scheduled threads. Likewise, @{text pasMayEditReadyQueues}
-has the integrity property permit the removal of threads from ready queues,
-as occurs when scheduling a new domain for instance. By setting each of these
-@{const False} we get a more constrained integrity property that is useful for
-establishing some of the proof obligations for the infoflow proofs, particularly
-those over @{const handle_event} that neither activates new threads nor schedules
-new domains.
-
-The @{text pasDomainAbs} relation describes which labels may run in
-a given scheduler domain. This relation is not relevant to integrity
-but will be used in the information flow theory (with additional
-constraints on its structure).
-\<close>
-
-end
-
-record 'a PAS =
-  pasObjectAbs :: "'a agent_map"
-  pasASIDAbs :: "'a agent_asid_map"
-  pasIRQAbs :: "'a agent_irq_map"
-  pasPolicy :: "'a auth_graph"
-  pasSubject :: "'a"                \<comment> \<open>The active label\<close>
-  pasMayActivate :: "bool"
-  pasMayEditReadyQueues :: "bool"
-  pasMaySendIrqs :: "bool"
-  pasDomainAbs :: "'a agent_domain_map"
-
-text\<open>
-
-Very often we want to say that the agent currently running owns a
-given pointer.
-
-\<close>
-
-abbreviation is_subject :: "'a PAS \<Rightarrow> obj_ref \<Rightarrow> bool"
-where
-  "is_subject aag ptr \<equiv> pasObjectAbs aag ptr = pasSubject aag"
-
-text\<open>
-
-Also we often want to say the current agent can do something to a
-pointer that he doesn't own but has some authority to.
-
-\<close>
-
-abbreviation(input) aag_has_auth_to :: "'a PAS \<Rightarrow> auth \<Rightarrow> obj_ref \<Rightarrow> bool"
-where
-  "aag_has_auth_to aag auth ptr \<equiv> (pasSubject aag, auth, pasObjectAbs aag ptr) \<in> pasPolicy aag"
-
-abbreviation aag_subjects_have_auth_to_label :: "'a set \<Rightarrow> 'a PAS \<Rightarrow> auth \<Rightarrow> 'a \<Rightarrow> bool"
-where
- "aag_subjects_have_auth_to_label subs aag auth label
-    \<equiv> \<exists>s \<in> subs. (s, auth, label) \<in> pasPolicy aag"
-
-abbreviation aag_subjects_have_auth_to :: "'a set \<Rightarrow> 'a PAS \<Rightarrow> auth \<Rightarrow> obj_ref \<Rightarrow> bool"
-where
- "aag_subjects_have_auth_to subs aag auth oref
-    \<equiv> aag_subjects_have_auth_to_label subs aag auth (pasObjectAbs aag oref)"
-
-
-context begin interpretation Arch . (*FIXME: arch_split*)
 
 subsection \<open>Policy wellformedness\<close>
 
@@ -186,83 +44,25 @@ Wellformedness of the agent authority function with respect to a label
 
 \<close>
 
-definition policy_wellformed
-where
+definition policy_wellformed where
   "policy_wellformed aag maySendIrqs irqs agent \<equiv>
      (\<forall>agent'. (agent, Control, agent') \<in> aag \<longrightarrow> agent = agent')
    \<and> (\<forall>a. (agent, a, agent) \<in> aag)
    \<and> (\<forall>s r ep. (s, Grant, ep) \<in> aag \<and> (r, Receive, ep) \<in> aag
-              \<longrightarrow> (s, Control, r) \<in> aag \<and> (r, Control, s) \<in> aag)
+                \<longrightarrow> (s, Control, r) \<in> aag \<and> (r, Control, s) \<in> aag)
    \<and> (maySendIrqs \<longrightarrow> (\<forall>irq ntfn. irq \<in> irqs \<and> (irq, Notify, ntfn) \<in> aag
-                  \<longrightarrow> (agent, Notify, ntfn) \<in> aag))
+                                  \<longrightarrow> (agent, Notify, ntfn) \<in> aag))
    \<and> (\<forall>s ep. (s, Call, ep) \<in> aag \<longrightarrow> (s, SyncSend, ep) \<in> aag)
    \<and> (\<forall>s r ep. (s, Call, ep) \<in> aag \<and> (r, Receive, ep) \<in> aag \<longrightarrow> (r, Reply, s) \<in> aag)
    \<and> (\<forall>s r. (s, Reply, r) \<in> aag \<longrightarrow> (r, DeleteDerived, s) \<in> aag)
    \<and> (\<forall>l1 l2 l3. (l1, DeleteDerived, l2) \<in> aag \<longrightarrow> (l2, DeleteDerived, l3) \<in> aag
-             \<longrightarrow> (l1, DeleteDerived, l3) \<in> aag)
+                  \<longrightarrow> (l1, DeleteDerived, l3) \<in> aag)
    \<and> (\<forall>s r ep. (s, Call, ep) \<in> aag \<and> (r, Receive, ep) \<in> aag \<and> (r, Grant, ep) \<in> aag
-              \<longrightarrow> (s, Control, r) \<in> aag \<and> (r, Control, s) \<in> aag)"
+                \<longrightarrow> (s, Control, r) \<in> aag \<and> (r, Control, s) \<in> aag)"
 
-abbreviation pas_wellformed
-where
+abbreviation pas_wellformed where
   "pas_wellformed aag \<equiv>
-    policy_wellformed (pasPolicy aag) (pasMaySendIrqs aag) (range (pasIRQAbs aag)) (pasSubject aag)"
-
-lemma aag_wellformed_Control:
-  "\<lbrakk>  (x, Control, y) \<in> aag; policy_wellformed aag mirqs irqs x \<rbrakk> \<Longrightarrow> x = y"
-  unfolding policy_wellformed_def by metis
-
-lemma aag_wellformed_refl:
-  "\<lbrakk> policy_wellformed aag mirqs irqs x \<rbrakk> \<Longrightarrow> (x, a, x) \<in> aag"
-  unfolding policy_wellformed_def by blast
-
-lemma aag_wellformed_grant_Control_to_recv:
-  "\<lbrakk> (s, Grant, ep) \<in> aag; (r, Receive, ep) \<in> aag; policy_wellformed aag mirqs irqs l\<rbrakk>
-        \<Longrightarrow> (s, Control, r) \<in> aag"
-  unfolding policy_wellformed_def by blast
-
-lemma aag_wellformed_grant_Control_to_send:
-  "\<lbrakk> (s, Grant, ep) \<in> aag; (r, Receive, ep) \<in> aag; policy_wellformed aag mirqs irqs l\<rbrakk>
-        \<Longrightarrow> (r, Control, s) \<in> aag"
-  unfolding policy_wellformed_def by blast
-
-lemma aag_wellformed_reply:
-  "\<lbrakk> (s, Call, ep) \<in> aag; (r, Receive, ep) \<in> aag; policy_wellformed aag mirqs irqs l\<rbrakk>
-        \<Longrightarrow> (r, Reply, s) \<in> aag"
-  unfolding policy_wellformed_def by blast
-
-lemma aag_wellformed_delete_derived':
-  "\<lbrakk>  (s, Call, ep) \<in> aag; (r, Receive, ep) \<in> aag; policy_wellformed aag mirqs irqs l\<rbrakk>
-        \<Longrightarrow> (s, DeleteDerived, r) \<in> aag"
-  unfolding policy_wellformed_def by blast
-
-lemma aag_wellformed_delete_derived:
-  "\<lbrakk> (s, Reply, r) \<in> aag; policy_wellformed aag mirqs irqs l\<rbrakk>
-        \<Longrightarrow> (r, DeleteDerived, s) \<in> aag"
-  unfolding policy_wellformed_def by blast
-
-lemma aag_wellformed_delete_derived_trans:
-  "\<lbrakk> (l1, DeleteDerived, l2) \<in> aag; (l2, DeleteDerived, l3) \<in> aag;
-     policy_wellformed aag mirqs irqs l\<rbrakk>
-        \<Longrightarrow> (l1, DeleteDerived, l3) \<in> aag"
-  unfolding policy_wellformed_def by blast
-
-lemma aag_wellformed_call_to_syncsend:
-  "\<lbrakk> (s, Call, ep) \<in> aag; policy_wellformed aag mirqs irqs l\<rbrakk>
-        \<Longrightarrow> (s, SyncSend, ep) \<in> aag"
-  unfolding policy_wellformed_def by blast
-
-lemma aag_wellformed_grant_Control_to_send_by_reply:
-  "\<lbrakk> (s, Call, ep) \<in> aag; (r, Receive, ep) \<in> aag; (r, Grant, ep) \<in> aag;
-   policy_wellformed aag mirqs irqs l\<rbrakk>
-        \<Longrightarrow> (r, Control, s) \<in> aag"
-  unfolding policy_wellformed_def by blast
-
-lemma aag_wellformed_grant_Control_to_recv_by_reply:
-  "\<lbrakk> (s, Call, ep) \<in> aag; (r, Receive, ep) \<in> aag; (r, Grant, ep) \<in> aag;
-   policy_wellformed aag mirqs irqs l\<rbrakk>
-        \<Longrightarrow> (s, Control, r) \<in> aag"
-  unfolding policy_wellformed_def by blast
+     policy_wellformed (pasPolicy aag) (pasMaySendIrqs aag) (range (pasIRQAbs aag)) (pasSubject aag)"
 
 
 subsection \<open>auth_graph_map\<close>
@@ -274,31 +74,8 @@ collapse (and not create) distinctions.
 
 \<close>
 
-definition
-  auth_graph_map :: "('a \<Rightarrow> 'b) \<Rightarrow> 'a auth_graph \<Rightarrow> 'b auth_graph"
-where
+definition auth_graph_map :: "('a \<Rightarrow> 'b) \<Rightarrow> 'a auth_graph \<Rightarrow> 'b auth_graph" where
   "auth_graph_map f aag \<equiv> {(f x, auth, f y) | x auth y. (x, auth, y) \<in> aag}"
-
-lemma auth_graph_map_mem:
-  "(x, auth, y) \<in> auth_graph_map f S
-     = (\<exists>x' y'. x = f x' \<and> y = f y' \<and> (x', auth, y') \<in> S)"
-  by (simp add: auth_graph_map_def)
-
-lemmas auth_graph_map_memD = auth_graph_map_mem[THEN iffD1]
-lemma auth_graph_map_memE:
-  assumes hyp:"(x, auth, y) \<in> auth_graph_map f S"
-  obtains x' and y' where "x = f x'" and "y = f y'" and "(x', auth, y') \<in> S"
-  using hyp[THEN auth_graph_map_mem[THEN iffD1]] by fastforce
-
-lemma auth_graph_map_memI:
-  "\<lbrakk> (x', auth, y') \<in> S; x = f x'; y = f y' \<rbrakk>
-      \<Longrightarrow> (x, auth, y) \<in> auth_graph_map f S"
-  by (fastforce simp add: auth_graph_map_mem)
-
-lemma auth_graph_map_mono:
-  "S \<subseteq> S' \<Longrightarrow> auth_graph_map G S \<subseteq> auth_graph_map G S'"
-  unfolding auth_graph_map_def by auto
-
 
 
 subsection \<open>Transform caps and tcb states into authority\<close>
@@ -311,8 +88,7 @@ in it.
 
 \<close>
 
-definition cap_rights_to_auth :: "cap_rights \<Rightarrow> bool \<Rightarrow> auth set"
-where
+definition cap_rights_to_auth :: "cap_rights \<Rightarrow> bool \<Rightarrow> auth set" where
   "cap_rights_to_auth r sync \<equiv>
      {Reset}
    \<union> (if AllowRead \<in> r then {Receive} else {})
@@ -320,94 +96,33 @@ where
    \<union> (if AllowGrant \<in> r then UNIV else {})
    \<union> (if AllowGrantReply \<in> r \<and> AllowWrite \<in> r then {Call} else {})"
 
-definition vspace_cap_rights_to_auth :: "cap_rights \<Rightarrow> auth set"
-where
-  "vspace_cap_rights_to_auth r \<equiv>
-      (if AllowWrite \<in> r then {Write} else {})
-    \<union> (if AllowRead \<in> r then {Read} else {})"
-
-definition reply_cap_rights_to_auth :: "bool \<Rightarrow> cap_rights \<Rightarrow> auth set"
-where
+definition reply_cap_rights_to_auth :: "bool \<Rightarrow> cap_rights \<Rightarrow> auth set" where
   "reply_cap_rights_to_auth master r \<equiv> if AllowGrant \<in> r \<or> master then UNIV else {Reply}"
 
-definition cap_auth_conferred :: "cap \<Rightarrow> auth set"
-where
- "cap_auth_conferred cap \<equiv>
-    case cap of
-      Structures_A.NullCap \<Rightarrow> {}
-    | Structures_A.UntypedCap isdev oref bits freeIndex \<Rightarrow> {Control}
-    | Structures_A.EndpointCap oref badge r \<Rightarrow>
-         cap_rights_to_auth r True
-    | Structures_A.NotificationCap oref badge r \<Rightarrow>
-         cap_rights_to_auth (r - {AllowGrant, AllowGrantReply}) False
-    | Structures_A.ReplyCap oref m r \<Rightarrow> reply_cap_rights_to_auth m r
-    | Structures_A.CNodeCap oref bits guard \<Rightarrow> {Control}
-    | Structures_A.ThreadCap obj_ref \<Rightarrow> {Control}
-    | Structures_A.DomainCap \<Rightarrow> {Control}
-    | Structures_A.IRQControlCap \<Rightarrow> {Control}
-    | Structures_A.IRQHandlerCap irq \<Rightarrow> {Control}
-    | Structures_A.Zombie ptr b n \<Rightarrow> {Control}
-    | Structures_A.ArchObjectCap arch_cap \<Rightarrow>
-         (if is_page_cap (the_arch_cap cap)
-         then vspace_cap_rights_to_auth (acap_rights arch_cap)
-             else {Control})"
+definition cap_auth_conferred :: "cap \<Rightarrow> auth set" where
+ "cap_auth_conferred cap \<equiv> case cap of
+    NullCap \<Rightarrow> {}
+  | UntypedCap isdev oref bits freeIndex \<Rightarrow> {Control}
+  | EndpointCap oref badge r \<Rightarrow> cap_rights_to_auth r True
+  | NotificationCap oref badge r \<Rightarrow> cap_rights_to_auth (r - {AllowGrant, AllowGrantReply}) False
+  | ReplyCap oref m r \<Rightarrow> reply_cap_rights_to_auth m r
+  | CNodeCap oref bits guard \<Rightarrow> {Control}
+  | ThreadCap obj_ref \<Rightarrow> {Control}
+  | DomainCap \<Rightarrow> {Control}
+  | IRQControlCap \<Rightarrow> {Control}
+  | IRQHandlerCap irq \<Rightarrow> {Control}
+  | Zombie ptr b n \<Rightarrow> {Control}
+  | ArchObjectCap arch_cap \<Rightarrow> arch_cap_auth_conferred arch_cap"
 
-fun tcb_st_to_auth :: "Structures_A.thread_state \<Rightarrow> (obj_ref \<times> auth) set"
-where
-  "tcb_st_to_auth (Structures_A.BlockedOnNotification ntfn) = {(ntfn, Receive)}"
-| "tcb_st_to_auth (Structures_A.BlockedOnSend ep payl)
-     = {(ep, SyncSend)} \<union> (if sender_can_grant payl then {(ep, Grant),(ep, Call)} else {})
-       \<union> (if sender_can_grant_reply payl then {(ep, Call)} else {})"
-| "tcb_st_to_auth (Structures_A.BlockedOnReceive ep payl)
-     = {(ep, Receive)} \<union> (if receiver_can_grant payl then {(ep, Grant)} else {})"
+fun tcb_st_to_auth :: "thread_state \<Rightarrow> (obj_ref \<times> auth) set" where
+  "tcb_st_to_auth (BlockedOnNotification ntfn) = {(ntfn, Receive)}"
+| "tcb_st_to_auth (BlockedOnSend ep payl) =
+     {(ep, SyncSend)} \<union> (if sender_can_grant payl then {(ep, Grant),(ep, Call)} else {})
+   \<union> (if sender_can_grant_reply payl then {(ep, Call)} else {})"
+| "tcb_st_to_auth (BlockedOnReceive ep payl) =
+     {(ep, Receive)} \<union> (if receiver_can_grant payl then {(ep, Grant)} else {})"
 | "tcb_st_to_auth _ = {}"
 
-subsection \<open>FIXME MOVE\<close>
-
-definition pte_ref
-where
-  "pte_ref pte \<equiv> case pte of
-    SmallPagePTE addr atts rights
-       \<Rightarrow> Some (ptrFromPAddr addr, pageBitsForSize ARMSmallPage, vspace_cap_rights_to_auth rights)
-  | LargePagePTE addr atts rights
-       \<Rightarrow> Some (ptrFromPAddr addr, pageBitsForSize ARMLargePage, vspace_cap_rights_to_auth rights)
-  | _ \<Rightarrow> None"
-
-definition pde_ref2
-where
-  "pde_ref2 pde \<equiv> case pde of
-    SectionPDE addr atts domain rights
-       \<Rightarrow> Some (ptrFromPAddr addr, pageBitsForSize ARMSection, vspace_cap_rights_to_auth rights)
-  | SuperSectionPDE addr atts rights
-       \<Rightarrow> Some (ptrFromPAddr addr, pageBitsForSize ARMSuperSection, vspace_cap_rights_to_auth rights)
-  | PageTablePDE addr atts domain
-    \<comment> \<open>The 0 is a hack, saying that we own only addr, although 12 would also be OK\<close>
-       \<Rightarrow> Some (ptrFromPAddr addr, 0, {Control})
-  | _ \<Rightarrow> None"
-
-definition ptr_range
-where
-  "ptr_range p sz \<equiv> {p .. p + 2 ^ sz - 1}"
-
-(* We exclude the global page tables from the authority graph. Alternatively,
-   we could include them and add a wellformedness constraint to policies that
-   requires that every label has the necessary authority to whichever label owns
-   the global page tables, so that when a new page directory is created and
-   references to the global page tables are added to it, no new authority is gained.
-   Note: excluding the references to global page tables in this way
-         brings in some ARM arch-specific VM knowledge here *)
-definition vs_refs_no_global_pts :: "Structures_A.kernel_object \<Rightarrow> (obj_ref \<times> vs_ref \<times> auth) set"
-where
-  "vs_refs_no_global_pts \<equiv> \<lambda>ko. case ko of
-    ArchObj (ASIDPool pool) \<Rightarrow>
-       (\<lambda>(r,p). (p, VSRef (ucast r) (Some AASIDPool), Control)) ` graph_of pool
-  | ArchObj (PageDirectory pd) \<Rightarrow>
-      \<Union>(r,(p, sz, auth)) \<in> graph_of (pde_ref2 o pd) - {(x,y). (ucast (kernel_base >> 20) \<le> x)}.
-          (\<lambda>(p, a). (p, VSRef (ucast r) (Some APageDirectory), a)) ` (ptr_range p sz \<times> auth)
-  | ArchObj (PageTable pt) \<Rightarrow>
-      \<Union>(r,(p, sz, auth)) \<in> graph_of (pte_ref o pt).
-          (\<lambda>(p, a). (p, VSRef (ucast r) (Some APageTable), a)) ` (ptr_range p sz \<times> auth)
-  | _ \<Rightarrow> {}"
 
 subsection \<open>Transferability: Moving caps between agents\<close>
 
@@ -415,10 +130,10 @@ text \<open>
   Tells if cap can move/be derived between agents without grant
   due to the inner workings of the system (Calling and replying for now)
 \<close>
-(* FIXME is_transferable should garantee directly that a non-NullCap cap is owned by its CDT
+
+(* FIXME is_transferable should guarantee directly that a non-NullCap cap is owned by its CDT
    parents without using directly the CDT so that we can use it in integrity *)
-inductive is_transferable for opt_cap
-where
+inductive is_transferable for opt_cap where
   it_None: "opt_cap = None \<Longrightarrow> is_transferable opt_cap" |
   it_Null: "opt_cap = Some NullCap \<Longrightarrow> is_transferable opt_cap" |
   it_Reply: "opt_cap = Some (ReplyCap t False R) \<Longrightarrow> is_transferable opt_cap"
@@ -426,103 +141,13 @@ where
 abbreviation "is_transferable_cap cap \<equiv> is_transferable (Some cap)"
 abbreviation "is_transferable_in slot s \<equiv> is_transferable (caps_of_state s slot)"
 
-lemma is_transferable_capE:
-  assumes hyp:"is_transferable_cap cap"
-  obtains "cap = NullCap" | t R where "cap = ReplyCap t False R"
-  by (rule is_transferable.cases[OF hyp]) auto
-
-lemma is_transferable_None[simp]: "is_transferable None"
-  using is_transferable.simps by simp
-lemma is_transferable_Null[simp]: "is_transferable_cap NullCap"
-  using is_transferable.simps by simp
-lemma is_transferable_Reply[simp]: "is_transferable_cap (ReplyCap t False R)"
-  using is_transferable.simps by simp
-
-lemma is_transferable_NoneE:
-  assumes hyp: "is_transferable opt_cap"
-  obtains "opt_cap = None" | cap where "opt_cap = Some cap" and "is_transferable_cap cap"
-  by (rule is_transferable.cases[OF hyp];simp)
-
-lemma is_transferable_Untyped[simp]: "\<not> is_transferable (Some (UntypedCap dev ptr sz freeIndex))"
-  by (blast elim: is_transferable.cases)
-lemma is_transferable_IRQ[simp]: "\<not> is_transferable_cap IRQControlCap"
-  by (blast elim: is_transferable.cases)
-lemma is_transferable_Zombie[simp]: "\<not> is_transferable (Some (Zombie ptr sz n))"
-  by (blast elim: is_transferable.cases)
-lemma is_transferable_Ntfn[simp]: "\<not> is_transferable (Some (NotificationCap ntfn badge R))"
-  by (blast elim: is_transferable.cases)
-lemma is_transferable_Endpoint[simp]: "\<not> is_transferable (Some (EndpointCap ntfn badge R))"
-  by (blast elim: is_transferable.cases)
-
-(*FIXME MOVE *)
-lemmas descendants_incD
-    = descendants_inc_def[THEN meta_eq_to_obj_eq, THEN iffD1, rule_format]
-
-lemma acap_class_reply:
-  "(acap_class acap \<noteq> ReplyClass t)"
-  (* warning: arch split *)
-  by (cases acap; simp)
-
-lemma cap_class_reply:
-  "(cap_class cap = ReplyClass t) = (\<exists>r m. cap = ReplyCap t m r)"
-  by (cases cap; simp add: acap_class_reply)
-
-lemma reply_cap_no_children:
-  "\<lbrakk> valid_mdb s; caps_of_state s p = Some (ReplyCap t False r) \<rbrakk> \<Longrightarrow> cdt s p' \<noteq> Some p"
-  apply (clarsimp simp: valid_mdb_def)
-  apply (frule descendants_incD[where p=p' and p'=p])
-   apply (rule child_descendant)
-   apply (fastforce)
-  apply clarsimp
-  apply (subgoal_tac "caps_of_state s p' \<noteq> None")
-   apply (clarsimp simp: cap_class_reply)
-   apply (simp only: reply_mdb_def reply_caps_mdb_def reply_masters_mdb_def)
-   apply (elim conjE allE[where x=p'])
-   apply simp
-  apply (drule(1) mdb_cte_atD)
-  apply (fastforce simp add: cte_wp_at_def caps_of_state_def)
-  done
-
-(*FIXME MOVE *)
-lemmas all_childrenI = all_children_def[THEN meta_eq_to_obj_eq, THEN iffD2, rule_format]
-lemmas all_childrenD = all_children_def[THEN meta_eq_to_obj_eq, THEN iffD1, rule_format]
-
-(*FIXME MOVE *)
-lemma valid_mdb_descendants_inc[elim!]:
-  "valid_mdb s \<Longrightarrow> descendants_inc (cdt s) (caps_of_state s)"
-  by (simp add:valid_mdb_def)
-
-(*FIXME MOVE *)
-lemma valid_mdb_mdb_cte_at [elim!]:
-  "valid_mdb s \<Longrightarrow> mdb_cte_at (swp (cte_wp_at ((\<noteq>) NullCap)) s) (cdt s)"
-  by (simp add:valid_mdb_def)
-
-(*FIXME MOVE *)
-lemma descendants_inc_cap_classD:
-  "\<lbrakk> descendants_inc m caps; p \<in> descendants_of p' m; caps p = Some cap ; caps p' = Some cap'\<rbrakk>
-   \<Longrightarrow> cap_class cap = cap_class cap'"
-  by (fastforce dest:descendants_incD)
-
-lemma is_transferable_all_children:
-  "valid_mdb s \<Longrightarrow> all_children (\<lambda>slot . is_transferable (caps_of_state s slot)) (cdt s)"
-  apply (rule all_childrenI)
-  apply (erule is_transferable.cases)
-    apply (fastforce dest: mdb_cte_atD valid_mdb_mdb_cte_at
-                     simp: mdb_cte_at_def cte_wp_at_def caps_of_state_def)
-   apply (fastforce dest: mdb_cte_atD valid_mdb_mdb_cte_at
-                    simp: mdb_cte_at_def cte_wp_at_def caps_of_state_def)
-  apply (blast dest:reply_cap_no_children)
-done
-
-
-
 
 subsection \<open>Generating a policy from the current cap, ASID and IRQs distribution\<close>
 
-(* TODO split that section between stba sata and sita and move a maximun
+(* TODO split that section between sbta sata and sita and move a maximum
    of accesor functions back to AInvs *)
 
-
+(* FIXME: update comment *)
 text \<open>
   sbta_caps/sbta_asid imply that a thread and it's vspace are labelled
   the same -- caps_of_state (tcb, vspace_index) will be the PD cap.
@@ -542,224 +167,75 @@ text \<open>
 
 \<close>
 
-primrec aobj_ref' :: "arch_cap \<Rightarrow> obj_ref set"
-where
-  "aobj_ref' (arch_cap.ASIDPoolCap p as) = {p}"
-| "aobj_ref' arch_cap.ASIDControlCap = {}"
-| "aobj_ref' (arch_cap.PageCap isdev x rs sz as4) = ptr_range x (pageBitsForSize sz)"
-| "aobj_ref' (arch_cap.PageDirectoryCap x as2) = {x}"
-| "aobj_ref' (arch_cap.PageTableCap x as3) = {x}"
+primrec obj_refs :: "cap \<Rightarrow> obj_ref set" where
+  "obj_refs NullCap = {}"
+| "obj_refs (ReplyCap r m cr) = {r}"
+| "obj_refs IRQControlCap = {}"
+| "obj_refs (IRQHandlerCap irq) = {}"
+| "obj_refs (UntypedCap d r s f) = {}"
+| "obj_refs (CNodeCap r bits guard) = {r}"
+| "obj_refs (EndpointCap r b cr) = {r}"
+| "obj_refs (NotificationCap r b cr) = {r}"
+| "obj_refs (ThreadCap r) = {r}"
+| "obj_refs (Zombie ptr b n) = {ptr}"
+| "obj_refs (ArchObjectCap x) = aobj_ref' x"
+| "obj_refs DomainCap = UNIV" (* hack, see above *)
 
-primrec obj_refs :: "cap \<Rightarrow> obj_ref set"
-where
-  "obj_refs cap.NullCap = {}"
-| "obj_refs (cap.ReplyCap r m cr) = {r}"
-| "obj_refs cap.IRQControlCap = {}"
-| "obj_refs (cap.IRQHandlerCap irq) = {}"
-| "obj_refs (cap.UntypedCap d r s f) = {}"
-| "obj_refs (cap.CNodeCap r bits guard) = {r}"
-| "obj_refs (cap.EndpointCap r b cr) = {r}"
-| "obj_refs (cap.NotificationCap r b cr) = {r}"
-| "obj_refs (cap.ThreadCap r) = {r}"
-| "obj_refs (cap.Zombie ptr b n) = {ptr}"
-| "obj_refs (cap.ArchObjectCap x) = aobj_ref' x"
-| "obj_refs cap.DomainCap = UNIV" (* hack, see above *)
+fun cap_irqs_controlled :: "cap \<Rightarrow> irq set" where
+  "cap_irqs_controlled IRQControlCap = UNIV"
+| "cap_irqs_controlled (IRQHandlerCap irq) = {irq}"
+| "cap_irqs_controlled _ = {}"
 
-inductive_set state_bits_to_policy for caps thread_sts thread_bas cdt vrefs
-where
-  sbta_caps: "\<lbrakk> caps ptr = Some cap; oref \<in> obj_refs cap;
-                auth \<in> cap_auth_conferred cap \<rbrakk>
-           \<Longrightarrow> (fst ptr, auth, oref) \<in> state_bits_to_policy caps thread_sts thread_bas cdt vrefs"
-| sbta_untyped: "\<lbrakk> caps ptr = Some cap; oref \<in> untyped_range cap \<rbrakk>
-           \<Longrightarrow> (fst ptr, Control, oref) \<in> state_bits_to_policy caps thread_sts thread_bas cdt vrefs"
-| sbta_ts: "\<lbrakk> (oref', auth) \<in> thread_sts oref \<rbrakk>
-           \<Longrightarrow> (oref, auth, oref') \<in> state_bits_to_policy caps thread_sts thread_bas cdt vrefs"
-| sbta_bounds: "\<lbrakk>thread_bas oref = Some oref'; auth \<in> {Receive, Reset} \<rbrakk>
-           \<Longrightarrow> (oref, auth, oref') \<in> state_bits_to_policy caps thread_sts thread_bas cdt vrefs"
-| sbta_cdt: "\<lbrakk> cdt slot' = Some slot ; \<not>is_transferable (caps slot') \<rbrakk>
-           \<Longrightarrow> (fst slot, Control, fst slot')
-                                   \<in> state_bits_to_policy caps thread_sts thread_bas cdt vrefs"
-| sbta_cdt_transferable: "\<lbrakk>cdt slot' = Some slot\<rbrakk>
-           \<Longrightarrow> (fst slot, DeleteDerived, fst slot')
-                                   \<in> state_bits_to_policy caps thread_sts thread_bas cdt vrefs"
-| sbta_vref: "\<lbrakk> (ptr', ref, auth) \<in> vrefs ptr \<rbrakk>
-           \<Longrightarrow> (ptr, auth, ptr') \<in> state_bits_to_policy caps thread_sts thread_bas cdt vrefs"
+inductive_set state_irqs_to_policy_aux for aag caps where
+  sita_controlled:
+    "\<lbrakk> caps ptr = Some cap; irq \<in> cap_irqs_controlled cap \<rbrakk>
+       \<Longrightarrow> (pasObjectAbs aag (fst ptr), Control, pasIRQAbs aag irq) \<in> state_irqs_to_policy_aux aag caps"
 
-fun cap_asid' :: "cap \<Rightarrow> asid set"
-where
-  "cap_asid' (ArchObjectCap (PageCap _ _ _ _ mapping))
-      = fst ` set_option mapping"
-  | "cap_asid' (ArchObjectCap (PageTableCap _ mapping))
-      = fst ` set_option mapping"
-  | "cap_asid' (ArchObjectCap (PageDirectoryCap _ asid_opt))
-      = set_option asid_opt"
-  | "cap_asid' (ArchObjectCap (ASIDPoolCap _ asid))
-          = {x. asid_high_bits_of x = asid_high_bits_of asid \<and> x \<noteq> 0}"
-  | "cap_asid' (ArchObjectCap ASIDControlCap) = UNIV"
-  | "cap_asid' _ = {}"
-
-inductive_set state_asids_to_policy_aux for aag caps asid_tab vrefs
-where
-    sata_asid: "\<lbrakk> caps ptr = Some cap; asid \<in> cap_asid' cap \<rbrakk>
-              \<Longrightarrow> ( pasObjectAbs aag (fst ptr), Control, pasASIDAbs aag asid)
-                        \<in> state_asids_to_policy_aux aag caps asid_tab vrefs"
-  | sata_asid_lookup: "\<lbrakk> asid_tab (asid_high_bits_of asid) = Some poolptr;
-                           (pdptr, VSRef (asid && mask asid_low_bits)
-                                         (Some AASIDPool), a) \<in> vrefs poolptr \<rbrakk>
-                       \<Longrightarrow> (pasASIDAbs aag asid, a, pasObjectAbs aag pdptr)
-                              \<in> state_asids_to_policy_aux aag caps asid_tab vrefs"
-  | sata_asidpool:    "\<lbrakk> asid_tab (asid_high_bits_of asid) = Some poolptr; asid \<noteq> 0 \<rbrakk> \<Longrightarrow>
-                        (pasObjectAbs aag poolptr, ASIDPoolMapsASID, pasASIDAbs aag asid)
-                                             \<in> state_asids_to_policy_aux aag caps asid_tab vrefs"
-
-fun cap_irqs_controlled :: "cap \<Rightarrow> irq set"
-where
-  "cap_irqs_controlled cap.IRQControlCap = UNIV"
-  | "cap_irqs_controlled (cap.IRQHandlerCap irq) = {irq}"
-  | "cap_irqs_controlled _ = {}"
-
-inductive_set state_irqs_to_policy_aux for aag caps
-where
-  sita_controlled: "\<lbrakk> caps ptr = Some cap; irq \<in> cap_irqs_controlled cap \<rbrakk>
-  \<Longrightarrow> (pasObjectAbs aag (fst ptr), Control, pasIRQAbs aag irq) \<in> state_irqs_to_policy_aux aag caps"
-
-abbreviation state_irqs_to_policy
-where
+abbreviation state_irqs_to_policy where
   "state_irqs_to_policy aag s \<equiv> state_irqs_to_policy_aux aag (caps_of_state s)"
 
-definition irq_map_wellformed_aux
-where
+definition irq_map_wellformed_aux where
   "irq_map_wellformed_aux aag irqs \<equiv> \<forall>irq. pasObjectAbs aag (irqs irq) = pasIRQAbs aag irq"
 
-abbreviation irq_map_wellformed
-where
+abbreviation irq_map_wellformed where
   "irq_map_wellformed aag s \<equiv> irq_map_wellformed_aux aag (interrupt_irq_node s)"
 
-definition state_vrefs
-where
-  "state_vrefs s = case_option {} vs_refs_no_global_pts o kheap s"
-
-abbreviation state_asids_to_policy
-where
-  "state_asids_to_policy aag s \<equiv> state_asids_to_policy_aux aag (caps_of_state s)
-        (arm_asid_table (arch_state s)) (state_vrefs s)"
-
-definition tcb_states_of_state
-where
-  "tcb_states_of_state s \<equiv> \<lambda>p. option_map tcb_state (get_tcb p s)"
-
-(* FIXME: RENAME: should be named something thread_st_auth. thread_states is confusing as
-   it outputs autorities *)
-definition thread_states
-where
+(* FIXME: rename to thread_st_auth or similar since it outputs authorities *)
+definition thread_states where
   "thread_states s \<equiv> case_option {} tcb_st_to_auth \<circ> tcb_states_of_state s"
 
-definition thread_bound_ntfns
-where
-  "thread_bound_ntfns s \<equiv> \<lambda>p. case (get_tcb p s) of None \<Rightarrow> None
-                                                  | Some tcb \<Rightarrow> tcb_bound_notification tcb"
+definition thread_bound_ntfns where
+  "thread_bound_ntfns s \<equiv> \<lambda>p. case_option None tcb_bound_notification (get_tcb p s)"
 
-definition state_objs_to_policy
-where
-  "state_objs_to_policy s =
-      state_bits_to_policy (caps_of_state s) (thread_states s) (thread_bound_ntfns s)
-                           (cdt s) (state_vrefs s)"
+inductive_set state_bits_to_policy for caps thread_sts thread_bas cdt vrefs where
+  sbta_caps:
+    "\<lbrakk> caps ptr = Some cap; oref \<in> obj_refs cap; auth \<in> cap_auth_conferred cap \<rbrakk>
+       \<Longrightarrow> (fst ptr, auth, oref) \<in> state_bits_to_policy caps thread_sts thread_bas cdt vrefs"
+| sbta_untyped:
+    "\<lbrakk> caps ptr = Some cap; oref \<in> untyped_range cap \<rbrakk>
+       \<Longrightarrow> (fst ptr, Control, oref) \<in> state_bits_to_policy caps thread_sts thread_bas cdt vrefs"
+| sbta_ts:
+    "(oref', auth) \<in> thread_sts oref
+     \<Longrightarrow> (oref, auth, oref') \<in> state_bits_to_policy caps thread_sts thread_bas cdt vrefs"
+| sbta_bounds:
+    "\<lbrakk> thread_bas oref = Some oref'; auth \<in> {Receive, Reset} \<rbrakk>
+       \<Longrightarrow> (oref, auth, oref') \<in> state_bits_to_policy caps thread_sts thread_bas cdt vrefs"
+| sbta_cdt:
+    "\<lbrakk> cdt slot' = Some slot ; \<not>is_transferable (caps slot') \<rbrakk>
+       \<Longrightarrow> (fst slot, Control, fst slot') \<in> state_bits_to_policy caps thread_sts thread_bas cdt vrefs"
+| sbta_cdt_transferable:
+    "cdt slot' = Some slot
+     \<Longrightarrow> (fst slot, DeleteDerived, fst slot') \<in> state_bits_to_policy caps thread_sts thread_bas cdt vrefs"
+| sbta_vref:
+    "(ptr', _, _, auth) \<in> vrefs ptr
+     \<Longrightarrow> (ptr, auth, ptr') \<in> state_bits_to_policy caps thread_sts thread_bas cdt vrefs"
 
-lemmas state_objs_to_policy_mem = eqset_imp_iff[OF state_objs_to_policy_def]
+definition state_objs_to_policy :: "det_ext state \<Rightarrow> (obj_ref \<times> auth \<times> obj_ref) set" where
+  "state_objs_to_policy s = state_bits_to_policy (caps_of_state s) (thread_states s)
+                                                 (thread_bound_ntfns s) (cdt s) (state_vrefs s)"
 
-lemmas state_objs_to_policy_intros
-    = state_bits_to_policy.intros[THEN state_objs_to_policy_mem[THEN iffD2]]
-
-(* FIXME this is non resilient at all to adding or removing rules to or from state_bits_to_policy *)
-lemmas sta_caps = state_objs_to_policy_intros(1)
-  and sta_untyped = state_objs_to_policy_intros(2)
-  and sta_ts = state_objs_to_policy_intros(3)
-  and sta_bas = state_objs_to_policy_intros(4)
-  and sta_cdt = state_objs_to_policy_intros(5)
-  and sta_cdt_transferable = state_objs_to_policy_intros(6)
-  and sta_vref = state_objs_to_policy_intros(7)
-
-lemmas state_objs_to_policy_cases
-    = state_bits_to_policy.cases[OF state_objs_to_policy_mem[THEN iffD1]]
-
-end
-
-context pspace_update_eq begin
-
-interpretation Arch . (*FIXME: arch_split*)
-
-lemma state_vrefs[iff]: "state_vrefs (f s) = state_vrefs s"
-  by (simp add: state_vrefs_def pspace)
-
-lemma thread_states[iff]: "thread_states (f s) = thread_states s"
-  by (simp add: thread_states_def pspace get_tcb_def swp_def tcb_states_of_state_def)
-
-lemma thread_bound_ntfns[iff]: "thread_bound_ntfns (f s) = thread_bound_ntfns s"
-  by (simp add: thread_bound_ntfns_def pspace get_tcb_def swp_def split: option.splits)
-
-(*
-  lemma ipc_buffers_of_state[iff]: "ipc_buffers_of_state (f s) = ipc_buffers_of_state s"
-  by (simp add: ipc_buffers_of_state_def pspace get_tcb_def swp_def)
-*)
-
-end
-
-context begin interpretation Arch . (*FIXME: arch_split*)
-
-lemma tcb_states_of_state_preserved:
-  "\<lbrakk> get_tcb thread s = Some tcb; tcb_state tcb' = tcb_state tcb \<rbrakk>
-     \<Longrightarrow> tcb_states_of_state (s\<lparr>kheap := kheap s(thread \<mapsto> TCB tcb')\<rparr>) = tcb_states_of_state s"
-  apply rule
-  apply (auto split: option.splits simp: tcb_states_of_state_def get_tcb_def)
-  done
-
-lemma thread_states_preserved:
-  "\<lbrakk> get_tcb thread s = Some tcb; tcb_state tcb' = tcb_state tcb \<rbrakk>
-     \<Longrightarrow> thread_states (s\<lparr>kheap := kheap s(thread \<mapsto> TCB tcb')\<rparr>) = thread_states s"
-  by (simp add: tcb_states_of_state_preserved thread_states_def)
-
-lemma thread_bound_ntfns_preserved:
-  "\<lbrakk> get_tcb thread s = Some tcb; tcb_bound_notification tcb' = tcb_bound_notification tcb \<rbrakk>
-     \<Longrightarrow> thread_bound_ntfns (s\<lparr>kheap := kheap s(thread \<mapsto> TCB tcb')\<rparr>) = thread_bound_ntfns s"
-  by (auto simp:  thread_bound_ntfns_def get_tcb_def split: option.splits)
-
-(* FIXME: move all three *)
-lemma null_filterI:
-  "\<lbrakk> cs p = Some cap; cap \<noteq> cap.NullCap \<rbrakk> \<Longrightarrow> null_filter cs p = Some cap"
-  unfolding null_filter_def by auto
-lemma null_filterI2:
-  "\<lbrakk> cs p = None \<rbrakk> \<Longrightarrow> null_filter cs p = None"
-  unfolding null_filter_def by auto
-
-lemma null_filterE2:
-  "\<lbrakk> null_filter cps x = None;
-      \<lbrakk> cps x = Some NullCap \<rbrakk> \<Longrightarrow> R ; \<lbrakk> cps x = None \<rbrakk> \<Longrightarrow> R  \<rbrakk>
-     \<Longrightarrow> R"
-  by (simp add: null_filter_def split: if_split_asm)
-
-lemma is_transferable_null_filter[simp]:
-  "is_transferable (null_filter caps ptr) = is_transferable (caps ptr)"
-  by (auto simp: is_transferable.simps null_filter_def)
-
-lemma sbta_null_filter:
-  "state_bits_to_policy (null_filter cs) sr bar cd vr = state_bits_to_policy cs sr bar cd vr"
-  apply (rule subset_antisym)
-  apply clarsimp
-  apply (erule state_bits_to_policy.induct,
-        (fastforce intro: state_bits_to_policy.intros
-                   elim: null_filterE null_filterE2 split: option.splits)+)[1]
-  apply clarsimp
-  apply (erule state_bits_to_policy.induct)
-  by (fastforce intro: state_bits_to_policy.intros null_filterI split:option.splits)+
-
-lemma sata_null_filter:
-  "state_asids_to_policy_aux aag (null_filter cs) asid_tab vrefs
-        = state_asids_to_policy_aux aag cs asid_tab vrefs"
-  by (auto elim!: state_asids_to_policy_aux.induct null_filterE
-           intro: state_asids_to_policy_aux.intros sata_asid[OF null_filterI])
 
 subsection \<open>Policy Refinement\<close>
-
 
 text\<open>
 
@@ -771,27 +247,18 @@ unauthorised subjects (see integrity_ready_queues).
 
 \<close>
 
-inductive_set domains_of_state_aux for ekheap
-where
-  domtcbs: "\<lbrakk> ekheap ptr = Some etcb; d = tcb_domain etcb \<rbrakk>
-  \<Longrightarrow> (ptr, d) \<in> domains_of_state_aux ekheap"
+inductive_set domains_of_state_aux for ekheap where
+  domtcbs:
+    "\<lbrakk> ekheap ptr = Some etcb; d = tcb_domain etcb \<rbrakk> \<Longrightarrow> (ptr, d) \<in> domains_of_state_aux ekheap"
 
-abbreviation domains_of_state
-where
-  "domains_of_state s \<equiv> domains_of_state_aux (ekheap s)"
+abbreviation "domains_of_state s \<equiv> domains_of_state_aux (ekheap s)"
 
-definition tcb_domain_map_wellformed_aux
-where
+definition tcb_domain_map_wellformed_aux where
   "tcb_domain_map_wellformed_aux aag etcbs_doms \<equiv>
      \<forall>(ptr, d) \<in> etcbs_doms. pasObjectAbs aag ptr \<in> pasDomainAbs aag d"
 
-abbreviation tcb_domain_map_wellformed
-where
+abbreviation tcb_domain_map_wellformed where
   "tcb_domain_map_wellformed aag s \<equiv> tcb_domain_map_wellformed_aux aag (domains_of_state s)"
-
-lemma tcb_domain_map_wellformed_mono:
-  "\<lbrakk> domains_of_state s' \<subseteq> domains_of_state s; tcb_domain_map_wellformed pas s \<rbrakk> \<Longrightarrow> tcb_domain_map_wellformed pas s'"
-by (auto simp: tcb_domain_map_wellformed_aux_def get_etcb_def)
 
 text\<open>
 
@@ -799,8 +266,7 @@ We sometimes need to know that our current subject may run in the current domain
 
 \<close>
 
-abbreviation
-  "pas_cur_domain aag s \<equiv> pasSubject aag \<in> pasDomainAbs aag (cur_domain s)"
+abbreviation "pas_cur_domain aag s \<equiv> pasSubject aag \<in> pasDomainAbs aag (cur_domain s)"
 
 text\<open>
 
@@ -815,15 +281,17 @@ the policy:
 \end{itemize}
 
 \<close>
-abbreviation state_objs_in_policy :: "'a PAS \<Rightarrow> det_ext state \<Rightarrow> bool"
-where
+
+abbreviation state_objs_in_policy :: "'a PAS \<Rightarrow> det_ext state \<Rightarrow> bool" where
   "state_objs_in_policy aag s \<equiv>
                 auth_graph_map (pasObjectAbs aag) (state_objs_to_policy s) \<subseteq> pasPolicy aag"
 
+abbreviation state_asids_to_policy :: "'a PAS \<Rightarrow> det_ext state \<Rightarrow> ('a \<times> auth \<times> 'a) set" where
+  "state_asids_to_policy aag s \<equiv>
+     state_asids_to_policy_arch aag (caps_of_state s) (arch_state s) (state_vrefs s)"
 
-definition pas_refined :: "'a PAS \<Rightarrow> det_ext state \<Rightarrow> bool"
-where
- "pas_refined aag \<equiv> \<lambda>s.
+definition pas_refined :: "'a PAS \<Rightarrow> det_ext state \<Rightarrow> bool" where
+  "pas_refined aag \<equiv> \<lambda>s.
      pas_wellformed aag
    \<and> irq_map_wellformed aag s
    \<and> tcb_domain_map_wellformed aag s
@@ -831,237 +299,89 @@ where
    \<and> state_asids_to_policy aag s \<subseteq> pasPolicy aag
    \<and> state_irqs_to_policy aag s \<subseteq> pasPolicy aag"
 
-lemma pas_refined_mem:
-  "\<lbrakk> (x, auth, y) \<in> state_objs_to_policy s; pas_refined aag s \<rbrakk>
-       \<Longrightarrow> (pasObjectAbs aag x, auth, pasObjectAbs aag y) \<in> pasPolicy aag"
-  by (auto simp: pas_refined_def intro: auth_graph_map_memI)
-
-lemma pas_refined_wellformed[elim!]:
-  "pas_refined aag s \<Longrightarrow> pas_wellformed aag"
-  unfolding pas_refined_def by simp
-
-lemmas pas_refined_Control
-    = aag_wellformed_Control[OF _ pas_refined_wellformed]
-  and pas_refined_refl = aag_wellformed_refl [OF pas_refined_wellformed]
-
-lemma caps_of_state_pasObjectAbs_eq:
-  "\<lbrakk> caps_of_state s p = Some cap; Control \<in> cap_auth_conferred cap;
-     is_subject aag (fst p); pas_refined aag s;
-     x \<in> obj_refs cap \<rbrakk>
-       \<Longrightarrow> is_subject aag x"
-  apply (frule sta_caps, simp+)
-  apply (drule pas_refined_mem, simp+)
-  apply (drule pas_refined_Control, simp+)
-  done
-
-lemma pas_refined_state_objs_to_policy_subset:
-  "\<lbrakk> pas_refined aag s;
-     state_objs_to_policy s' \<subseteq> state_objs_to_policy s;
-     state_asids_to_policy aag s' \<subseteq> state_asids_to_policy aag s;
-     state_irqs_to_policy aag s' \<subseteq> state_irqs_to_policy aag s;
-     domains_of_state s' \<subseteq> domains_of_state s;
-     interrupt_irq_node s' = interrupt_irq_node s
-    \<rbrakk>
-    \<Longrightarrow> pas_refined aag s'"
-by (simp add: pas_refined_def) (blast dest: tcb_domain_map_wellformed_mono dest: auth_graph_map_mono[where G="pasObjectAbs aag"])
-
-lemma aag_wellformed_all_auth_is_owns':
-  "\<lbrakk> Control \<in> S; pas_wellformed aag \<rbrakk> \<Longrightarrow> (\<forall>auth \<in> S. aag_has_auth_to aag auth x) = (is_subject aag x)"
-  apply (rule iffI)
-   apply (drule (1) bspec)
-   apply (frule (1) aag_wellformed_Control )
-   apply fastforce
-  apply (clarsimp simp: aag_wellformed_refl)
-  done
-
-lemmas aag_wellformed_all_auth_is_owns
-   = aag_wellformed_all_auth_is_owns'[where S=UNIV, simplified]
-     aag_wellformed_all_auth_is_owns'[where S="{Control}", simplified]
-
-lemmas aag_wellformed_control_is_owns
-   = aag_wellformed_all_auth_is_owns'[where S="{Control}", simplified]
-
-lemmas pas_refined_all_auth_is_owns = aag_wellformed_all_auth_is_owns[OF pas_refined_wellformed]
-
-lemma pas_refined_sita_mem:
-  "\<lbrakk> (x, auth, y) \<in> state_irqs_to_policy aag s; pas_refined aag s \<rbrakk>
-       \<Longrightarrow> (x, auth, y) \<in> pasPolicy aag"
-  by (auto simp: pas_refined_def)
-
-
-
 
 section \<open>Integrity definition\<close>
 
 subsection \<open>How kernel objects can change\<close>
 
-fun blocked_on :: "obj_ref \<Rightarrow> Structures_A.thread_state \<Rightarrow> bool"
-where
-    "blocked_on ref (Structures_A.BlockedOnReceive ref' _)     = (ref = ref')"
-  | "blocked_on ref (Structures_A.BlockedOnSend    ref' _)     = (ref = ref')"
-  | "blocked_on ref (Structures_A.BlockedOnNotification ref')  = (ref = ref')"
-  | "blocked_on _ _ = False"
+fun blocked_on :: "obj_ref \<Rightarrow> thread_state \<Rightarrow> bool" where
+  "blocked_on ref (BlockedOnReceive ref' _)    = (ref = ref')"
+| "blocked_on ref (BlockedOnSend    ref' _)    = (ref = ref')"
+| "blocked_on ref (BlockedOnNotification ref') = (ref = ref')"
+| "blocked_on _ _ = False"
 
-lemma blocked_on_def2:
-  "blocked_on ref ts = (ref \<in> fst ` tcb_st_to_auth ts)"
-  by (cases ts, simp_all)
-
-fun receive_blocked_on :: "obj_ref \<Rightarrow> Structures_A.thread_state \<Rightarrow> bool"
-where
-   "receive_blocked_on ref (Structures_A.BlockedOnReceive ref' _)     = (ref = ref')"
-  | "receive_blocked_on ref (Structures_A.BlockedOnNotification ref') = (ref = ref')"
-  | "receive_blocked_on _ _ = False"
+fun receive_blocked_on :: "obj_ref \<Rightarrow> thread_state \<Rightarrow> bool" where
+  "receive_blocked_on ref (BlockedOnReceive ref' _)    = (ref = ref')"
+| "receive_blocked_on ref (BlockedOnNotification ref') = (ref = ref')"
+| "receive_blocked_on _ _ = False"
 
 lemma receive_blocked_on_def2:
   "receive_blocked_on ref ts = ((ref, Receive) \<in> tcb_st_to_auth ts)"
   by (cases ts, simp_all)
 
-fun can_receive_ipc :: "Structures_A.thread_state \<Rightarrow> bool"
-where
-   "can_receive_ipc (Structures_A.BlockedOnReceive _ _)     = True"
-  | "can_receive_ipc (Structures_A.BlockedOnSend _ pl)     =
-         (sender_is_call pl \<and> (sender_can_grant pl \<or> sender_can_grant_reply pl))"
-  | "can_receive_ipc (Structures_A.BlockedOnNotification _) = True"
-  | "can_receive_ipc Structures_A.BlockedOnReply = True"
-  | "can_receive_ipc _ = False"
-
-lemma receive_blocked_on_can_receive_ipc[elim!,simp]:
-  "receive_blocked_on ref ts \<Longrightarrow>can_receive_ipc ts"
-  by (cases ts;simp)
-
-lemma receive_blocked_on_can_receive_ipc'[elim!,simp]:
-  "case_option False (receive_blocked_on ref) tsopt \<Longrightarrow> case_option False can_receive_ipc tsopt"
-  by (cases tsopt;simp)
-
-
-fun send_blocked_on :: "obj_ref \<Rightarrow> Structures_A.thread_state \<Rightarrow> bool"
-where
-  "send_blocked_on ref (Structures_A.BlockedOnSend ref' _)     = (ref = ref')"
-  | "send_blocked_on _ _ = False"
+fun send_blocked_on :: "obj_ref \<Rightarrow> thread_state \<Rightarrow> bool" where
+  "send_blocked_on ref (BlockedOnSend ref' _) = (ref = ref')"
+| "send_blocked_on _ _ = False"
 
 lemma send_blocked_on_def2:
   "send_blocked_on ref ts = ((ref, SyncSend) \<in> tcb_st_to_auth ts)"
   by (cases ts, simp_all)
 
-lemma send_blocked_on_def3:
-  "send_blocked_on ref ts = (\<exists> pl. ts = BlockedOnSend ref pl)"
-  by (cases ts; force)
-
-fun send_is_call :: "Structures_A.thread_state \<Rightarrow> bool"
-where
-  "send_is_call (Structures_A.BlockedOnSend _ payl) = sender_is_call payl"
+fun send_is_call :: "thread_state \<Rightarrow> bool" where
+  "send_is_call (BlockedOnSend _ payl) = sender_is_call payl"
 | "send_is_call _ = False"
 
+definition tcb_bound_notification_reset_integrity ::
+  "obj_ref option \<Rightarrow> obj_ref option \<Rightarrow> 'a set \<Rightarrow> 'a PAS \<Rightarrow> bool" where
+  "tcb_bound_notification_reset_integrity ntfn ntfn' subjects aag \<equiv>
+     (ntfn = ntfn') \<comment> \<open>no change to bound ntfn\<close>
+   \<or> (ntfn' = None \<and> aag_subjects_have_auth_to subjects aag Reset (the ntfn)) \<comment> \<open>ntfn is unbound\<close>"
 
-
-definition tcb_bound_notification_reset_integrity
-  :: "obj_ref option \<Rightarrow> obj_ref option \<Rightarrow> 'a set \<Rightarrow> 'a PAS \<Rightarrow> bool"
-where
-  "tcb_bound_notification_reset_integrity ntfn ntfn' subjects aag
-    = ((ntfn = ntfn') \<comment> \<open>no change to bound ntfn\<close>
-       \<or> (ntfn' = None \<and> aag_subjects_have_auth_to subjects aag Reset (the ntfn))
-         \<comment> \<open>ntfn is unbound\<close>)"
-
-lemma tcb_bound_notification_reset_integrity_refl[simp]:
-  "tcb_bound_notification_reset_integrity ntfn ntfn subjects aag"
-  by (simp add: tcb_bound_notification_reset_integrity_def)
-
-
-definition direct_send :: "'a set \<Rightarrow> 'a PAS \<Rightarrow> obj_ref \<Rightarrow> tcb \<Rightarrow> bool"
-where
+definition direct_send :: "'a set \<Rightarrow> 'a PAS \<Rightarrow> obj_ref \<Rightarrow> tcb \<Rightarrow> bool" where
   "direct_send subjects aag ep tcb \<equiv> receive_blocked_on ep (tcb_state tcb) \<and>
-                                   (aag_subjects_have_auth_to subjects aag SyncSend ep
-                                     \<or> aag_subjects_have_auth_to subjects aag Notify ep)"
+                                     (aag_subjects_have_auth_to subjects aag SyncSend ep \<or>
+                                      aag_subjects_have_auth_to subjects aag Notify ep)"
 
-abbreviation ep_recv_blocked :: "obj_ref \<Rightarrow> thread_state \<Rightarrow> bool"
-where
-  "ep_recv_blocked ep ts \<equiv> case ts of BlockedOnReceive w _ \<Rightarrow> w = ep
-                             | _ \<Rightarrow> False"
+abbreviation ep_recv_blocked :: "obj_ref \<Rightarrow> thread_state \<Rightarrow> bool" where
+  "ep_recv_blocked ep ts \<equiv> case ts of BlockedOnReceive w _ \<Rightarrow> w = ep | _ \<Rightarrow> False"
 
-definition direct_call :: "'a set \<Rightarrow> 'a PAS \<Rightarrow> obj_ref \<Rightarrow> thread_state \<Rightarrow> bool"
-where
+definition direct_call :: "'a set \<Rightarrow> 'a PAS \<Rightarrow> obj_ref \<Rightarrow> thread_state \<Rightarrow> bool" where
   "direct_call subjects aag ep tcbst \<equiv> ep_recv_blocked ep (tcbst) \<and>
-                                   aag_subjects_have_auth_to subjects aag Call ep"
+                                        aag_subjects_have_auth_to subjects aag Call ep"
 
-definition indirect_send :: "'a set \<Rightarrow> 'a PAS \<Rightarrow> obj_ref \<Rightarrow> obj_ref \<Rightarrow> tcb \<Rightarrow> bool"
-where
-  "indirect_send subjects aag ntfn recv_ep tcb \<equiv> ep_recv_blocked recv_ep (tcb_state tcb)
-                                                    \<comment> \<open>tcb is blocked on sync ep\<close>
-                                         \<and> (tcb_bound_notification tcb = Some ntfn)
-                                         \<and> aag_subjects_have_auth_to subjects aag Notify ntfn"
+definition indirect_send :: "'a set \<Rightarrow> 'a PAS \<Rightarrow> obj_ref \<Rightarrow> obj_ref \<Rightarrow> tcb \<Rightarrow> bool" where
+  "indirect_send subjects aag ntfn recv_ep tcb \<equiv>
+     ep_recv_blocked recv_ep (tcb_state tcb) \<and> aag_subjects_have_auth_to subjects aag Notify ntfn
+              \<comment> \<open>tcb is blocked on sync ep\<close> \<and> (tcb_bound_notification tcb = Some ntfn)"
 
+definition call_blocked :: "obj_ref \<Rightarrow> thread_state \<Rightarrow> bool" where
+  "call_blocked ep tst \<equiv> \<exists>pl. tst = BlockedOnSend ep pl \<and> sender_is_call pl"
 
-definition call_blocked :: "obj_ref \<Rightarrow> thread_state \<Rightarrow> bool"
-where
-  "call_blocked ep tst \<equiv> \<exists> pl. tst = BlockedOnSend ep pl \<and> sender_is_call pl"
-
-definition allowed_call_blocked :: "obj_ref \<Rightarrow> thread_state \<Rightarrow> bool"
-where
-  "allowed_call_blocked ep tst \<equiv> \<exists> pl. tst = BlockedOnSend ep pl \<and> sender_is_call pl \<and>
+definition allowed_call_blocked :: "obj_ref \<Rightarrow> thread_state \<Rightarrow> bool" where
+  "allowed_call_blocked ep tst \<equiv> \<exists>pl. tst = BlockedOnSend ep pl \<and> sender_is_call pl \<and>
                                               (sender_can_grant pl \<or> sender_can_grant_reply pl)"
 
-lemma allowed_call_blocked_call_blocked[elim!]:
-  "allowed_call_blocked ep tst \<Longrightarrow> call_blocked ep tst"
-  unfolding allowed_call_blocked_def call_blocked_def by fastforce
-
-definition direct_reply :: "'a set \<Rightarrow> 'a PAS \<Rightarrow> 'a \<Rightarrow> tcb \<Rightarrow> bool"
-where
+definition direct_reply :: "'a set \<Rightarrow> 'a PAS \<Rightarrow> 'a \<Rightarrow> tcb \<Rightarrow> bool" where
   "direct_reply subjects aag tcb_owner tcb \<equiv>
      (awaiting_reply (tcb_state tcb)
         \<or> (\<exists>ep. allowed_call_blocked ep (tcb_state tcb)
             \<and> aag_subjects_have_auth_to subjects aag Receive ep))
      \<and> aag_subjects_have_auth_to_label subjects aag Reply tcb_owner"
 
-definition reply_cap_deletion_integrity :: "'a set \<Rightarrow> 'a PAS \<Rightarrow> cap \<Rightarrow> cap \<Rightarrow> bool"
-where
+definition reply_cap_deletion_integrity :: "'a set \<Rightarrow> 'a PAS \<Rightarrow> cap \<Rightarrow> cap \<Rightarrow> bool" where
   "reply_cap_deletion_integrity subjects aag cap cap' \<equiv>
-   (cap = cap') \<or> (\<exists> caller R. cap = ReplyCap caller False R \<and>
-                               cap' = NullCap \<and>
-                               pasObjectAbs aag caller \<in> subjects)"
+   (cap = cap') \<or> (\<exists>caller R. cap = ReplyCap caller False R \<and> cap' = NullCap \<and>
+                              pasObjectAbs aag caller \<in> subjects)"
 
-lemmas reply_cap_deletion_integrityI1 =
-       reply_cap_deletion_integrity_def[THEN meta_eq_to_obj_eq,THEN iffD2,OF disjI1]
-lemmas reply_cap_deletion_integrityI2 =
-       reply_cap_deletion_integrity_def[THEN meta_eq_to_obj_eq,THEN iffD2, OF disjI2, OF exI,
-                                        OF exI, OF conjI [OF _ conjI], rule_format]
-lemmas reply_cap_deletion_integrity_intros =
-       reply_cap_deletion_integrityI1 reply_cap_deletion_integrityI2
-
-lemma reply_cap_deletion_integrityE:
-  assumes hyp:"reply_cap_deletion_integrity subjects aag cap cap'"
-  obtains "cap = cap'" | caller R where "cap = ReplyCap caller False R"
-  and "cap' = NullCap" and "pasObjectAbs aag caller \<in> subjects"
-  using hyp reply_cap_deletion_integrity_def by blast
-
-lemma reply_cap_deletion_integrity_refl[simp]:
-  "reply_cap_deletion_integrity subjects aag cap cap"
-  by (rule reply_cap_deletion_integrityI1) simp
-
-
-(* WARNING if some one want to add a cap to is_transferable, it must appear here *)
-definition cnode_integrity :: "'a set \<Rightarrow> 'a PAS \<Rightarrow> cnode_contents \<Rightarrow> cnode_contents \<Rightarrow> bool"
-  where
+(* WARNING: if some one want to add a cap to is_transferable, it must appear here *)
+definition cnode_integrity :: "'a set \<Rightarrow> 'a PAS \<Rightarrow> cnode_contents \<Rightarrow> cnode_contents \<Rightarrow> bool" where
   "cnode_integrity subjects aag content content' \<equiv>
-   \<forall> l. content l = content' l \<or> (\<exists> cap cap'. content l = Some cap \<and> content' l = Some cap' \<and>
-                                         reply_cap_deletion_integrity subjects aag cap cap')"
-
-lemmas cnode_integrityI = cnode_integrity_def[THEN meta_eq_to_obj_eq,THEN iffD2,rule_format]
-lemmas cnode_integrityD = cnode_integrity_def[THEN meta_eq_to_obj_eq,THEN iffD1,rule_format]
-lemma cnode_integrityE:
-  assumes hyp:"cnode_integrity subjects aag content content'"
-  obtains "content l = content' l" | cap cap' where "content l = Some cap"
-  and "content' l = Some cap'" and "reply_cap_deletion_integrity subjects aag cap cap'"
-  using hyp cnode_integrityD by blast
-
-definition asid_pool_integrity ::
-  "'a set \<Rightarrow> 'a PAS \<Rightarrow> (asid_low_index \<rightharpoonup> obj_ref) \<Rightarrow> (asid_low_index \<rightharpoonup> obj_ref) \<Rightarrow> bool"
-  where
-  "asid_pool_integrity subjects aag pool pool' \<equiv>
-   \<forall>x. pool' x \<noteq> pool x \<longrightarrow> pool' x = None
-       \<and> aag_subjects_have_auth_to subjects aag Control (the (pool x))"
+   \<forall>l. content l = content' l \<or> (\<exists>cap cap'. content l = Some cap \<and> content' l = Some cap' \<and>
+                                            reply_cap_deletion_integrity subjects aag cap cap')"
 
 
 subsubsection \<open>Definition of object integrity\<close>
+
 text \<open>
   The object integrity relation describes which modification to kernel objects are allowed by the
   policy aag when the system is controlled by subjects.
@@ -1074,223 +394,129 @@ text \<open>
 
   Creation and destruction or retyping of kernel objects are not allowed unless l \<in> subjects
 \<close>
+
 (* FIXME it would be nice if there was an arch_tcb_context_update with all the required lemmas*)
-inductive integrity_obj_atomic for aag activate subjects l ko ko'
-  where
+inductive integrity_obj_atomic for aag activate subjects l ko ko' where
   (* l can modify any object it owns *)
   troa_lrefl:
-    "\<lbrakk>l \<in> subjects \<rbrakk> \<Longrightarrow> integrity_obj_atomic aag activate subjects l ko ko'"
-  (* l can modify an Notification object state if it has rights to interact with it *)
+    "l \<in> subjects \<Longrightarrow> integrity_obj_atomic aag activate subjects l ko ko'"
+  (* l can modify a Notification object state if it has rights to interact with it *)
 | troa_ntfn:
-    "\<lbrakk>ko = Some (Notification ntfn); ko' = Some (Notification ntfn');
-      auth \<in> {Receive, Notify, Reset}; s \<in> subjects;
-      (s, auth, l) \<in> pasPolicy aag\<rbrakk>
-     \<Longrightarrow> integrity_obj_atomic aag activate subjects l ko ko'"
+    "\<lbrakk> ko = Some (Notification ntfn); ko' = Some (Notification ntfn');
+       auth \<in> {Receive, Notify, Reset}; s \<in> subjects; (s, auth, l) \<in> pasPolicy aag \<rbrakk>
+       \<Longrightarrow> integrity_obj_atomic aag activate subjects l ko ko'"
   (* l can modify an Endpoint object state if it has rights to interact with it *)
 | troa_ep:
     "\<lbrakk> ko = Some (Endpoint ep); ko' = Some (Endpoint ep');
-      auth \<in> {Receive, SyncSend, Reset}; s \<in> subjects;
-      (s, auth, l) \<in> pasPolicy aag\<rbrakk>
-     \<Longrightarrow> integrity_obj_atomic aag activate subjects l ko ko'"
+       auth \<in> {Receive, SyncSend, Reset}; s \<in> subjects; (s, auth, l) \<in> pasPolicy aag \<rbrakk>
+       \<Longrightarrow> integrity_obj_atomic aag activate subjects l ko ko'"
   (* If a tcb is waiting on receiving on an Endpoint but could be bound to a notification ntfn.
      Then if we can Notify ntfn, we could modify the endpoint *)
 | troa_ep_unblock:
-    "\<lbrakk>ko = Some (Endpoint ep); ko' = Some (Endpoint ep');
-      (tcb, Receive, pasObjectAbs aag ntfn) \<in> pasPolicy aag;
-      (tcb, Receive, l) \<in> pasPolicy aag;
-      aag_subjects_have_auth_to subjects aag Notify ntfn\<rbrakk>
-     \<Longrightarrow> integrity_obj_atomic aag activate subjects l ko ko'"
+    "\<lbrakk> ko = Some (Endpoint ep); ko' = Some (Endpoint ep');
+       (tcb, Receive, pasObjectAbs aag ntfn) \<in> pasPolicy aag;
+       (tcb, Receive, l) \<in> pasPolicy aag;
+       aag_subjects_have_auth_to subjects aag Notify ntfn \<rbrakk>
+       \<Longrightarrow> integrity_obj_atomic aag activate subjects l ko ko'"
   (* If the subjects can send to an Endpoint or its bound notification, they can also
      modify any thread that is waiting on it *)
 | troa_tcb_send:
-    "\<lbrakk>ko = Some (TCB tcb); ko' = Some (TCB tcb');
-      tcb' = tcb \<lparr>tcb_arch := arch_tcb_context_set ctxt' (tcb_arch tcb), tcb_state := Running\<rparr>;
-      direct_send subjects aag ep tcb
-       \<or> indirect_send subjects aag (the (tcb_bound_notification tcb)) ep tcb\<rbrakk>
-     \<Longrightarrow> integrity_obj_atomic aag activate subjects l ko ko'"
+    "\<lbrakk> ko = Some (TCB tcb); ko' = Some (TCB tcb');
+       tcb' = tcb \<lparr>tcb_arch := arch_tcb_context_set ctxt' (tcb_arch tcb), tcb_state := Running\<rparr>;
+       direct_send subjects aag ep tcb
+       \<or> indirect_send subjects aag (the (tcb_bound_notification tcb)) ep tcb \<rbrakk>
+       \<Longrightarrow> integrity_obj_atomic aag activate subjects l ko ko'"
   (* If a tcb is waiting on an Endpoint that the subjects can Call, they are allowed
      to do that call, and insert a ReplyCap back towards a subject*)
 | troa_tcb_call:
-    "\<lbrakk>ko = Some (TCB tcb); ko' = Some (TCB tcb');
-      tcb' = tcb \<lparr>tcb_arch := arch_tcb_context_set ctxt' (tcb_arch tcb), tcb_state := Running,
-                  tcb_caller := ReplyCap caller False R\<rparr>;
-      pasObjectAbs aag caller \<in> subjects;
-      direct_call subjects aag ep (tcb_state tcb)\<rbrakk>
-     \<Longrightarrow> integrity_obj_atomic aag activate subjects l ko ko'"
+    "\<lbrakk> ko = Some (TCB tcb); ko' = Some (TCB tcb');
+       tcb' = tcb \<lparr>tcb_arch := arch_tcb_context_set ctxt' (tcb_arch tcb), tcb_state := Running,
+                   tcb_caller := ReplyCap caller False R\<rparr>;
+       pasObjectAbs aag caller \<in> subjects;
+       direct_call subjects aag ep (tcb_state tcb) \<rbrakk>
+       \<Longrightarrow> integrity_obj_atomic aag activate subjects l ko ko'"
   (* Subjects can reply to a tcb waiting for a Reply, if they have authority to do that Reply
      In case of a fault Reply, the new state of the thread can be Restart or Inactive depending on
      the fault handler*)
 | troa_tcb_reply:
-    "\<lbrakk>ko = Some (TCB tcb); ko' = Some (TCB tcb');
-      tcb' = tcb \<lparr>tcb_arch := arch_tcb_context_set ctxt' (tcb_arch tcb),
-                  tcb_state := new_st, tcb_fault := None\<rparr>;
-      new_st = Running \<or> (tcb_fault tcb \<noteq> None \<and> (new_st = Restart \<or> new_st = Inactive));
-      awaiting_reply (tcb_state tcb);
-      aag_subjects_have_auth_to_label subjects aag Reply l\<rbrakk>
-     \<Longrightarrow> integrity_obj_atomic aag activate subjects l ko ko'"
+    "\<lbrakk> ko = Some (TCB tcb); ko' = Some (TCB tcb');
+       tcb' = tcb \<lparr>tcb_arch := arch_tcb_context_set ctxt' (tcb_arch tcb),
+                   tcb_state := new_st, tcb_fault := None\<rparr>;
+       new_st = Running \<or> (tcb_fault tcb \<noteq> None \<and> (new_st = Restart \<or> new_st = Inactive));
+       awaiting_reply (tcb_state tcb); aag_subjects_have_auth_to_label subjects aag Reply l \<rbrakk>
+       \<Longrightarrow> integrity_obj_atomic aag activate subjects l ko ko'"
   (* Subjects can receive a message from an Endpoint. The sender state will then be set to
      Running if it is a normal send and to Inactive or BlockedOnReply if it is a call.
      TODO split that rule *)
 | troa_tcb_receive:
-    "\<lbrakk>ko = Some (TCB tcb); ko' = Some (TCB tcb');
-      tcb' = tcb \<lparr>tcb_state := new_st\<rparr>;
-      new_st = Running
+    "\<lbrakk> ko = Some (TCB tcb); ko' = Some (TCB tcb');
+       tcb' = tcb \<lparr>tcb_state := new_st\<rparr>;
+       new_st = Running
        \<or> (inactive new_st \<and> call_blocked ep (tcb_state tcb))
        \<or> (awaiting_reply new_st \<and> allowed_call_blocked ep (tcb_state tcb));
-      send_blocked_on ep (tcb_state tcb);
-      aag_subjects_have_auth_to subjects aag Receive ep \<rbrakk>
-     \<Longrightarrow> integrity_obj_atomic aag activate subjects l ko ko'"
+       send_blocked_on ep (tcb_state tcb);
+       aag_subjects_have_auth_to subjects aag Receive ep \<rbrakk>
+       \<Longrightarrow> integrity_obj_atomic aag activate subjects l ko ko'"
   (* Subjects can Reset an Endpoint/Notification they have Reset authority to, and thus
      all TCBs blocked on it need to be restarted *)
 | troa_tcb_restart:
-    "\<lbrakk>ko = Some (TCB tcb); ko' = Some (TCB tcb');
-      tcb' = tcb\<lparr>tcb_state := Restart\<rparr>;
-      blocked_on ep (tcb_state tcb);
-      aag_subjects_have_auth_to subjects aag Reset ep\<rbrakk>
-    \<Longrightarrow> integrity_obj_atomic aag activate subjects l ko ko'"
+    "\<lbrakk> ko = Some (TCB tcb); ko' = Some (TCB tcb');
+       tcb' = tcb\<lparr>tcb_state := Restart\<rparr>;
+       blocked_on ep (tcb_state tcb);
+       aag_subjects_have_auth_to subjects aag Reset ep \<rbrakk>
+       \<Longrightarrow> integrity_obj_atomic aag activate subjects l ko ko'"
   (* Subjects can Reset a bound Notification which then need to be unbound*)
 | troa_tcb_unbind:
-    "\<lbrakk>ko = Some (TCB tcb); ko' = Some (TCB tcb');
-      tcb' = tcb\<lparr>tcb_bound_notification := None\<rparr>;
-      aag_subjects_have_auth_to subjects aag Reset (the (tcb_bound_notification tcb))\<rbrakk>
-    \<Longrightarrow> integrity_obj_atomic aag activate subjects l ko ko'"
+    "\<lbrakk> ko = Some (TCB tcb); ko' = Some (TCB tcb');
+       tcb' = tcb\<lparr>tcb_bound_notification := None\<rparr>;
+       aag_subjects_have_auth_to subjects aag Reset (the (tcb_bound_notification tcb)) \<rbrakk>
+       \<Longrightarrow> integrity_obj_atomic aag activate subjects l ko ko'"
   (* Allow subjects to delete their reply caps in other subjects' threads.
    * Note that we need to account for the reply cap being in tcb_ctable,
    * because recursive deletion of the root CNode may temporarily place any
    * contained cap (in particular, a copied reply cap) in that location. *)
 | troa_tcb_empty_ctable:
-    "\<lbrakk>ko = Some (TCB tcb); ko' = Some (TCB tcb');
-      tcb' = tcb\<lparr>tcb_ctable := cap'\<rparr>;
-      reply_cap_deletion_integrity subjects aag (tcb_ctable tcb) cap'\<rbrakk>
-    \<Longrightarrow> integrity_obj_atomic aag activate subjects l ko ko'"
+    "\<lbrakk> ko = Some (TCB tcb); ko' = Some (TCB tcb');
+       tcb' = tcb\<lparr>tcb_ctable := cap'\<rparr>;
+       reply_cap_deletion_integrity subjects aag (tcb_ctable tcb) cap' \<rbrakk>
+       \<Longrightarrow> integrity_obj_atomic aag activate subjects l ko ko'"
 | troa_tcb_empty_caller:
-    "\<lbrakk>ko = Some (TCB tcb); ko' = Some (TCB tcb');
-      tcb' = tcb\<lparr>tcb_caller := cap'\<rparr>;
-      reply_cap_deletion_integrity subjects aag (tcb_caller tcb) cap'\<rbrakk>
-    \<Longrightarrow> integrity_obj_atomic aag activate subjects l ko ko'"
+    "\<lbrakk> ko = Some (TCB tcb); ko' = Some (TCB tcb');
+       tcb' = tcb\<lparr>tcb_caller := cap'\<rparr>;
+       reply_cap_deletion_integrity subjects aag (tcb_caller tcb) cap' \<rbrakk>
+       \<Longrightarrow> integrity_obj_atomic aag activate subjects l ko ko'"
   (* If the activate flag is on, any thread in Restart state can be restarted *)
 | troa_tcb_activate:
-    "\<lbrakk>ko = Some (TCB tcb); ko' = Some (TCB tcb');
-      tcb' = tcb\<lparr>tcb_arch := arch_tcb_context_set
-                        ((arch_tcb_context_get (tcb_arch tcb))(NextIP :=
-                                          (arch_tcb_context_get (tcb_arch tcb)) FaultIP)
-                        ) (tcb_arch tcb),
-                   tcb_state := Running\<rparr>;
-      tcb_state tcb = Restart;
-      activate\<rbrakk> \<comment> \<open>Anyone can do this\<close>
-     \<Longrightarrow> integrity_obj_atomic aag activate subjects l ko ko'"
-  (* Subjects can clear ASIDs that they control *)
-| troa_asidpool_clear:
-    "\<lbrakk>ko = Some (ArchObj (ASIDPool pool)); ko' = Some (ArchObj (ASIDPool pool'));
-      asid_pool_integrity subjects aag pool pool' \<rbrakk>
-    \<Longrightarrow> integrity_obj_atomic aag activate subjects l ko ko'"
+    "\<lbrakk> ko = Some (TCB tcb); ko' = Some (TCB tcb');
+       tcb' = tcb\<lparr>tcb_arch := arch_IP_update (tcb_arch tcb),
+                  tcb_state := Running\<rparr>;
+       tcb_state tcb = Restart; activate \<rbrakk> \<comment> \<open>Anyone can do this\<close>
+       \<Longrightarrow> integrity_obj_atomic aag activate subjects l ko ko'"
   (* If there is a deletable_cap in a CNode, it must be allowed to be deleted *)
 | troa_cnode:
-      "\<lbrakk>ko = Some (CNode n content); ko' = Some (CNode n content');
+      "\<lbrakk> ko = Some (CNode n content); ko' = Some (CNode n content');
          cnode_integrity subjects aag content content' \<rbrakk>
-       \<Longrightarrow> integrity_obj_atomic aag activate subjects l ko ko'"
+         \<Longrightarrow> integrity_obj_atomic aag activate subjects l ko ko'"
+  (* Arch-specific rules *)
+| troa_arch:
+      "\<lbrakk> ko = Some (ArchObj ao); ko' = Some (ArchObj ao');
+         arch_integrity_obj_atomic aag subjects l ao ao' \<rbrakk>
+         \<Longrightarrow> integrity_obj_atomic aag activate subjects l ko ko'"
 
-definition integrity_obj
-  where
+definition integrity_obj where
   "integrity_obj aag activate subjects l \<equiv> (integrity_obj_atomic aag activate subjects l)\<^sup>*\<^sup>*"
 
-subsubsection \<open>Introduction rules for object integrity\<close>
-
-lemma troa_tro:
-  "integrity_obj_atomic aag activate subjects l ko ko'
-    \<Longrightarrow> integrity_obj aag activate subjects l ko ko'"
-  unfolding integrity_obj_def by (rule r_into_rtranclp)
-
-lemmas tro_lrefl = troa_lrefl[THEN troa_tro]
-lemma tro_orefl:
-  "\<lbrakk> ko = ko' \<rbrakk> \<Longrightarrow> integrity_obj aag activate subjects l' ko ko'"
-  unfolding integrity_obj_def by simp
-lemmas tro_ntfn = troa_ntfn[THEN troa_tro]
-lemmas tro_ep = troa_ep[THEN troa_tro]
-lemmas tro_ep_unblock = troa_ep_unblock[THEN troa_tro]
-lemmas tro_tcb_send = troa_tcb_send[THEN troa_tro]
-lemmas tro_tcb_call = troa_tcb_call[THEN troa_tro]
-lemmas tro_tcb_reply = troa_tcb_reply[THEN troa_tro]
-lemmas tro_tcb_receive = troa_tcb_receive[THEN troa_tro]
-lemmas tro_tcb_restart = troa_tcb_restart[THEN troa_tro]
-lemmas tro_tcb_unbind = troa_tcb_unbind[THEN troa_tro]
-lemmas tro_tcb_empty_ctable = troa_tcb_empty_ctable[THEN troa_tro]
-lemmas tro_tcb_empty_caller = troa_tcb_empty_caller[THEN troa_tro]
-lemmas tro_tcb_activate = troa_tcb_activate[THEN troa_tro]
-lemmas tro_asidpool_clear = troa_asidpool_clear[THEN troa_tro]
-lemmas tro_cnode = troa_cnode[THEN troa_tro]
-
-lemmas tro_intros = tro_lrefl tro_orefl tro_ntfn tro_ep tro_ep_unblock tro_tcb_send tro_tcb_call
-           tro_tcb_reply tro_tcb_receive tro_tcb_restart tro_tcb_unbind tro_tcb_empty_ctable
-           tro_tcb_empty_caller tro_tcb_activate tro_asidpool_clear tro_cnode
-
-lemma tro_tcb_unbind':
-  "\<lbrakk> ko  = Some (TCB tcb); ko' = Some (TCB tcb');
-     tcb' = tcb\<lparr>tcb_bound_notification := ntfn'\<rparr>;
-     tcb_bound_notification_reset_integrity (tcb_bound_notification tcb) ntfn' subjects aag\<rbrakk>
-                 \<Longrightarrow> integrity_obj aag activate subjects l' ko ko'"
-  apply (clarsimp simp:tcb_bound_notification_reset_integrity_def)
-  apply (elim disjE)
-   apply (rule tro_orefl;fastforce)
-  apply (rule tro_tcb_unbind;fastforce)
-  done
-
-lemmas rtranclp_transp[intro!] = transp_rtranclp
-
-lemma tro_transp[intro!]:
-  "transp (integrity_obj aag activate es subjects)"
-  unfolding integrity_obj_def by simp
-
-lemmas tro_trans_spec = tro_transp[THEN transpD]
-
-lemma tro_tcb_generic':
-  "\<lbrakk>ko = Some (TCB tcb); ko' = Some (TCB tcb');
-    tcb' = tcb \<lparr>tcb_bound_notification := ntfn', tcb_caller := cap', tcb_ctable := ccap'\<rparr>;
-    tcb_bound_notification_reset_integrity (tcb_bound_notification tcb) ntfn' subjects aag ;
-    reply_cap_deletion_integrity subjects aag (tcb_caller tcb) cap';
-    reply_cap_deletion_integrity subjects aag (tcb_ctable tcb) ccap' \<rbrakk>
-   \<Longrightarrow> integrity_obj aag activate subjects l' ko ko'"
-  apply clarsimp
-  apply (rule tro_trans_spec)
-   apply (rule tro_tcb_empty_caller[OF refl refl refl];simp)
-  apply (rule tro_trans_spec)
-   apply (rule tro_tcb_empty_ctable[OF refl refl refl];simp)
-  apply (rule tro_trans_spec)
-   apply (rule tro_tcb_unbind'[OF refl refl refl];simp)
-  apply (fastforce intro!: tro_orefl tcb.equality)
-  done
-
-lemma tro_tcb_reply':
-  "\<lbrakk>ko = Some (TCB tcb); ko' = Some (TCB tcb');
-    tcb' = tcb \<lparr>tcb_arch := arch_tcb_context_set ctxt' (tcb_arch tcb),
-                        tcb_state := new_st, tcb_fault := None\<rparr>;
-    new_st = Running \<or> (tcb_fault tcb \<noteq> None \<and> (new_st = Restart \<or> new_st = Inactive));
-    direct_reply subjects aag l' tcb \<rbrakk>
-   \<Longrightarrow> integrity_obj aag activate subjects l' ko ko'"
-  apply (clarsimp simp:direct_reply_def simp del:not_None_eq)
-  apply (erule disjE, (rule tro_tcb_reply[OF refl refl], force; force)) (* Warning: schematics *)
-  apply (clarsimp simp del:not_None_eq)
-  apply (rule tro_trans_spec)
-   apply (frule allowed_call_blocked_def[THEN meta_eq_to_obj_eq,THEN iffD1],clarsimp)
-   apply (rule tro_tcb_receive[OF refl refl refl, where new_st=BlockedOnReply];force)
-  apply (rule tro_trans_spec)
-   apply (rule tro_tcb_reply[OF refl refl refl, where new_st=new_st];force)
-  by (fastforce intro!: tro_orefl tcb.equality)
-
-abbreviation integrity_obj_state
-where
+abbreviation integrity_obj_state where
   "integrity_obj_state aag activate subjects s s' \<equiv>
-       (\<forall>x. integrity_obj aag activate subjects (pasObjectAbs aag x) (kheap s x) (kheap s' x))"
-
+     (\<forall>x. integrity_obj aag activate subjects (pasObjectAbs aag x) (kheap s x) (kheap s' x))"
 
 
 subsubsection \<open>Alternative tagged formulation of object integrity\<close>
 
-datatype Tro_rules = LRefl | ORefl | RNtfn | REp | EpUnblock | TCBSend | TCBCall |
-  TCBReply | TCBReceive | TCBRestart | TCBGeneric | RASID | TCBActivate | RCNode
+datatype Tro_rules = LRefl | ORefl | RNtfn | REp | EpUnblock | TCBSend | TCBCall | TCBReply
+                           | TCBReceive | TCBRestart | TCBGeneric | RArch | TCBActivate | RCNode
 
-definition tro_tag :: "Tro_rules \<Rightarrow> bool"
-where
+definition tro_tag :: "Tro_rules \<Rightarrow> bool" where
   "tro_tag t \<equiv> True"
 
 (* do not put that one in the simpset unless you know what you are doing *)
@@ -1298,8 +524,7 @@ lemma tro_tagI[intro!]:
   "tro_tag t"
   unfolding tro_tag_def ..
 
-definition tro_tag' :: "Tro_rules \<Rightarrow> bool"
-where
+definition tro_tag' :: "Tro_rules \<Rightarrow> bool" where
   "tro_tag' t \<equiv> True"
 
 (* do not put that one in the simpset unless you know what you are doing *)
@@ -1329,145 +554,111 @@ text \<open>
       implying @{const integrity_obj}. It is not quite true, and we
       do not need it in any case.
 \<close>
-inductive integrity_obj_alt for aag activate subjects l' ko ko'
-where
+
+inductive integrity_obj_alt for aag activate subjects l' ko ko' where
   tro_alt_lrefl:
-      "\<lbrakk> tro_tag LRefl ; l' \<in> subjects  \<rbrakk> \<Longrightarrow> integrity_obj_alt aag activate subjects l' ko ko'"
+    "\<lbrakk> tro_tag LRefl; l' \<in> subjects \<rbrakk> \<Longrightarrow> integrity_obj_alt aag activate subjects l' ko ko'"
 | tro_alt_orefl:
-      "\<lbrakk> tro_tag ORefl; ko = ko' \<rbrakk> \<Longrightarrow> integrity_obj_alt aag activate subjects l' ko ko'"
+    "\<lbrakk> tro_tag ORefl; ko = ko' \<rbrakk> \<Longrightarrow> integrity_obj_alt aag activate subjects l' ko ko'"
 | tro_alt_ntfn:
-      "\<lbrakk>tro_tag RNtfn; ko = Some (Notification ntfn); ko' = Some (Notification ntfn');
-        auth \<in> {Receive, Notify, Reset};
-        \<exists>s \<in> subjects. (s, auth, l') \<in> pasPolicy aag \<rbrakk>
+    "\<lbrakk> tro_tag RNtfn; ko = Some (Notification ntfn); ko' = Some (Notification ntfn');
+       auth \<in> {Receive, Notify, Reset};
+       \<exists>s \<in> subjects. (s, auth, l') \<in> pasPolicy aag \<rbrakk>
        \<Longrightarrow> integrity_obj_alt aag activate subjects l' ko ko'"
 | tro_alt_ep:
-      "\<lbrakk>tro_tag REp; ko = Some (Endpoint ep); ko' = Some (Endpoint ep');
-             auth \<in> {Receive, SyncSend, Reset};
-             (\<exists>s \<in> subjects. (s, auth, l') \<in> pasPolicy aag) \<rbrakk>
-           \<Longrightarrow> integrity_obj_alt aag activate subjects l' ko ko'"
-| tro_alt_ep_unblock:
-      "\<lbrakk>tro_tag EpUnblock; ko = Some (Endpoint ep); ko' = Some (Endpoint ep');
-        \<exists>tcb ntfn. (tcb, Receive, pasObjectAbs aag ntfn) \<in> pasPolicy aag \<and>
-                   (tcb, Receive, l') \<in> pasPolicy aag \<and>
-        aag_subjects_have_auth_to subjects aag Notify ntfn \<rbrakk>
+    "\<lbrakk> tro_tag REp; ko = Some (Endpoint ep); ko' = Some (Endpoint ep');
+       auth \<in> {Receive, SyncSend, Reset}; (\<exists>s \<in> subjects. (s, auth, l') \<in> pasPolicy aag) \<rbrakk>
        \<Longrightarrow> integrity_obj_alt aag activate subjects l' ko ko'"
-
+| tro_alt_ep_unblock:
+    "\<lbrakk> tro_tag EpUnblock; ko = Some (Endpoint ep); ko' = Some (Endpoint ep');
+       \<exists>tcb ntfn. (tcb, Receive, pasObjectAbs aag ntfn) \<in> pasPolicy aag \<and>
+                  (tcb, Receive, l') \<in> pasPolicy aag \<and>
+                  aag_subjects_have_auth_to subjects aag Notify ntfn \<rbrakk>
+       \<Longrightarrow> integrity_obj_alt aag activate subjects l' ko ko'"
 | tro_alt_tcb_send:
-      "\<lbrakk>tro_tag TCBSend; ko = Some (TCB tcb); ko' = Some (TCB tcb');
-        \<exists>ctxt'. tcb' = tcb \<lparr>tcb_arch := arch_tcb_context_set ctxt' (tcb_arch tcb),
-                            tcb_state := Running,
-                            tcb_bound_notification := ntfn', tcb_caller := cap',
-                            tcb_ctable := ccap'\<rparr>;
-        tcb_bound_notification_reset_integrity (tcb_bound_notification tcb) ntfn' subjects aag;
-        reply_cap_deletion_integrity subjects aag (tcb_caller tcb) cap';
-        reply_cap_deletion_integrity subjects aag (tcb_ctable tcb) ccap';
-        direct_send subjects aag ep tcb \<or> indirect_send subjects aag (the (tcb_bound_notification tcb)) ep tcb \<rbrakk>
+    "\<lbrakk> tro_tag TCBSend; ko = Some (TCB tcb); ko' = Some (TCB tcb');
+       \<exists>ctxt'. tcb' = tcb \<lparr>tcb_arch := arch_tcb_context_set ctxt' (tcb_arch tcb),
+                           tcb_state := Running, tcb_bound_notification := ntfn',
+                           tcb_caller := cap', tcb_ctable := ccap'\<rparr>;
+       tcb_bound_notification_reset_integrity (tcb_bound_notification tcb) ntfn' subjects aag;
+       reply_cap_deletion_integrity subjects aag (tcb_caller tcb) cap';
+       reply_cap_deletion_integrity subjects aag (tcb_ctable tcb) ccap';
+       direct_send subjects aag ep tcb
+       \<or> indirect_send subjects aag (the (tcb_bound_notification tcb)) ep tcb \<rbrakk>
        \<Longrightarrow> integrity_obj_alt aag activate subjects l' ko ko'"
 | tro_alt_tcb_call:
-      "\<lbrakk>tro_tag TCBCall; ko = Some (TCB tcb); ko' = Some (TCB tcb');
-        \<exists>ctxt'. tcb' = tcb \<lparr>tcb_arch := arch_tcb_context_set ctxt' (tcb_arch tcb),
-                            tcb_state := Running,
-                            tcb_bound_notification := ntfn', tcb_caller := cap',
-                            tcb_ctable := ccap'\<rparr>;
-        pasObjectAbs aag caller \<in> subjects;
-        tcb_bound_notification_reset_integrity (tcb_bound_notification tcb) ntfn' subjects aag;
-        reply_cap_deletion_integrity subjects aag (ReplyCap caller False R) cap';
-        reply_cap_deletion_integrity subjects aag (tcb_ctable tcb) ccap';
-        direct_call subjects aag ep (tcb_state tcb) \<rbrakk>
+    "\<lbrakk> tro_tag TCBCall; ko = Some (TCB tcb); ko' = Some (TCB tcb');
+       \<exists>ctxt'. tcb' = tcb \<lparr>tcb_arch := arch_tcb_context_set ctxt' (tcb_arch tcb),
+                           tcb_state := Running, tcb_bound_notification := ntfn',
+                            tcb_caller := cap', tcb_ctable := ccap'\<rparr>;
+       pasObjectAbs aag caller \<in> subjects;
+       tcb_bound_notification_reset_integrity (tcb_bound_notification tcb) ntfn' subjects aag;
+       reply_cap_deletion_integrity subjects aag (ReplyCap caller False R) cap';
+       reply_cap_deletion_integrity subjects aag (tcb_ctable tcb) ccap';
+       direct_call subjects aag ep (tcb_state tcb) \<rbrakk>
        \<Longrightarrow> integrity_obj_alt aag activate subjects l' ko ko'"
 | tro_alt_tcb_reply:
-      "\<lbrakk>tro_tag TCBReply; ko = Some (TCB tcb); ko' = Some (TCB tcb');
-        \<exists>ctxt'. tcb' = tcb \<lparr>tcb_arch := arch_tcb_context_set ctxt' (tcb_arch tcb),
-                            tcb_state := new_st, tcb_fault := None,
-                            tcb_bound_notification := ntfn', tcb_caller := cap',
-                            tcb_ctable := ccap'\<rparr>;
-        new_st = Running \<or> (tcb_fault tcb \<noteq> None \<and> (new_st = Restart \<or> new_st = Inactive));
-        tcb_bound_notification_reset_integrity (tcb_bound_notification tcb) ntfn' subjects aag;
-        reply_cap_deletion_integrity subjects aag (tcb_caller tcb) cap';
-        reply_cap_deletion_integrity subjects aag (tcb_ctable tcb) ccap';
-        direct_reply subjects aag l' tcb \<rbrakk>
+    "\<lbrakk> tro_tag TCBReply; ko = Some (TCB tcb); ko' = Some (TCB tcb');
+       \<exists>ctxt'. tcb' = tcb \<lparr>tcb_arch := arch_tcb_context_set ctxt' (tcb_arch tcb),
+                           tcb_state := new_st, tcb_fault := None,
+                           tcb_bound_notification := ntfn',
+                           tcb_caller := cap', tcb_ctable := ccap'\<rparr>;
+       new_st = Running \<or> (tcb_fault tcb \<noteq> None \<and> (new_st = Restart \<or> new_st = Inactive));
+       tcb_bound_notification_reset_integrity (tcb_bound_notification tcb) ntfn' subjects aag;
+       reply_cap_deletion_integrity subjects aag (tcb_caller tcb) cap';
+       reply_cap_deletion_integrity subjects aag (tcb_ctable tcb) ccap';
+       direct_reply subjects aag l' tcb \<rbrakk>
        \<Longrightarrow> integrity_obj_alt aag activate subjects l' ko ko'"
 | tro_alt_tcb_receive:
-      "\<lbrakk>tro_tag TCBReceive; ko = Some (TCB tcb); ko' = Some (TCB tcb');
-        tcb' = tcb \<lparr>tcb_state := new_st, tcb_bound_notification := ntfn', tcb_caller := cap',
-                    tcb_ctable := ccap'\<rparr>;
-        new_st = Running \<or> (((new_st = Inactive \<and> call_blocked ep (tcb_state tcb)) \<or> (new_st = BlockedOnReply \<and> (allowed_call_blocked ep (tcb_state tcb)))));
-        tcb_bound_notification_reset_integrity (tcb_bound_notification tcb) ntfn' subjects aag;
-        reply_cap_deletion_integrity subjects aag (tcb_caller tcb) cap';
-        reply_cap_deletion_integrity subjects aag (tcb_ctable tcb) ccap';
-        send_blocked_on ep (tcb_state tcb);
-        aag_subjects_have_auth_to subjects aag Receive ep \<rbrakk>
+    "\<lbrakk> tro_tag TCBReceive; ko = Some (TCB tcb); ko' = Some (TCB tcb');
+       tcb' = tcb \<lparr>tcb_state := new_st, tcb_bound_notification := ntfn',
+                   tcb_caller := cap', tcb_ctable := ccap'\<rparr>;
+       new_st = Running \<or> ((new_st = Inactive \<and> call_blocked ep (tcb_state tcb)) \<or>
+       (new_st = BlockedOnReply \<and> (allowed_call_blocked ep (tcb_state tcb))));
+       tcb_bound_notification_reset_integrity (tcb_bound_notification tcb) ntfn' subjects aag;
+       reply_cap_deletion_integrity subjects aag (tcb_caller tcb) cap';
+       reply_cap_deletion_integrity subjects aag (tcb_ctable tcb) ccap';
+       send_blocked_on ep (tcb_state tcb);
+       aag_subjects_have_auth_to subjects aag Receive ep \<rbrakk>
        \<Longrightarrow> integrity_obj_alt aag activate subjects l' ko ko'"
 | tro_alt_tcb_restart:
-      "\<lbrakk>tro_tag TCBRestart; ko  = Some (TCB tcb); ko' = Some (TCB tcb');
-        tcb' = tcb\<lparr> tcb_arch := arch_tcb_context_set
-                                         (arch_tcb_context_get (tcb_arch tcb')) (tcb_arch tcb),
-                    tcb_state := tcb_state tcb', tcb_bound_notification := ntfn',
-                    tcb_caller := cap',tcb_ctable := ccap'\<rparr>;
-        (tcb_state tcb' = Restart \<and>
-               arch_tcb_context_get (tcb_arch tcb') = arch_tcb_context_get (tcb_arch tcb)) \<or>
-        (tcb_state tcb' = Running \<and>
-        arch_tcb_context_get (tcb_arch tcb')
-             = (arch_tcb_context_get (tcb_arch tcb))
-                   (NextIP := arch_tcb_context_get (tcb_arch tcb) FaultIP));
-        tcb_bound_notification_reset_integrity (tcb_bound_notification tcb) ntfn' subjects aag;
-        reply_cap_deletion_integrity subjects aag (tcb_caller tcb) cap';
-        reply_cap_deletion_integrity subjects aag (tcb_ctable tcb) ccap';
-        blocked_on ep (tcb_state tcb);
-        aag_subjects_have_auth_to subjects aag Reset ep \<rbrakk>
+    "\<lbrakk> tro_tag TCBRestart; ko  = Some (TCB tcb); ko' = Some (TCB tcb');
+       tcb' = tcb\<lparr>tcb_arch := new_arch, tcb_state := tcb_state tcb',
+                  tcb_bound_notification := ntfn', tcb_caller := cap', tcb_ctable := ccap'\<rparr>;
+       (tcb_state tcb' = Restart \<and> new_arch = tcb_arch tcb) \<or>
+       (tcb_state tcb' = Running \<and> new_arch = arch_IP_update (tcb_arch tcb));
+       tcb_bound_notification_reset_integrity (tcb_bound_notification tcb) ntfn' subjects aag;
+       reply_cap_deletion_integrity subjects aag (tcb_caller tcb) cap';
+       reply_cap_deletion_integrity subjects aag (tcb_ctable tcb) ccap';
+       blocked_on ep (tcb_state tcb);
+       aag_subjects_have_auth_to subjects aag Reset ep \<rbrakk>
        \<Longrightarrow> integrity_obj_alt aag activate subjects l' ko ko'"
 | tro_alt_tcb_generic:
-      "\<lbrakk>tro_tag TCBGeneric; ko = Some (TCB tcb); ko' = Some (TCB tcb');
-        tcb' = tcb \<lparr>tcb_bound_notification := ntfn', tcb_caller := cap', tcb_ctable := ccap'\<rparr>;
-        tcb_bound_notification_reset_integrity (tcb_bound_notification tcb) ntfn' subjects aag ;
-        reply_cap_deletion_integrity subjects aag (tcb_caller tcb) cap';
-        reply_cap_deletion_integrity subjects aag (tcb_ctable tcb) ccap' \<rbrakk>
-       \<Longrightarrow> integrity_obj_alt aag activate subjects l' ko ko'"
-| tro_alt_asidpool_clear:
-      "\<lbrakk>tro_tag RASID; ko = Some (ArchObj (ASIDPool pool)); ko' = Some (ArchObj (ASIDPool pool'));
-        asid_pool_integrity subjects aag pool pool'\<rbrakk>
+    "\<lbrakk> tro_tag TCBGeneric; ko = Some (TCB tcb); ko' = Some (TCB tcb');
+       tcb' = tcb \<lparr>tcb_bound_notification := ntfn', tcb_caller := cap', tcb_ctable := ccap'\<rparr>;
+       tcb_bound_notification_reset_integrity (tcb_bound_notification tcb) ntfn' subjects aag ;
+       reply_cap_deletion_integrity subjects aag (tcb_caller tcb) cap';
+       reply_cap_deletion_integrity subjects aag (tcb_ctable tcb) ccap' \<rbrakk>
        \<Longrightarrow> integrity_obj_alt aag activate subjects l' ko ko'"
 | tro_alt_tcb_activate:
-      "\<lbrakk>tro_tag TCBActivate; ko  = Some (TCB tcb); ko' = Some (TCB tcb');
-        tcb' = tcb \<lparr> tcb_arch := arch_tcb_context_set
-                              ((arch_tcb_context_get (tcb_arch tcb))(NextIP :=
-                                           (arch_tcb_context_get (tcb_arch tcb)) FaultIP)
-                               ) (tcb_arch tcb),
-                     tcb_caller := cap', tcb_ctable := ccap',
-                     tcb_state := Running, tcb_bound_notification := ntfn'\<rparr>;
-        tcb_state tcb = Restart;
-        reply_cap_deletion_integrity subjects aag (tcb_caller tcb) cap';
-        reply_cap_deletion_integrity subjects aag (tcb_ctable tcb) ccap';
-        tcb_bound_notification_reset_integrity (tcb_bound_notification tcb) ntfn' subjects aag;
-        activate \<rbrakk> \<comment> \<open>Anyone can do this\<close>
+    "\<lbrakk> tro_tag TCBActivate; ko  = Some (TCB tcb); ko' = Some (TCB tcb');
+       tcb' = tcb \<lparr>tcb_arch := arch_IP_update (tcb_arch tcb),
+                   tcb_caller := cap', tcb_ctable := ccap',
+                   tcb_state := Running, tcb_bound_notification := ntfn'\<rparr>;
+       tcb_state tcb = Restart;
+       reply_cap_deletion_integrity subjects aag (tcb_caller tcb) cap';
+       reply_cap_deletion_integrity subjects aag (tcb_ctable tcb) ccap';
+       tcb_bound_notification_reset_integrity (tcb_bound_notification tcb) ntfn' subjects aag;
+       activate \<rbrakk> \<comment> \<open>Anyone can do this\<close>
        \<Longrightarrow> integrity_obj_alt aag activate subjects l' ko ko'"
 | tro_alt_cnode:
-      "\<lbrakk>tro_tag RCNode; ko  = Some (CNode n content); ko' = Some (CNode n content');
-        cnode_integrity subjects aag content content' \<rbrakk>
+    "\<lbrakk> tro_tag RCNode; ko  = Some (CNode n content); ko' = Some (CNode n content');
+       cnode_integrity subjects aag content content' \<rbrakk>
        \<Longrightarrow> integrity_obj_alt aag activate subjects l' ko ko'"
-
-lemmas disj_cong' = arg_cong2[where f="(\<or>)"]
-
-
-lemma troa_tro_alt[elim!]:
-  "integrity_obj_atomic aag activate subjects l ko ko'
-   \<Longrightarrow> integrity_obj_alt aag activate subjects l ko ko'"
-  apply (erule integrity_obj_atomic.cases)
-
-  text \<open>Single out TCB cases for special handling. We manually simplify
-        the TCB updates in the tro_alt rules using @{thm tcb.equality}.\<close>
-  (* somewhat slow 10s *)
-  apply (find_goal \<open>match premises in "ko = Some (TCB _)" \<Rightarrow> succeed\<close>,
-         ((erule(1) integrity_obj_alt.intros[OF tro_tagI],
-                  (intro exI tcb.equality; solves \<open>simp\<close>));
-          fastforce simp: reply_cap_deletion_integrity_def
-                          tcb_bound_notification_reset_integrity_def
-                          direct_reply_def))+
-
-  text \<open>Remaining cases.\<close>
-  apply (fastforce intro: integrity_obj_alt.intros[OF tro_tagI])+
-  done
-
+| tro_alt_arch:
+    "\<lbrakk> tro_tag RArch; ko = Some (ArchObj ao); ko' = Some (ArchObj ao');
+       arch_integrity_obj_alt aag subjects l' ao ao'\<rbrakk>
+       \<Longrightarrow> integrity_obj_alt aag activate subjects l' ko ko'"
 
 
 subsubsection \<open>ekheap and ready queues\<close>
@@ -1485,81 +676,105 @@ text\<open>
 
 \<close>
 
-definition integrity_ready_queues
-where
+definition integrity_ready_queues where
   "integrity_ready_queues aag subjects queue_labels rq rq' \<equiv>
      pasMayEditReadyQueues aag \<or> (queue_labels \<inter> subjects = {} \<longrightarrow> (\<exists>threads. threads @ rq = rq'))"
 
-lemma integrity_ready_queues_refl[simp]: "integrity_ready_queues aag subjects ptr s s"
-unfolding integrity_ready_queues_def by simp
+inductive integrity_eobj for aag subjects l' eko eko' where
+  tre_lrefl: "l' \<in> subjects \<Longrightarrow> integrity_eobj aag subjects l' eko eko'"
+| tre_orefl: "eko = eko' \<Longrightarrow> integrity_eobj aag subjects l' eko eko'"
 
-inductive integrity_eobj for aag subjects l' eko eko'
-where
-  tre_lrefl: "\<lbrakk> l' \<in> subjects \<rbrakk> \<Longrightarrow> integrity_eobj aag subjects l' eko eko'"
-| tre_orefl: "\<lbrakk> eko = eko' \<rbrakk> \<Longrightarrow> integrity_eobj aag subjects l' eko eko'"
 
-subsubsection \<open>generic stuff : FIXME MOVE\<close>
-
-lemma integrity_obj_activate:
-  "integrity_obj aag False subjects l' ko ko' \<Longrightarrow>
-   integrity_obj aag activate subjects l' ko ko'"
-  unfolding integrity_obj_def
-  apply (erule rtranclp_mono[THEN predicate2D, rotated])
-  apply (rule predicate2I)
-  by (erule integrity_obj_atomic.cases; (intro integrity_obj_atomic.intros; assumption | simp))
-
-abbreviation object_integrity
-where
+abbreviation object_integrity where
   "object_integrity aag \<equiv> integrity_obj (aag :: 'a PAS) (pasMayActivate aag) {pasSubject aag}"
 
 
-subsection \<open>auth_ipc_buffer\<close>
+subsection \<open>How the CDT can change\<close>
 
-definition auth_ipc_buffers :: "'z::state_ext state \<Rightarrow> obj_ref \<Rightarrow> obj_ref set"
-where
-  "auth_ipc_buffers s \<equiv>
-     \<lambda>p. case (get_tcb p s) of
-         None \<Rightarrow> {}
-       | Some tcb \<Rightarrow>
-           (case tcb_ipcframe tcb of
-              cap.ArchObjectCap (arch_cap.PageCap False p' R vms _) \<Rightarrow>
-                if AllowWrite \<in> R
-                then (ptr_range (p' + (tcb_ipc_buffer tcb && mask (pageBitsForSize vms)))
-                                msg_align_bits)
-                else {}
-            | _ \<Rightarrow> {})"
+text \<open>
+  The CDT and CDT_list integrity relations describe which modification to the CDT (@{term cdt})
+  , @{term is_original_cap} and @{term cdt_list})
+  are allowed by the policy aag when the system is controlled by subjects.
 
-(* MOVE *)
-lemma caps_of_state_tcb':
-  "\<lbrakk> get_tcb p s = Some tcb; option_map fst (tcb_cap_cases idx) = Some getF \<rbrakk> \<Longrightarrow> caps_of_state s (p, idx) = Some (getF tcb)"
-  apply (drule get_tcb_SomeD)
-  apply clarsimp
-  apply (drule (1) cte_wp_at_tcbI [where t = "(p, idx)" and P = "(=) (getF tcb)", simplified])
-  apply simp
-  apply (clarsimp simp: cte_wp_at_caps_of_state)
-  done
+  A modification to the CDT at a specific slot can happen for different reasons :
+  \begin{itemize}
+  \item we own directly or indirectly the slot. The "indirectly" means that
+        if an ancestor of a slot is owned by the subject, the slot is indirectly own by the subject
+  \item we are allowed explicitly to take ownership of the slot, for now this only happens when
+        we call someone: we are allowed to put a reply cap in its caller slot (slot number 3)
+\<close>
 
-(* MOVE *)
-lemma caps_of_state_tcb_cap_cases:
-  "\<lbrakk> get_tcb p s = Some tcb; idx \<in> dom tcb_cap_cases \<rbrakk> \<Longrightarrow> caps_of_state s (p, idx) = Some ((the (option_map fst (tcb_cap_cases idx))) tcb)"
-  apply (clarsimp simp: dom_def)
-  apply (erule caps_of_state_tcb')
-  apply simp
-  done
+(* FIXME MOVE *)
+notation parent_of_rtrancl ("_ \<Turnstile> _ \<rightarrow>* _" [60,0,60] 60)
 
-lemma auth_ipc_buffers_member_def:
-  "x \<in> auth_ipc_buffers s p =
-      (\<exists>tcb p' R vms xx. get_tcb p s = Some tcb
-                       \<and> tcb_ipcframe tcb = (cap.ArchObjectCap (arch_cap.PageCap False p' R vms xx))
-                       \<and> caps_of_state s (p, tcb_cnode_index 4) =
-                                    Some (cap.ArchObjectCap (arch_cap.PageCap False p' R vms xx))
-                       \<and> AllowWrite \<in> R
-                       \<and> x \<in> ptr_range (p' + (tcb_ipc_buffer tcb && mask (pageBitsForSize vms)))
-                                       msg_align_bits)"
-  unfolding auth_ipc_buffers_def
-  by (clarsimp simp: caps_of_state_tcb' split: option.splits cap.splits arch_cap.splits bool.splits)
+inductive cdt_direct_change_allowed for aag subjects tcbsts ptr where
+  cdca_owned:
+    "pasObjectAbs aag (fst ptr) \<in> subjects \<Longrightarrow> cdt_direct_change_allowed aag subjects tcbsts ptr"
+| cdca_reply:
+    "\<lbrakk> tcbsts (fst ptr) = Some tcbst; direct_call subjects aag ep tcbst; (snd ptr) = tcb_cnode_index 3 \<rbrakk>
+       \<Longrightarrow> cdt_direct_change_allowed aag subjects tcbsts ptr"
 
-subsection \<open>How User and device memory can change\<close>
+(* for the moment the only caps that can be affected by that indirect control are reply caps *)
+definition cdt_change_allowed where
+  "cdt_change_allowed aag subjects m tcbsts ptr \<equiv>
+     \<exists>pptr. m \<Turnstile> pptr \<rightarrow>* ptr \<and> cdt_direct_change_allowed aag subjects tcbsts pptr"
+
+(* FIXME get a coherent naming scheme *)
+abbreviation cdt_change_allowed' where
+  "cdt_change_allowed' aag ptr s \<equiv>
+     cdt_change_allowed aag {pasSubject aag} (cdt s) (tcb_states_of_state s) ptr"
+
+text\<open>
+  ptr is the slot we currently looking at
+  s is the initial state (v should be coherent with s)
+  v = (initial parent of ptr, initial "originality" of ptr)
+  v' = (final parent of ptr, final "originality" of ptr)
+\<close>
+definition integrity_cdt ::
+   "'a PAS \<Rightarrow> 'a set \<Rightarrow> cdt \<Rightarrow> (obj_ref \<Rightarrow> thread_state option) \<Rightarrow> cslot_ptr
+           \<Rightarrow> (cslot_ptr option \<times> bool) \<Rightarrow> (cslot_ptr option \<times> bool) \<Rightarrow> bool" where
+  "integrity_cdt aag subjects m tcbsts ptr v v' \<equiv>
+     v = v' \<or> cdt_change_allowed aag subjects m tcbsts ptr"
+
+abbreviation integrity_cdt_state where
+  "integrity_cdt_state aag subjects s s' \<equiv>
+     (\<forall>x. integrity_cdt aag subjects (cdt s) (tcb_states_of_state s) x
+                        (cdt s x,is_original_cap s x) (cdt s' x, is_original_cap s' x))"
+
+abbreviation "cdt_integrity aag \<equiv> integrity_cdt (aag :: 'a PAS) {pasSubject aag} "
+
+abbreviation cdt_integrity_state where
+  "cdt_integrity_state aag s s' \<equiv>
+     (\<forall>x. integrity_cdt (aag :: 'a PAS) {pasSubject aag} (cdt s) (tcb_states_of_state s) x
+                        (cdt s x,is_original_cap s x) (cdt s' x, is_original_cap s' x))"
+
+text\<open>
+  m is the cdt of the initial state
+  tcbsts are tcb_states_of_state of the initial state
+  ptr is the slot we currently looking at
+  l and l' are the initial and final list of children of ptr
+\<close>
+definition integrity_cdt_list ::
+   "'a PAS \<Rightarrow> 'a set \<Rightarrow> cdt \<Rightarrow> (obj_ref \<Rightarrow> thread_state option)
+           \<Rightarrow> cslot_ptr \<Rightarrow> (cslot_ptr list) \<Rightarrow> (cslot_ptr list) \<Rightarrow> bool" where
+  "integrity_cdt_list aag subjects m tcbsts ptr l l' \<equiv>
+     filtered_eq (cdt_change_allowed aag subjects m tcbsts) l l'
+   \<or> cdt_change_allowed aag subjects m tcbsts ptr"
+
+abbreviation integrity_cdt_list_state where
+  "integrity_cdt_list_state aag subjects s s' \<equiv>
+     (\<forall>x. integrity_cdt_list aag subjects (cdt s) (tcb_states_of_state s)
+                             x (cdt_list s x) (cdt_list s' x))"
+
+abbreviation "cdt_list_integrity aag \<equiv> integrity_cdt_list (aag :: 'a PAS) {pasSubject aag}"
+
+abbreviation cdt_list_integrity_state where
+  "cdt_list_integrity_state aag  s s' \<equiv>
+     (\<forall>x. integrity_cdt_list (aag :: 'a PAS) {pasSubject aag} (cdt s) (tcb_states_of_state s) x
+                             (cdt_list s x) (cdt_list s' x))"
+
+
+subsection \<open>How user and device memory can change\<close>
 
 text \<open>
   The memory integrity relation describes which modification to user memory are allowed by the
@@ -1584,217 +799,39 @@ text \<open>
   Inductive for now, we should add something about user memory/transitions.
 \<close>
 
-inductive integrity_mem for aag subjects p ts ts' ipcbufs globals w w'
-where
-  trm_lrefl: "\<lbrakk> pasObjectAbs aag p \<in> subjects \<rbrakk>
-     \<Longrightarrow> integrity_mem aag subjects p ts ts' ipcbufs globals w w'" (* implied by wf and write *)
-  | trm_orefl: "\<lbrakk> w = w' \<rbrakk> \<Longrightarrow> integrity_mem aag subjects p ts ts' ipcbufs globals w w'"
-  | trm_write: "\<lbrakk> aag_subjects_have_auth_to subjects aag Write p \<rbrakk> \<Longrightarrow> integrity_mem aag subjects p ts ts' ipcbufs globals w w'"
-  | trm_globals: "\<lbrakk> p \<in> globals \<rbrakk> \<Longrightarrow> integrity_mem aag subjects p ts ts' ipcbufs globals w w'"
-  | trm_ipc: "\<lbrakk> case_option False can_receive_ipc (ts p'); ts' p' = Some Structures_A.Running;
-                p \<in> ipcbufs p'; pasObjectAbs aag p' \<notin> subjects
-        \<rbrakk> \<Longrightarrow> integrity_mem aag subjects p ts ts' ipcbufs globals w w'"
+inductive integrity_mem for aag subjects p ts ts' ipcbufs globals w w' where
+  trm_lrefl:
+    "pasObjectAbs aag p \<in> subjects \<Longrightarrow> integrity_mem aag subjects p ts ts' ipcbufs globals w w'"
+| trm_orefl:
+    "w = w' \<Longrightarrow> integrity_mem aag subjects p ts ts' ipcbufs globals w w'"
+| trm_write:
+    "aag_subjects_have_auth_to subjects aag Write p
+     \<Longrightarrow> integrity_mem aag subjects p ts ts' ipcbufs globals w w'"
+| trm_globals:
+    "p \<in> globals \<Longrightarrow> integrity_mem aag subjects p ts ts' ipcbufs globals w w'"
+| trm_ipc:
+    "\<lbrakk> case_option False can_receive_ipc (ts p');
+       ts' p' = Some Running; p \<in> ipcbufs p'; pasObjectAbs aag p' \<notin> subjects \<rbrakk>
+       \<Longrightarrow> integrity_mem aag subjects p ts ts' ipcbufs globals w w'"
 
+abbreviation
+  "memory_integrity X aag x t1 t2 ipc \<equiv> integrity_mem (aag :: 'a PAS) {pasSubject aag} x t1 t2 ipc X"
 
-abbreviation memory_integrity
-where
-  "memory_integrity X aag x t1 t2 ipc == integrity_mem (aag :: 'a PAS) {pasSubject aag} x t1 t2 ipc X"
-
-inductive integrity_device for aag subjects p ts ts' w w'
-where
-  trd_lrefl: "\<lbrakk> pasObjectAbs aag p \<in> subjects \<rbrakk>
-     \<Longrightarrow> integrity_device aag subjects p ts ts' w w'" (* implied by wf and write *)
-  | trd_orefl: "\<lbrakk> w = w' \<rbrakk> \<Longrightarrow> integrity_device aag subjects p ts ts' w w'"
-  | trd_write: "\<lbrakk> aag_subjects_have_auth_to subjects aag Write p \<rbrakk> \<Longrightarrow> integrity_device aag subjects p ts ts' w w'"
-
-lemmas integrity_obj_simps [simp] = tro_orefl[OF refl]
-    tro_lrefl[OF singletonI]
-    trm_orefl[OF refl]
-    trd_orefl[OF refl]
-    tre_lrefl[OF singletonI]
-    tre_orefl[OF refl]
-
-
-
-
-subsection \<open>How the CDT can change\<close>
-
-text \<open>
-  The CDT and CDT_list integrity relations describe which modification to the CDT (@{term cdt})
-  , @{term is_original_cap} and @{term cdt_list})
-  are allowed by the policy aag when the system is controlled by subjects.
-
-  A modification to the CDT at a specific slot can happen for different reasons :
-  \begin{itemize}
-  \item we own directly or indirectly the slot. The "indirectly" means that
-        if an ancestor of a slot is owned by the subject, the slot is indirectly own by the subject
-  \item we are allowed explicitly to take ownership of the slot, for now this only happens when
-        we call someone: we are allowed to put a reply cap in its caller slot (slot number 3)
-\<close>
-
-(* FIXME MOVE*)
-notation parent_of_rtrancl ("_ \<Turnstile> _ \<rightarrow>* _" [60,0,60] 60)
-
-inductive cdt_direct_change_allowed for aag subjects tcbsts ptr
-  where
-  cdca_owned:
-  "pasObjectAbs aag (fst ptr) \<in> subjects \<Longrightarrow> cdt_direct_change_allowed aag subjects tcbsts ptr"
-| cdca_reply:
-  "\<lbrakk>tcbsts (fst ptr) = Some tcbst; direct_call subjects aag ep tcbst; (snd ptr) = tcb_cnode_index 3\<rbrakk>
-   \<Longrightarrow> cdt_direct_change_allowed aag subjects tcbsts ptr"
-
-(* for the moment the only caps that can be affected by that indirect control are reply caps *)
-definition cdt_change_allowed
-  where
-  "cdt_change_allowed aag subjects m tcbsts ptr \<equiv>
-   \<exists> pptr. m \<Turnstile> pptr \<rightarrow>* ptr \<and> cdt_direct_change_allowed aag subjects tcbsts pptr"
-
-lemma cdt_change_allowedI:
-  "\<lbrakk>m \<Turnstile> pptr \<rightarrow>* ptr; cdt_direct_change_allowed aag subjects tcbsts pptr\<rbrakk>
-   \<Longrightarrow> cdt_change_allowed aag subjects m tcbsts ptr"
-  by (fastforce simp: cdt_change_allowed_def simp del: split_paired_Ex)
-
-lemma cdt_change_allowedE:
-  assumes "cdt_change_allowed aag subjects m tcbsts ptr"
-  obtains pptr where "m \<Turnstile> pptr \<rightarrow>* ptr" "cdt_direct_change_allowed aag subjects tcbsts pptr"
-  using assms by (fastforce simp: cdt_change_allowed_def simp del: split_paired_Ex)
-
-lemma cdca_ccaI:
-  "\<lbrakk>cdt_direct_change_allowed aag subjects tcbsts ptr\<rbrakk>
-   \<Longrightarrow> cdt_change_allowed aag subjects m tcbsts ptr"
-  by (fastforce simp: cdt_change_allowed_def simp del: split_paired_Ex)
-
-lemmas cca_owned = cdt_change_allowedI[OF _ cdca_owned]
-lemmas cca_reply' = cdt_change_allowedI[OF _ cdca_owned]
-lemmas cca_direct[intro] = cdca_ccaI[OF cdca_owned]
-lemmas cca_reply = cdca_ccaI[OF cdca_reply]
-
-lemma cca_direct_single[intro]:
-  "is_subject aag (fst ptr) \<Longrightarrow> cdt_change_allowed aag {pasSubject aag} m kh ptr"
-  apply (rule cca_direct) by blast
-
-(* FIXME get a coherent naming scheme *)
-abbreviation cdt_change_allowed'
-where
-  "cdt_change_allowed' aag ptr s \<equiv> cdt_change_allowed aag {pasSubject aag} (cdt s)
-(tcb_states_of_state s) ptr"
-
-
-
-text\<open>
-  ptr is the slot we currently looking at
-  s is the initial state (v should be coherent with s)
-  v = (initial parent of ptr, initial "originality" of ptr)
-  v' = (final parent of ptr, final "originality" of ptr)
-\<close>
-definition integrity_cdt
-  :: "'a PAS \<Rightarrow> 'a set \<Rightarrow> cdt \<Rightarrow> (obj_ref \<Rightarrow> thread_state option)
-       \<Rightarrow> cslot_ptr \<Rightarrow> (cslot_ptr option \<times> bool) \<Rightarrow> (cslot_ptr option \<times> bool) \<Rightarrow> bool"
-where
-  "integrity_cdt aag subjects m tcbsts ptr v v'
-     \<equiv> v = v' \<or> cdt_change_allowed aag subjects m tcbsts ptr"
-
-lemma integrity_cdtE:
-  assumes hyp:"integrity_cdt aag subjects m tcbsts ptr v v'"
-  obtains "v = v'" | "cdt_change_allowed aag subjects m tcbsts ptr"
-  using hyp integrity_cdt_def by blast
-
-abbreviation integrity_cdt_state
-where
-  "integrity_cdt_state aag subjects s s' \<equiv>
-   (\<forall>x. integrity_cdt aag subjects (cdt s) (tcb_states_of_state s) x
-                      (cdt s x,is_original_cap s x) (cdt s' x, is_original_cap s' x))"
-
-abbreviation cdt_integrity
-where
-  "cdt_integrity aag \<equiv> integrity_cdt (aag :: 'a PAS) {pasSubject aag} "
-
-abbreviation cdt_integrity_state
-where
-  "cdt_integrity_state aag s s' \<equiv>
-   (\<forall>x. integrity_cdt (aag :: 'a PAS) {pasSubject aag} (cdt s) (tcb_states_of_state s) x
-                      (cdt s x,is_original_cap s x) (cdt s' x, is_original_cap s' x))"
-
-lemma integrity_cdt_refl[simp]: "integrity_cdt aag subjects m kh ptr v v"
-  by (simp add: integrity_cdt_def)
-
-lemma integrity_cdt_change_allowed[simp,intro]:
-  "cdt_change_allowed aag subjects m kh ptr \<Longrightarrow> integrity_cdt aag subjects m kh ptr v v'"
-  by (simp add: integrity_cdt_def)
-
-lemmas integrity_cdt_intros = integrity_cdt_refl integrity_cdt_change_allowed
-
-lemmas integrity_cdt_direct = cca_direct[THEN  integrity_cdt_change_allowed]
-
-
-
-text\<open>
-  m is the cdt of the initial state
-  tcbsts are tcb_states_of_state of the initial state
-  ptr is the slot we currently looking at
-  l and l' are the initial and final list of children of ptr
-\<close>
-definition integrity_cdt_list
-  :: "'a PAS \<Rightarrow> 'a set \<Rightarrow> cdt \<Rightarrow> (obj_ref \<Rightarrow> thread_state option) \<Rightarrow> cslot_ptr \<Rightarrow>
-      (cslot_ptr list) \<Rightarrow> (cslot_ptr list) \<Rightarrow> bool"
-where
-  "integrity_cdt_list aag subjects m tcbsts ptr l l'
-     \<equiv> (filtered_eq (cdt_change_allowed aag subjects m tcbsts) l l') \<or>
-        cdt_change_allowed aag subjects m tcbsts ptr"
-
-abbreviation integrity_cdt_list_state
-where
-  "integrity_cdt_list_state aag subjects s s' \<equiv>
-     (\<forall>x. integrity_cdt_list aag subjects (cdt s) (tcb_states_of_state s) x (cdt_list s x) (cdt_list s' x))"
-
-abbreviation cdt_list_integrity
-where
-  "cdt_list_integrity aag == integrity_cdt_list (aag :: 'a PAS) {pasSubject aag}"
-
-abbreviation cdt_list_integrity_state
-where
-  "cdt_list_integrity_state aag  s s' \<equiv>
-     (\<forall>x. integrity_cdt_list (aag :: 'a PAS) {pasSubject aag} (cdt s) (tcb_states_of_state s) x
-                             (cdt_list s x) (cdt_list s' x))"
-
-lemma integrity_cdt_list_refl[simp]: "integrity_cdt_list aag subjects m kh ptr v v"
-  by (simp add: integrity_cdt_list_def)
-
-lemma integrity_cdt_list_filt:
-  "filtered_eq (cdt_change_allowed aag subjects m kh) l l' \<Longrightarrow> integrity_cdt_list aag subjects m kh ptr l l'"
-  by (simp add: integrity_cdt_list_def)
-lemma integrity_cdt_list_change_allowed:
-  "cdt_change_allowed aag subjects m kh ptr \<Longrightarrow> integrity_cdt_list aag subjects m kh ptr l l'"
-  by (simp add: integrity_cdt_list_def)
-
-lemmas integrity_cdt_list_intros = integrity_cdt_list_filt integrity_cdt_list_change_allowed
-
-lemma integrity_cdt_listE:
-  assumes hyp:"integrity_cdt_list aag subjects m kh ptr l l'"
-  obtains "filtered_eq (cdt_change_allowed aag subjects m kh) l l'" |
-          "cdt_change_allowed aag subjects m kh ptr"
-  using hyp integrity_cdt_list_def by blast
-
+inductive integrity_device for aag subjects p ts ts' w w' where
+  trd_lrefl:
+    "pasObjectAbs aag p \<in> subjects \<Longrightarrow> integrity_device aag subjects p ts ts' w w'"
+| trd_orefl:
+    "w = w' \<Longrightarrow> integrity_device aag subjects p ts ts' w w'"
+| trd_write:
+    "aag_subjects_have_auth_to subjects aag Write p \<Longrightarrow> integrity_device aag subjects p ts ts' w w'"
 
 
 subsection \<open>How other stuff can change\<close>
 
-definition integrity_interrupts
-  :: "'a PAS \<Rightarrow> 'a set \<Rightarrow> irq \<Rightarrow> (obj_ref \<times> irq_state) \<Rightarrow> (obj_ref \<times> irq_state) \<Rightarrow> bool"
-where
-  "integrity_interrupts aag subjects irq v v'
-     \<equiv> v = v' \<or> pasIRQAbs aag irq \<in> subjects"
+definition integrity_interrupts ::
+  "'a PAS \<Rightarrow> 'a set \<Rightarrow> irq \<Rightarrow> (obj_ref \<times> irq_state) \<Rightarrow> (obj_ref \<times> irq_state) \<Rightarrow> bool" where
+  "integrity_interrupts aag subjects irq v v' \<equiv> v = v' \<or> pasIRQAbs aag irq \<in> subjects"
 
-lemma integrity_interrupts_refl[simp]: "integrity_interrupts aag subjects ptr v v"
-  by (simp add: integrity_interrupts_def)
-
-definition integrity_asids :: "'a PAS \<Rightarrow> 'a set \<Rightarrow> asid \<Rightarrow> obj_ref option \<Rightarrow> obj_ref option \<Rightarrow> bool"
-where
-  "integrity_asids aag subjects asid pp_opt pp_opt'
-     \<equiv> pp_opt = pp_opt' \<or> (\<forall> asid'. asid' \<noteq> 0 \<and> asid_high_bits_of asid' = asid_high_bits_of asid \<longrightarrow> pasASIDAbs aag asid' \<in> subjects)"
-
-lemma integrity_asids_refl[simp]: "integrity_asids aag subjects ptr s s"
-  by (simp add: integrity_asids_def)
 
 subsection \<open>General integrity\<close>
 
@@ -1809,1226 +846,58 @@ policy. See @{term "state_objs_to_policy s"} and @{term "pas_refined aag s"}.
 
 \<close>
 
-definition integrity_subjects
-  :: "'a set \<Rightarrow> 'a PAS \<Rightarrow> bool \<Rightarrow> obj_ref set \<Rightarrow> det_ext state \<Rightarrow> det_ext state \<Rightarrow> bool"
-where
+definition integrity_subjects ::
+  "'a set \<Rightarrow> 'a PAS \<Rightarrow> bool \<Rightarrow> obj_ref set \<Rightarrow> det_ext state \<Rightarrow> det_ext state \<Rightarrow> bool" where
   "integrity_subjects subjects aag activate X s s' \<equiv>
-         (\<forall>x. integrity_obj aag activate subjects (pasObjectAbs aag x) (kheap s x) (kheap s' x)) \<and>
-         (\<forall>x. integrity_eobj aag subjects (pasObjectAbs aag x) (ekheap s x) (ekheap s' x)) \<and>
-         (\<forall>x. integrity_mem aag subjects x (tcb_states_of_state s) (tcb_states_of_state s')
-                       (auth_ipc_buffers s) X
-                       (underlying_memory (machine_state s) x)
-                       (underlying_memory (machine_state s') x)) \<and>
-         (\<forall>x. integrity_device aag subjects x (tcb_states_of_state s) (tcb_states_of_state s')
-                       (device_state (machine_state s) x)
-                       (device_state (machine_state s') x)) \<and>
-         integrity_cdt_state aag subjects s s'\<and>
-         integrity_cdt_list_state aag subjects s s' \<and>
-         (\<forall>x. integrity_interrupts aag subjects x (interrupt_irq_node s x, interrupt_states s x)
-                                   (interrupt_irq_node s' x, interrupt_states s' x)) \<and>
-         (\<forall>x. integrity_asids aag subjects x (arm_asid_table (arch_state s) (asid_high_bits_of x))
-                              (arm_asid_table (arch_state s') (asid_high_bits_of x))) \<and>
-         (\<forall>d p. integrity_ready_queues aag subjects (pasDomainAbs aag d) (ready_queues s d p)
-                                       (ready_queues s' d p))"
-
-abbreviation integrity
-where
-  "integrity pas \<equiv> integrity_subjects {pasSubject pas} pas (pasMayActivate pas)"
-
-
-
-section \<open>Integrity transitivity\<close>
-
-subsection \<open>Object integrity transitivity\<close>
-
-lemma clear_asidpool_trans[elim]:
-  "\<lbrakk>asid_pool_integrity subjects aag pool pool';
-    asid_pool_integrity subjects aag pool' pool''\<rbrakk>
-   \<Longrightarrow> asid_pool_integrity subjects aag pool pool''"
-  unfolding asid_pool_integrity_def
-  apply clarsimp
-  apply (drule_tac x=x in spec)+
-  apply auto
-  done
-
-lemma tcb_bound_notification_reset_integrity_trans[elim]:
-  "\<lbrakk> tcb_bound_notification_reset_integrity ntfn ntfn' subjects aag;
-    tcb_bound_notification_reset_integrity ntfn' ntfn'' subjects aag \<rbrakk>
-    \<Longrightarrow> tcb_bound_notification_reset_integrity ntfn ntfn'' subjects aag"
-  by (auto simp: tcb_bound_notification_reset_integrity_def)
-
-lemma reply_cap_deletion_integrity_trans[elim]:
-  "\<lbrakk> reply_cap_deletion_integrity subjects aag cap cap';
-    reply_cap_deletion_integrity subjects aag cap' cap'' \<rbrakk>
-    \<Longrightarrow> reply_cap_deletion_integrity subjects aag cap cap''"
-  by (auto simp: reply_cap_deletion_integrity_def)
-
-
-lemma cnode_integrity_trans[elim]:
-  "\<lbrakk> cnode_integrity subjects aag cont cont';
-    cnode_integrity subjects aag cont' cont'' \<rbrakk>
-    \<Longrightarrow> cnode_integrity subjects aag cont cont''"
-   unfolding cnode_integrity_def
-   apply (intro allI)
-   apply (drule_tac x=l in spec)+
-   by fastforce
-
-lemma tcb_bound_notification_reset_eq_or_none:
-  "tcb_bound_notification_reset_integrity ntfn ntfn' subjects aag \<Longrightarrow> ntfn = ntfn' \<or> ntfn' = None"
-  by (auto simp: tcb_bound_notification_reset_integrity_def)
-
-
-lemma tro_alt_trans_spec: (* this takes a long time to process *)
-  "\<lbrakk>integrity_obj_alt aag activate es subjects ko ko';
-    integrity_obj_alt aag activate es subjects ko' ko'' \<rbrakk> \<Longrightarrow>
-    integrity_obj_alt aag activate es subjects ko ko''"
-  (* We need to consider nearly 200 cases, one for each possible pair
-     of integrity steps. We use the tro_tags to select subsets of goals
-     that can be solved by the same method. *)
-
-  (* Expand the first integrity step *)
-  apply (erule integrity_obj_alt.cases[where ko=ko and ko'=ko'])
-
-  (* LRefl and ORefl trivially collapse into the second integrity step *)
-  apply (find_goal \<open>match premises in "tro_tag LRefl" \<Rightarrow> -\<close>)
-  subgoal by (rule tro_alt_lrefl, simp)
-
-  apply (find_goal \<open>match premises in "tro_tag ORefl" \<Rightarrow> -\<close>)
-  subgoal by simp
-
-  (* Now re-tag the first step with tro_tag' *)
-  apply (all \<open>simp only:tro_tag_to_prime\<close>)
-  (* Expand the second integrity step, which will be tagged with tro_tag *)
-  apply (all \<open>erule integrity_obj_alt.cases\<close>)
-
-  (* There are some special cases that would be too slow or unsolvable by the bulk tactics.
-     We move them up here and solve manually *)
-  apply (find_goal \<open>match premises in "tro_tag' TCBReply" and "tro_tag TCBActivate" \<Rightarrow> -\<close>)
-  apply (clarsimp, rule tro_alt_tcb_reply[OF tro_tagI refl refl],
-         (rule exI; rule tcb.equality; simp add: arch_tcb_context_set_def); fastforce)
-
-  apply (find_goal \<open>match premises in "tro_tag' TCBReceive" and "tro_tag TCBReply" \<Rightarrow> -\<close>)
-  apply (clarsimp, rule tro_alt_tcb_reply[OF tro_tagI refl refl],
-         (rule exI; rule tcb.equality;
-          simp add: arch_tcb_context_set_def);
-         fastforce simp: indirect_send_def direct_send_def direct_reply_def
-                         allowed_call_blocked_def)
-
-  apply (find_goal \<open>match premises in "tro_tag TCBGeneric" and "tro_tag' TCBRestart" \<Rightarrow> -\<close>)
-  subgoal
-    apply (erule integrity_obj_alt.intros[simplified tro_tag_to_prime])
-            apply (rule refl | assumption
-                  | fastforce intro: tcb.equality
-                  | (erule tcb_bound_notification_reset_integrity_trans
-                           reply_cap_deletion_integrity_trans;
-                     fastforce))+
-    done
-
-  apply (find_goal \<open>match premises in "tro_tag TCBActivate" and "tro_tag' TCBRestart" \<Rightarrow> -\<close>)
-  apply (rule tro_alt_tcb_restart[OF tro_tagI],
-                 rule refl,
-                assumption,
-               (* somehow works better than tcb.equality *)
-               (simp only: tcb.splits; simp),
-              force+)[1]
-
-  apply (find_goal \<open>match premises in "tro_tag REp" and "tro_tag' REp" \<Rightarrow> -\<close>)
-  subgoal by (erule integrity_obj_alt.intros, (rule refl | assumption)+)
-
-  (* Select groups of subgoals by tag, then solve with the given methods *)
-  apply (all \<open>fails \<open>erule thin_rl[of "tro_tag LRefl"]\<close>
-             | time_methods \<open>solves \<open>
-                   fastforce intro: tro_alt_lrefl\<close>\<close>\<close>)
-
-  apply (all \<open>fails \<open>erule thin_rl[of "tro_tag ORefl"]\<close>
-             | time_methods \<open>solves \<open>
-                   drule sym[where t="ko''"];
-                   erule integrity_obj_alt.intros[simplified tro_tag_to_prime];
-                   solves \<open>simp\<close>\<close>\<close>\<close>)
-
-  apply (all \<open>fails \<open>erule thin_rl[of "tro_tag RNtfn"] thin_rl[of "tro_tag' RNtfn"]\<close>
-             | time_methods \<open>solves \<open>
-                   fastforce intro: tro_alt_ntfn\<close>\<close>\<close>)
-
-  apply (all \<open>fails \<open>erule thin_rl[of "tro_tag REp"]
-                    | erule thin_rl[of "tro_tag' REp"]
-                    | erule thin_rl[of "tro_tag RASID"]
-                    | erule thin_rl[of "tro_tag' RASID"]
-                    | erule thin_rl[of "tro_tag EpUnblock"]
-                    | erule thin_rl[of "tro_tag' EpUnblock"]
-                    | erule thin_rl[of "tro_tag RCNode"]
-                    | erule thin_rl[of "tro_tag' RCNode"]\<close>
-             | time_methods \<open>solves \<open>
-                   fastforce intro: integrity_obj_alt.intros tcb.equality
-                             simp: indirect_send_def direct_send_def\<close>\<close>\<close>)
-
-  (* TCB-TCB steps, somewhat slow *)
-  apply (all \<open>fails \<open>erule thin_rl[of "tro_tag TCBGeneric"]\<close>
-             | time_methods \<open>solves \<open>
-                    erule integrity_obj_alt.intros[simplified tro_tag_to_prime],
-                    (assumption | rule refl
-                    | ((erule exE)+)?, (rule exI)?, force intro: tcb.equality)+\<close>\<close>\<close>)
-
-  apply (all \<open>fails \<open>erule thin_rl[of "tro_tag' TCBGeneric"]\<close>
-             | time_methods \<open>solves \<open>
-                    erule integrity_obj_alt.intros,
-                    (assumption | rule refl
-                    | (elim exE)?, (intro exI)?, fastforce intro: tcb.equality
-                    | fastforce simp: indirect_send_def direct_send_def direct_call_def direct_reply_def
-                                dest: tcb_bound_notification_reset_eq_or_none)+\<close>\<close>\<close>)
-
-  apply (time_methods \<open>
-           succeeds \<open>match premises in T: "tro_tag _" and T': "tro_tag' _" \<Rightarrow>
-                                       \<open>print_fact T, print_fact T'\<close>\<close>,
-           fastforce intro: integrity_obj_alt.intros tcb.equality
-                     simp: indirect_send_def direct_send_def direct_call_def direct_reply_def
-                           send_blocked_on_def3 call_blocked_def allowed_call_blocked_def\<close>)+
-  done
-
-lemma tro_alt_reflp[intro!]:
-  "reflp (integrity_obj_alt aag activate es subjects)"
-  by (rule reflpI) (rule tro_alt_orefl; blast)
-
-lemma tro_alt_transp[intro!]:
-  "transp (integrity_obj_alt aag activate es subjects)"
-  by (rule transpI) (rule tro_alt_trans_spec)
-
-
-
-lemma tro_tro_alt[elim!]:
-  "integrity_obj aag activate es subjects ko ko'
-  \<Longrightarrow> integrity_obj_alt aag activate es subjects ko ko'"
-  unfolding integrity_obj_def
-  by (subst rtranclp_id[symmetric]; fastforce elim: rtranclp_mono[THEN predicate2D,rotated])
-
-lemmas integrity_objE = tro_tro_alt[THEN integrity_obj_alt.cases
-                                          [simplified tro_tag_def True_implies_equals]]
-
-
-
-lemma tro_trans:
-  "\<lbrakk>integrity_obj_state aag activate es s s'; integrity_obj_state aag activate es s' s''\<rbrakk>
-    \<Longrightarrow> integrity_obj_state aag activate es s s''"
-   unfolding integrity_obj_def
-  apply clarsimp
-  apply (drule_tac x = x in spec)+
-  by force
-
-lemma tre_trans:
-  "\<lbrakk>(\<forall>x. integrity_eobj aag es (pasObjectAbs aag x) (ekh x) (ekh' x));
-    (\<forall>x. integrity_eobj aag es (pasObjectAbs aag x) (ekh' x) (ekh'' x)) \<rbrakk> \<Longrightarrow>
-    (\<forall>x. integrity_eobj aag es (pasObjectAbs aag x) (ekh x) (ekh'' x))"
-by (fastforce elim!: integrity_eobj.cases
-              intro: integrity_eobj.intros)
-
-
-
-subsection \<open>CDT integrity transitivity\<close>
-
-lemma tcb_caller_slot_empty_on_recieve:
-  "\<lbrakk> valid_mdb s ; valid_objs s; kheap s tcb_ptr = Some (TCB tcb); ep_recv_blocked ep (tcb_state tcb) \<rbrakk> \<Longrightarrow>
-   tcb_caller tcb = NullCap \<and> cdt s (tcb_ptr,(tcb_cnode_index 3)) = None \<and>
-   descendants_of (tcb_ptr,(tcb_cnode_index 3)) (cdt s) = {}"
-   apply (simp only:valid_objs_def)
-   apply (drule bspec,fastforce)
-   apply (simp add:valid_obj_def)
-   apply (simp only:valid_tcb_def)
-   apply (drule conjunct1)
-   apply (drule_tac x="the (tcb_cap_cases (tcb_cnode_index 3))" in  bspec)
-    apply (fastforce simp:tcb_cap_cases_def)
-   apply (simp add:tcb_cap_cases_def split: thread_state.splits)
-  apply (subgoal_tac "caps_of_state s (tcb_ptr, tcb_cnode_index 3) = Some NullCap")
-   apply (simp only: valid_mdb_def2, drule conjunct1)
-   apply (intro conjI)
-    apply (simp add: mdb_cte_at_def)
-    apply (rule classical)
-    apply fastforce
-   apply (rule mdb_cte_at_no_descendants, fastforce+)[1]
-  apply (fastforce simp add: tcb_cnode_map_def caps_of_state_tcb_index_trans[OF get_tcb_rev])
-done
-
-
-(* FIXME MOVE next to tcb_states_of_state definition *)
-lemma tcb_states_of_state_kheap:
-   "\<lbrakk>kheap s slot = Some (TCB tcb)\<rbrakk>
-    \<Longrightarrow> tcb_states_of_state s slot = Some (tcb_state tcb)"
-  by (simp add:tcb_states_of_state_def get_tcb_def split: option.splits kernel_object.splits)
-
-lemma tcb_states_of_state_kheapI:
-   "\<lbrakk>kheap s slot = Some (TCB tcb); tcb_state tcb = tcbst\<rbrakk>
-    \<Longrightarrow> tcb_states_of_state s slot = Some tcbst"
-  by (simp add:tcb_states_of_state_def get_tcb_def split: option.splits kernel_object.splits)
-
-lemma tcb_states_of_state_kheapD:
-   "tcb_states_of_state s slot = Some tcbst \<Longrightarrow>
-    \<exists> tcb. kheap s slot = Some (TCB tcb) \<and> tcb_state tcb = tcbst"
-  by (simp add:tcb_states_of_state_def get_tcb_def split: option.splits kernel_object.splits)
-
-lemma tcb_states_of_state_kheapE:
-   assumes "tcb_states_of_state s slot = Some tcbst"
-   obtains tcb where "kheap s slot = Some (TCB tcb)" "tcb_state tcb = tcbst"
-  using assms tcb_states_of_state_kheapD by blast
-
-lemma cdt_direct_change_allowed_backward:
-  "\<lbrakk>integrity_obj_state aag activate subjects s s';
-    cdt_direct_change_allowed aag subjects (tcb_states_of_state s') ptr\<rbrakk> \<Longrightarrow>
-    cdt_direct_change_allowed aag subjects (tcb_states_of_state s) ptr"
-  apply (erule cdt_direct_change_allowed.cases)
-   subgoal by (rule cdca_owned)
-  apply (erule tcb_states_of_state_kheapE)
-  by (drule spec,
-      erule integrity_objE, erule cdca_owned;
-      (elim exE)?;
-      simp;
-      rule cdca_reply[rotated], assumption, assumption,
-        fastforce elim:tcb_states_of_state_kheapI simp:direct_call_def)
-
-lemma cdt_change_allowed_to_child:
-  "cdt_change_allowed aag subjects m tcbsts pptr \<Longrightarrow> m ptr = Some pptr
-   \<Longrightarrow> cdt_change_allowed aag subjects m tcbsts ptr"
-  apply (elim cdt_change_allowedE)
-  apply (erule cdt_change_allowedI[rotated])
-  by(fastforce intro: rtrancl_into_rtrancl simp: cdt_parent_of_def)
-
-lemma cdt_change_allowed_backward:
-  "\<lbrakk>integrity_obj_state aag activate subjects s s';
-    integrity_cdt_state aag subjects s s';
-    cdt_change_allowed aag subjects (cdt s') (tcb_states_of_state s') ptr\<rbrakk> \<Longrightarrow>
-    cdt_change_allowed aag subjects (cdt s) (tcb_states_of_state s) ptr"
-  apply (elim cdt_change_allowedE)
-  apply (drule(1) cdt_direct_change_allowed_backward)
-  apply (erule rtrancl_induct)
-  subgoal by (rule cdca_ccaI)
-  apply (rename_tac pptr0 ptr)
-  apply (frule_tac x=ptr in spec)
-  apply (elim integrity_cdtE; simp; elim conjE)
-  apply (erule cdt_change_allowed_to_child)
-  by(simp add: cdt_parent_of_def)
-
-lemma trcdt_trans:
-  "\<lbrakk>integrity_cdt_state aag subjects s s' ;
-    integrity_obj_state aag activate subjects s s' ;
-    integrity_cdt_state aag subjects s' s'' \<rbrakk>
-   \<Longrightarrow> integrity_cdt_state aag subjects s s''"
-  apply (intro allI)
-  apply (frule_tac x=x in spec)
-  apply (frule_tac x=x in spec[where P = "\<lambda>x. integrity_cdt _ _ (cdt s') _ x (_ x) (_ x)"])
-  apply (erule integrity_cdtE)+
-  apply simp
-  by (blast dest: cdt_change_allowed_backward)+
-
-lemma trcdtlist_trans:
-  "\<lbrakk>integrity_cdt_list_state aag subjects s s' ;
-    integrity_obj_state aag activate subjects s s' ;
-    integrity_cdt_state aag subjects s s' ;
-    integrity_cdt_list_state aag subjects s' s'' \<rbrakk>
-   \<Longrightarrow> integrity_cdt_list_state aag subjects s s''"
-  apply (intro allI)
-  apply (drule_tac x=x in spec [where P="\<lambda>ptr. integrity_cdt_list _ _ _ _ ptr (_ ptr) (_ ptr)"] )+
-  apply (erule integrity_cdt_listE)+
-      apply (rule integrity_cdt_list_filt)
-      apply (simp del: split_paired_All split_paired_Ex)
-      apply (erule weaken_filter_eq')
-  by (blast intro: integrity_cdt_list_intros dest: cdt_change_allowed_backward)+
-
-
-subsection \<open>Main integrity transitivity\<close>
-
-
-lemma trinterrupts_trans:
-  "\<lbrakk> (\<forall>x. integrity_interrupts aag subjects x (interrupt_irq_node s x, interrupt_states s x) (interrupt_irq_node s' x, interrupt_states s' x));
-    (\<forall>x. integrity_interrupts aag subjects x (interrupt_irq_node s' x, interrupt_states s' x) (interrupt_irq_node s'' x, interrupt_states s'' x)) \<rbrakk>
-   \<Longrightarrow> (\<forall>x. integrity_interrupts aag subjects x (interrupt_irq_node s x, interrupt_states s x) (interrupt_irq_node s'' x, interrupt_states s'' x))"
-  apply (simp add: integrity_interrupts_def
-                  del: split_paired_All)
-  apply metis
-  done
-
-lemma trasids_trans:
-  "\<lbrakk> (\<forall>x. integrity_asids aag subjects x (arm_asid_table (arch_state s) (asid_high_bits_of x)) (arm_asid_table (arch_state s') (asid_high_bits_of x)));
-     (\<forall>x. integrity_asids aag subjects x (arm_asid_table (arch_state s') (asid_high_bits_of x)) (arm_asid_table (arch_state s'') (asid_high_bits_of x)))\<rbrakk>
-   \<Longrightarrow>
-     (\<forall>x. integrity_asids aag subjects x (arm_asid_table (arch_state s) (asid_high_bits_of x)) (arm_asid_table (arch_state s'') (asid_high_bits_of x)))"
-  apply (clarsimp simp: integrity_asids_def)
-  apply metis
-  done
-
-lemma trrqs_trans:
-  "\<lbrakk> (\<forall>d p. integrity_ready_queues aag subjects (pasDomainAbs aag d) (ready_queues s d p) (ready_queues s' d p));
-     (\<forall>d p. integrity_ready_queues aag subjects (pasDomainAbs aag d) (ready_queues s' d p) (ready_queues s'' d p)) \<rbrakk>
-   \<Longrightarrow> (\<forall>d p. integrity_ready_queues aag subjects (pasDomainAbs aag d) (ready_queues s d p) (ready_queues s'' d p))"
-apply (clarsimp simp: integrity_ready_queues_def)
-apply (metis append_assoc)
-done
-
-(* FIXME RENAME *)
-lemma tsos_tro:
-  "\<lbrakk>integrity_obj_state aag activate subjects s s'; tcb_states_of_state s' p = Some a;
-    receive_blocked_on ep a; pasObjectAbs aag p \<notin> subjects \<rbrakk> \<Longrightarrow> tcb_states_of_state s p = Some a"
-  apply (drule_tac x = p in spec)
-  apply (erule integrity_objE, simp_all add: tcb_states_of_state_def get_tcb_def)
-  by fastforce+
-
-lemma can_receive_ipc_backward:
-  "\<lbrakk>integrity_obj_state aag activate subjects s s'; tcb_states_of_state s' p = Some a;
-    can_receive_ipc a; pasObjectAbs aag p \<notin> subjects \<rbrakk>
-   \<Longrightarrow> case tcb_states_of_state s p of None \<Rightarrow> False | Some x \<Rightarrow> can_receive_ipc x"
-  apply (drule_tac x = p in spec)
-  apply (erule integrity_objE;
-         (fastforce simp: tcb_states_of_state_def get_tcb_def
-                         call_blocked_def allowed_call_blocked_def
-                   split: option.splits kernel_object.splits
-         | cases a \<comment> \<open>only split when needed\<close>)+)
-  done
-
-
-
-lemma auth_ipc_buffers_tro:
-  "\<lbrakk>integrity_obj_state aag activate subjects s s'; x \<in> auth_ipc_buffers s' p;
-          pasObjectAbs aag p \<notin> subjects \<rbrakk>
-  \<Longrightarrow> x \<in> auth_ipc_buffers s p "
-  by (drule_tac x = p in spec)
-     (erule integrity_objE;
-      fastforce simp: tcb_states_of_state_def get_tcb_def auth_ipc_buffers_def
-               split: cap.split_asm arch_cap.split_asm if_split_asm bool.splits)
-
-
-lemma auth_ipc_buffers_tro_fwd:
-  "\<lbrakk>integrity_obj_state aag activate subjects s s'; x \<in> auth_ipc_buffers s p;
-          pasObjectAbs aag p \<notin> subjects \<rbrakk>
-  \<Longrightarrow> x \<in> auth_ipc_buffers s' p "
-  by (drule_tac x = p in spec)
-     (erule integrity_objE;
-      fastforce simp: tcb_states_of_state_def get_tcb_def auth_ipc_buffers_def
-               split: cap.split_asm arch_cap.split_asm if_split_asm bool.splits)
-
-
-lemma tsos_tro_running:
-  "\<lbrakk>\<forall>x. integrity_obj aag activate subjects (pasObjectAbs aag x) (kheap s x) (kheap s' x);
-       tcb_states_of_state s p = Some Structures_A.Running;
-          pasObjectAbs aag p \<notin> subjects \<rbrakk>
-     \<Longrightarrow> tcb_states_of_state s' p = Some Structures_A.Running"
-  by (drule_tac x = p in spec)
-     (erule integrity_objE,
-         simp_all add: tcb_states_of_state_def get_tcb_def indirect_send_def
-                       direct_send_def direct_call_def direct_reply_def call_blocked_def allowed_call_blocked_def)
-
-
-lemma integrity_trans:
-  assumes t1: "integrity_subjects subjects aag activate X s s'"
-  and     t2: "integrity_subjects subjects aag activate X s' s''"
-  shows  "integrity_subjects subjects aag activate X s s''"
-proof -
-  from t1 have tro1: "integrity_obj_state aag activate subjects s s'"
-    unfolding integrity_subjects_def by simp
-  from t2 have tro2: "integrity_obj_state aag activate subjects s' s''"
-    unfolding integrity_subjects_def by simp
-
-  have intm: "\<forall>x. integrity_mem aag subjects x
-                  (tcb_states_of_state s) (tcb_states_of_state s'') (auth_ipc_buffers s) X
-                  (underlying_memory (machine_state s) x)
-                  (underlying_memory (machine_state s'') x)" (is "\<forall>x. ?P x s s''")
-  proof
-    fix x
-    from t1 t2 have m1: "?P x s s'" and m2: "?P x s' s''" unfolding integrity_subjects_def by auto
-
-    from m1 show "?P x s s''"
-    proof cases
-      case trm_lrefl thus ?thesis by (rule integrity_mem.intros)
-    next
-      case trm_globals thus ?thesis by (rule integrity_mem.intros)
-    next
-      case trm_orefl
-      from m2 show ?thesis
-      proof cases
-        case (trm_ipc p')
-
-        show ?thesis
-        proof (rule integrity_mem.trm_ipc)
-          from trm_ipc show "case_option False can_receive_ipc (tcb_states_of_state s p')"
-            by (fastforce split: option.splits dest: can_receive_ipc_backward [OF tro1])
-
-          from trm_ipc show "x \<in> auth_ipc_buffers s p'"
-            by (fastforce split: option.splits intro: auth_ipc_buffers_tro [OF tro1])
-        qed (simp_all add: trm_ipc)
-      qed (auto simp add: trm_orefl intro: integrity_mem.intros)
-    next
-      case trm_write thus ?thesis by (rule integrity_mem.intros)
-    next
-      case (trm_ipc p')
-      note trm_ipc1 = trm_ipc
-
-      from m2 show ?thesis
-      proof cases
-        case trm_orefl
-        thus ?thesis using trm_ipc1
-          by (auto intro!: integrity_mem.trm_ipc simp add: restrict_map_Some_iff elim!: tsos_tro_running [OF tro2, rotated])
-      next
-        case (trm_ipc p'')
-        show ?thesis
-        proof (cases "p' = p''")
-          case True thus ?thesis using trm_ipc trm_ipc1 by (simp add: restrict_map_Some_iff)
-        next
-          (* 2 tcbs sharing same IPC buffer, we can appeal to either t1 or t2 *)
-          case False
-          thus ?thesis using trm_ipc1
-            by (auto intro!: integrity_mem.trm_ipc simp add: restrict_map_Some_iff elim!: tsos_tro_running [OF tro2, rotated])
-        qed
-      qed (auto simp add: trm_ipc intro: integrity_mem.intros)
-    qed
-  qed
-
-  moreover have "\<forall>x. integrity_device aag subjects x
-                  (tcb_states_of_state s) (tcb_states_of_state s'')
-                  (device_state (machine_state s) x)
-                  (device_state (machine_state s'') x)" (is "\<forall>x. ?P x s s''")
-  proof
-    fix x
-    from t1 t2 have m1: "?P x s s'" and m2: "?P x s' s''" unfolding integrity_subjects_def by auto
-
-    from m1 show "?P x s s''"
-    proof cases
-      case trd_lrefl thus ?thesis by (rule integrity_device.intros)
-    next
-      case torel1: trd_orefl
-      from m2 show ?thesis
-      proof cases
-        case (trd_lrefl) thus ?thesis by (rule integrity_device.trd_lrefl)
-      next
-        case trd_orefl thus ?thesis
-          by (simp add:torel1)
-      next
-        case trd_write thus ?thesis by (rule integrity_device.trd_write)
-      qed
-    next
-      case trd_write thus ?thesis by (rule integrity_device.intros)
-    qed
-  qed
-  thus ?thesis using tro_trans[OF tro1 tro2] t1 t2 intm
-    apply (clarsimp simp add: integrity_subjects_def simp del:  split_paired_All)
-    apply (frule(2) trcdt_trans)
-    apply (frule(3) trcdtlist_trans)
-    apply (frule(1) trinterrupts_trans[simplified])
-    apply (frule(1) trasids_trans[simplified])
-    apply (frule(1) tre_trans[simplified])
-    apply (frule(1) trrqs_trans[simplified])
-    by blast
-qed
-
-lemma integrity_refl [simp]:
-  "integrity_subjects S aag activate X s s"
-unfolding integrity_subjects_def
-by simp
-
-section \<open>Generic AC stuff\<close>
-
-subsection \<open>Basic integrity lemmas\<close>
-
-(* Tom says that Gene Wolfe says that autarchy \<equiv> self authority. *)
-
-lemma integrity_update_autarch:
-  "\<lbrakk> integrity aag X st s; is_subject aag ptr \<rbrakk>
-   \<Longrightarrow> integrity aag X st (s\<lparr>kheap := kheap s(ptr \<mapsto> obj)\<rparr>)"
-  unfolding integrity_subjects_def
-  apply (intro conjI,simp_all)
-   apply clarsimp
-   apply (drule_tac x = x in spec, erule integrity_mem.cases)
-   apply ((auto intro: integrity_mem.intros)+)[4]
-   apply (erule trm_ipc, simp_all)
-   apply (clarsimp simp: restrict_map_Some_iff tcb_states_of_state_def get_tcb_def)
-  apply clarsimp
-  apply (drule_tac x = x in spec, erule integrity_device.cases)
-    apply (erule integrity_device.trd_lrefl)
-   apply (erule integrity_device.trd_orefl)
-  apply (erule integrity_device.trd_write)
-  done
-
-lemma set_object_integrity_autarch:
-  "\<lbrace>integrity aag X st and K (is_subject aag ptr)\<rbrace>
-     set_object ptr obj
-   \<lbrace>\<lambda>rv. integrity aag X st\<rbrace>"
-  apply (wpsimp wp: set_object_wp)
-  apply (rule integrity_update_autarch, simp_all)
-  done
-
-lemma tcb_states_of_state_trans_state[simp]:
-  "tcb_states_of_state (trans_state f s) = tcb_states_of_state s"
-  by (simp add: tcb_states_of_state_def get_tcb_exst_update)
-
-lemma eintegrity_sa_update[simp]:
-  "integrity aag X st (scheduler_action_update f s) = integrity aag X st s"
-  by (simp add: integrity_subjects_def trans_state_update'[symmetric])
-
-lemma trans_state_back[simp]:
-  "trans_state (\<lambda>_. exst s) s = s"
-  by simp
-
-declare wrap_ext_op_det_ext_ext_def[simp]
-
-crunch integrity[wp]: set_thread_state_ext "integrity aag X st"
-
-crunch integrity_autarch: set_thread_state "integrity aag X st"
-
-lemmas integrity_def = integrity_subjects_def
-
-subsection \<open>Out of subject cap manipulation\<close>
-
-(* FIXME MOVE *)
-lemma all_children_descendants_of:
-  "\<lbrakk> all_children P m ; p \<in> descendants_of q m ; P q \<rbrakk> \<Longrightarrow> P p "
-  apply (simp add: descendants_of_def)
-  apply (erule trancl_induct[where P=P])
-  unfolding cdt_parent_of_def
-   apply (erule(2) all_childrenD)+
-  done
-
-lemmas all_children_parent_of_trancl =
-                    all_children_descendants_of[simplified descendants_of_def,simplified]
-
-lemma all_children_parent_of_rtrancl:
-  "\<lbrakk> all_children P m ; m \<Turnstile> q \<rightarrow>* p ; P q \<rbrakk> \<Longrightarrow> P p "
-  by (drule rtranclD,elim conjE disjE; blast dest:all_children_parent_of_trancl)
-
-lemma pas_refined_all_children':
-  "\<lbrakk>valid_mdb s ; pas_refined aag s ; m = (cdt s) \<rbrakk> \<Longrightarrow>
-   all_children (\<lambda>x. is_subject aag (fst x) \<or> is_transferable (caps_of_state s x)) m"
-  apply (rule all_childrenI)
-  apply (erule disjE)
-   apply (simp add: pas_refined_def,elim conjE)
-   apply (rule disjCI)
-   apply (subgoal_tac
-               "(pasObjectAbs aag (fst p), Control, pasObjectAbs aag (fst c)) \<in> pasPolicy aag")
-    apply (fastforce elim: aag_wellformed_control_is_owns[THEN iffD1])
-   apply (simp add: state_objs_to_policy_def auth_graph_map_def)
-   apply (erule set_mp)
-   apply (frule(1) sbta_cdt)
-   apply force
-  apply (rule disjI2)
-  by (rule is_transferable_all_children[THEN all_childrenD]; solves \<open>simp\<close>)
-
-lemmas pas_refined_all_children = pas_refined_all_children'[OF _ _ refl]
-
-(* FIXME MOVE just after cte_wp_at_cases2 *)
-lemma caps_of_state_def':
-  "caps_of_state s slot =
-    (case kheap s (fst slot) of
-       Some (TCB tcb) \<Rightarrow> tcb_cnode_map tcb (snd slot)
-     | Some (CNode sz content) \<Rightarrow> (if well_formed_cnode_n sz content then content (snd slot) else None)
-     | _ \<Rightarrow> None)"
-  by (fastforce simp: caps_of_state_cte_wp_at cte_wp_at_cases2
-                split: option.splits kernel_object.splits)
-
-lemma caps_of_state_cnode:
-  "\<lbrakk>kheap s pos = Some (CNode sz content); well_formed_cnode_n sz content\<rbrakk> \<Longrightarrow>
-   caps_of_state s (pos,addr) = content addr"
-  by (simp add:caps_of_state_def')
-
-lemma caps_of_state_tcb:
-  "\<lbrakk>kheap s pos = Some (TCB tcb)\<rbrakk> \<Longrightarrow>
-   caps_of_state s (pos,addr) = tcb_cnode_map tcb addr"
-  by (simp add:caps_of_state_def')
-
-(* FIXME MOVE next to tcb_cnode_cases_simps *)
-lemma tcb_cnode_map_simps[simp]:
-  "tcb_cnode_map tcb (tcb_cnode_index 0) = Some (tcb_ctable tcb)"
-  "tcb_cnode_map tcb (tcb_cnode_index (Suc 0)) = Some (tcb_vtable tcb)"
-  "tcb_cnode_map tcb (tcb_cnode_index 2) = Some (tcb_reply tcb)"
-  "tcb_cnode_map tcb (tcb_cnode_index 3) = Some (tcb_caller tcb)"
-  "tcb_cnode_map tcb (tcb_cnode_index 4) = Some (tcb_ipcframe tcb)"
-  by (simp_all add: tcb_cnode_map_def)
-
-(* FIXME MOVE *)
-lemma valid_mdb_reply_mdb[elim!]:
-  "valid_mdb s \<Longrightarrow> reply_mdb (cdt s) (caps_of_state s)"
-  by (simp add:valid_mdb_def)
-
-(* FIXME MOVE *)
-lemma invs_reply_mdb[elim!]: "invs s \<Longrightarrow> reply_mdb (cdt s) (caps_of_state s)"
-  by (simp add:invs_def valid_state_def valid_mdb_def)
-
-lemma parent_of_rtrancl_no_descendant:
-  "\<lbrakk>m \<Turnstile> pptr \<rightarrow>* ptr; descendants_of pptr m = {}\<rbrakk> \<Longrightarrow> pptr = ptr"
-  by (fastforce simp add:rtrancl_eq_or_trancl descendants_of_def)
-
-(* FIXME MOVE *)
-lemma tcb_atD:
-  "tcb_at ptr s \<Longrightarrow> \<exists>tcb. kheap s ptr = Some (TCB tcb)"
-   by (cases "the (kheap s ptr)";fastforce simp:obj_at_def is_tcb_def)
-
-(* FIXME MOVE *)
-lemma tcb_atE:
-  assumes hyp: "tcb_at ptr s"
-  obtains tcb where "kheap s ptr = Some (TCB tcb)"
-   using hyp[THEN tcb_atD] by blast
-
-(*FIXME MOVE *)
-lemma tcb_atI:
-  "kheap s ptr = Some (TCB tcb) \<Longrightarrow> tcb_at ptr s"
-  by (simp add:obj_at_def is_tcb_def)
-
-
-
-lemma descendant_of_caller_slot:
-  "\<lbrakk>valid_mdb s; valid_objs s; tcb_at t s\<rbrakk> \<Longrightarrow> descendants_of (t, tcb_cnode_index 3) (cdt s) = {}"
-  apply (frule(1) tcb_caller_cap)
-  apply (clarsimp simp add:cte_wp_at_caps_of_state is_cap_simps; elim disjE ;clarsimp)
-  subgoal by (intro allI no_children_empty_desc[THEN iffD1] reply_cap_no_children)
-  apply (drule valid_mdb_mdb_cte_at)
-  apply (erule mdb_cte_at_no_descendants)
-  apply (simp add:cte_wp_at_caps_of_state)
-  done
-
-lemma cca_to_transferable_or_subject:
-  "\<lbrakk>valid_objs s; valid_mdb s; pas_refined aag s; cdt_change_allowed' aag ptr s \<rbrakk>
-  \<Longrightarrow> is_subject aag (fst ptr) \<or> is_transferable (caps_of_state s ptr)"
-  apply (elim cdt_change_allowedE cdt_direct_change_allowed.cases)
-   apply (rule all_children_parent_of_rtrancl[OF pas_refined_all_children]; blast)
-  apply (simp add:rtrancl_eq_or_trancl,elim disjE conjE)
-   apply (simp add:direct_call_def, elim conjE)
-   apply (drule tcb_states_of_state_kheapD, elim exE conjE)
-   apply (frule(2) tcb_caller_slot_empty_on_recieve ,simp)
-   apply (cases ptr,simp)
-   apply (simp add:caps_of_state_tcb)
-  apply (elim tcb_states_of_state_kheapE)
-  apply (drule(2) descendant_of_caller_slot[OF _ _ tcb_atI])
-  by (force simp add: descendants_of_def simp del:split_paired_All)
-
-lemma is_transferable_weak_derived:
-  "weak_derived cap cap' \<Longrightarrow> is_transferable_cap cap = is_transferable_cap cap'"
-  unfolding is_transferable.simps weak_derived_def copy_of_def same_object_as_def
-  by (fastforce simp: is_cap_simps split:cap.splits)
-
-lemma aag_cdt_link_Control:
-  "\<lbrakk> cdt s x = Some y; \<not> is_transferable(caps_of_state s x); pas_refined aag s \<rbrakk>
-    \<Longrightarrow> (pasObjectAbs aag (fst y), Control, pasObjectAbs aag (fst x)) \<in> pasPolicy aag"
-  by (fastforce elim: pas_refined_mem[rotated] sta_cdt)
-
-lemma aag_cdt_link_DeleteDerived:
-  "\<lbrakk> cdt s x = Some y; pas_refined aag s \<rbrakk>
-    \<Longrightarrow> (pasObjectAbs aag (fst y), DeleteDerived, pasObjectAbs aag (fst x)) \<in> pasPolicy aag"
-  by (fastforce elim: pas_refined_mem[rotated] sta_cdt_transferable)
-
-lemma tcb_states_of_state_to_auth:
-  "\<lbrakk>tcb_states_of_state s thread = Some tcbst; pas_refined aag s \<rbrakk>
-   \<Longrightarrow> \<forall> (obj,auth) \<in> tcb_st_to_auth tcbst.
-                  (pasObjectAbs aag thread, auth, pasObjectAbs aag obj) \<in> pasPolicy aag"
-
-   apply clarsimp
-   apply (erule pas_refined_mem[rotated])
-   apply (rule sta_ts)
-   apply (simp add:thread_states_def)
-   done
-
-lemma tcb_states_of_state_to_auth':
-  "\<lbrakk>tcb_states_of_state s thread = Some tcbst; pas_refined aag s;
-    (obj,auth) \<in> tcb_st_to_auth tcbst \<rbrakk>
-   \<Longrightarrow> (pasObjectAbs aag thread, auth, pasObjectAbs aag obj) \<in> pasPolicy aag"
-   using tcb_states_of_state_to_auth by blast
-
-lemma ep_recv_blocked_def:
-  "ep_recv_blocked ep st \<longleftrightarrow> (\<exists>pl. st = BlockedOnReceive ep pl)"
-  by (simp split: thread_state.split)
-
-lemma cdt_change_allowed_delete_derived:
-  "valid_objs s \<Longrightarrow> valid_mdb s \<Longrightarrow> pas_refined aag s \<Longrightarrow> cdt_change_allowed' aag slot s
-   \<Longrightarrow> aag_has_auth_to aag DeleteDerived (fst slot)"
-  apply (elim cdt_change_allowedE cdt_direct_change_allowed.cases)
-   apply (erule rtrancl_induct)
-    apply (solves\<open>simp add: pas_refined_refl\<close>)
-   apply (fastforce simp: cdt_parent_of_def
-                    dest: aag_cdt_link_DeleteDerived
-                   intro: aag_wellformed_delete_derived_trans)
-  apply (clarsimp simp: direct_call_def ep_recv_blocked_def)
-  apply (frule(1)tcb_states_of_state_to_auth)
-  apply (elim tcb_states_of_state_kheapE)
-  apply (frule(2) descendant_of_caller_slot[OF _ _ tcb_atI])
-  apply (frule(1) parent_of_rtrancl_no_descendant)
-  apply clarsimp
-  by (rule aag_wellformed_delete_derived'[OF _ _ pas_refined_wellformed])
-
-end
-
-context pspace_update_eq begin
-
-interpretation Arch . (*FIXME: arch_split*)
-
-lemma integrity_update_eq[iff]:
-  "tcb_states_of_state (f s) = tcb_states_of_state s"
-  by (simp add: pspace tcb_states_of_state_def get_tcb_def)
-
-end
-
-subsection \<open>Various abbreviations\<close>
-
-context begin interpretation Arch . (*FIXME: arch_split*)
-
-definition label_owns_asid_slot :: "'a PAS \<Rightarrow> 'a \<Rightarrow> asid \<Rightarrow> bool"
-where
+     (\<forall>x. integrity_obj aag activate subjects (pasObjectAbs aag x) (kheap s x) (kheap s' x))
+   \<and> (\<forall>x. integrity_eobj aag subjects (pasObjectAbs aag x) (ekheap s x) (ekheap s' x))
+   \<and> integrity_cdt_state aag subjects s s'
+   \<and> integrity_cdt_list_state aag subjects s s'
+   \<and> (\<forall>x. integrity_interrupts aag subjects x (interrupt_irq_node s x, interrupt_states s x)
+                               (interrupt_irq_node s' x, interrupt_states s' x))
+   \<and> (\<forall>d p. integrity_ready_queues aag subjects (pasDomainAbs aag d) (ready_queues s d p)
+                                   (ready_queues s' d p))
+   \<and> (\<forall>x. integrity_mem aag subjects x (tcb_states_of_state s) (tcb_states_of_state s')
+                        (auth_ipc_buffers s) X
+                        (underlying_memory (machine_state s) x)
+                        (underlying_memory (machine_state s') x))
+   \<and> (\<forall>x. integrity_device aag subjects x (tcb_states_of_state s) (tcb_states_of_state s')
+                           (device_state (machine_state s) x)
+                           (device_state (machine_state s') x))
+   \<and> (\<forall>x. integrity_asids aag subjects x s s')"
+
+abbreviation "integrity pas \<equiv> integrity_subjects {pasSubject pas} pas (pasMayActivate pas)"
+
+subsection \<open>Various definitions and abbreviations\<close>
+
+definition label_owns_asid_slot :: "'a PAS \<Rightarrow> 'a \<Rightarrow> asid \<Rightarrow> bool" where
   "label_owns_asid_slot aag l asid \<equiv>
      (l, Control, pasASIDAbs aag asid) \<in> pasPolicy aag"
 
-definition cap_links_asid_slot :: "'a PAS \<Rightarrow> 'a \<Rightarrow> cap \<Rightarrow> bool"
-where
-  "cap_links_asid_slot aag l cap \<equiv> (\<forall>asid \<in> cap_asid' cap.
-      label_owns_asid_slot aag l asid)"
+fun cap_asid' :: "cap \<Rightarrow> asid set" where
+  "cap_asid' (ArchObjectCap acap) = acap_asid' acap"
+| "cap_asid' _ = {}"
 
-abbreviation is_subject_asid :: "'a PAS \<Rightarrow> asid \<Rightarrow> bool"
-where
+definition cap_links_asid_slot :: "'a PAS \<Rightarrow> 'a \<Rightarrow> cap \<Rightarrow> bool" where
+  "cap_links_asid_slot aag l cap \<equiv> (\<forall>asid \<in> cap_asid' cap. label_owns_asid_slot aag l asid)"
+
+abbreviation is_subject_asid :: "'a PAS \<Rightarrow> asid \<Rightarrow> bool" where
   "is_subject_asid aag asid \<equiv> pasASIDAbs aag asid = pasSubject aag"
 
-lemma clas_no_asid:
-  "cap_asid' cap = {} \<Longrightarrow> cap_links_asid_slot aag l cap"
-  unfolding cap_links_asid_slot_def by simp
-
-definition cap_links_irq
-where
+definition cap_links_irq :: "'a PAS \<Rightarrow> 'a \<Rightarrow> cap \<Rightarrow> bool" where
   "cap_links_irq aag l cap \<equiv>
-       \<forall>irq \<in> cap_irqs_controlled cap. (l, Control, pasIRQAbs aag irq) \<in> pasPolicy aag"
+     \<forall>irq \<in> cap_irqs_controlled cap. (l, Control, pasIRQAbs aag irq) \<in> pasPolicy aag"
 
-lemma cli_no_irqs:
-  "cap_irqs_controlled cap = {} \<Longrightarrow> cap_links_irq aag l cap"
-  unfolding cap_links_irq_def by simp
-
-abbreviation is_subject_irq :: "'a PAS \<Rightarrow> irq \<Rightarrow> bool"
-where
+abbreviation is_subject_irq :: "'a PAS \<Rightarrow> irq \<Rightarrow> bool" where
   "is_subject_irq aag irq \<equiv> pasIRQAbs aag irq = pasSubject aag"
 
-definition aag_cap_auth :: "'a PAS \<Rightarrow> 'a \<Rightarrow> cap \<Rightarrow> bool"
-where
+definition aag_cap_auth :: "'a PAS \<Rightarrow> 'a \<Rightarrow> cap \<Rightarrow> bool" where
   "aag_cap_auth aag l cap \<equiv>
-      (\<forall>x \<in> obj_refs cap. \<forall>auth \<in> cap_auth_conferred cap. (l, auth, pasObjectAbs aag x) \<in> pasPolicy aag)
-    \<and> (\<forall>x \<in> untyped_range cap. (l, Control, pasObjectAbs aag x) \<in> pasPolicy aag)
-    \<and> cap_links_asid_slot aag l cap \<and> cap_links_irq aag l cap"
+     (\<forall>x \<in> obj_refs cap. \<forall>auth \<in> cap_auth_conferred cap. (l, auth, pasObjectAbs aag x) \<in> pasPolicy aag)
+   \<and> (\<forall>x \<in> untyped_range cap. (l, Control, pasObjectAbs aag x) \<in> pasPolicy aag)
+   \<and> cap_links_asid_slot aag l cap \<and> cap_links_irq aag l cap"
 
-abbreviation pas_cap_cur_auth :: "'a PAS \<Rightarrow> cap \<Rightarrow> bool"
-where
+abbreviation pas_cap_cur_auth :: "'a PAS \<Rightarrow> cap \<Rightarrow> bool" where
   "pas_cap_cur_auth aag cap \<equiv> aag_cap_auth aag (pasSubject aag) cap"
-
-subsection \<open>Random lemmas that belong here\<close>
-
-crunch integrity_autarch: as_user "integrity aag X st"
-
-lemma owns_thread_owns_cspace:
-  "\<lbrakk> is_subject aag thread; pas_refined aag s; get_tcb thread s = Some tcb; is_cnode_cap (tcb_ctable tcb); x \<in> obj_refs (tcb_ctable tcb)\<rbrakk>
-    \<Longrightarrow> is_subject aag x"
-  apply (drule get_tcb_SomeD)
-  apply (drule cte_wp_at_tcbI[where t="(thread, tcb_cnode_index 0)" and P="\<lambda>cap. cap = tcb_ctable tcb", simplified])
-  apply (auto simp: cte_wp_at_caps_of_state is_cap_simps cap_auth_conferred_def
-              elim: caps_of_state_pasObjectAbs_eq [where p = "(thread, tcb_cnode_index 0)"])
-  done
-
-
-
-lemma is_subject_into_is_subject_asid:
-  "\<lbrakk> cap_links_asid_slot aag (pasObjectAbs aag p) cap; is_subject aag p; pas_refined aag s;
-         asid \<in> cap_asid' cap \<rbrakk>
-     \<Longrightarrow> is_subject_asid aag asid"
-  apply (clarsimp simp add: cap_links_asid_slot_def label_owns_asid_slot_def)
-  apply (drule (1) bspec)
-  apply (drule (1) pas_refined_Control)
-  apply simp
-  done
-
-(* MOVE *)
-lemma clas_caps_of_state:
-  "\<lbrakk> caps_of_state s slot = Some cap; pas_refined aag s \<rbrakk> \<Longrightarrow> cap_links_asid_slot aag (pasObjectAbs aag (fst slot)) cap"
-apply (clarsimp simp add: cap_links_asid_slot_def label_owns_asid_slot_def pas_refined_def)
-apply (blast dest: state_asids_to_policy_aux.intros)
-done
-
-lemma as_user_state_vrefs[wp]:
-  "\<lbrace>\<lambda>s. P (state_vrefs s)\<rbrace> as_user t f \<lbrace>\<lambda>rv s. P (state_vrefs s)\<rbrace>"
-  apply (simp add: as_user_def)
-  apply (wpsimp wp: set_object_wp)
-  apply (clarsimp simp: state_vrefs_def vs_refs_no_global_pts_def get_tcb_def
-                 elim!: rsubst[where P=P, OF _ ext]
-                 split: option.split_asm Structures_A.kernel_object.split)
-  done
-
-lemma as_user_tcb_states[wp]:
-  "\<lbrace>\<lambda>s. P (tcb_states_of_state s)\<rbrace> as_user t f \<lbrace>\<lambda>rv s. P (tcb_states_of_state s)\<rbrace>"
-  apply (simp add: as_user_def)
-  apply (wpsimp wp: set_object_wp)
-  apply (clarsimp simp: thread_states_def get_tcb_def tcb_states_of_state_def
-                 elim!: rsubst[where P=P, OF _ ext] split: option.split)
-  done
-
-lemma as_user_thread_state[wp]:
-  "\<lbrace>\<lambda>s. P (thread_states s)\<rbrace> as_user t f \<lbrace>\<lambda>rv s. P (thread_states s)\<rbrace>"
-  apply (simp add: thread_states_def)
-  apply wp
-  done
-
-lemma as_user_thread_bound_ntfn[wp]:
-  "\<lbrace>\<lambda>s. P (thread_bound_ntfns s)\<rbrace> as_user t f \<lbrace>\<lambda>rv s. P (thread_bound_ntfns s)\<rbrace>"
-  apply (simp add: as_user_def set_object_def split_def thread_bound_ntfns_def)
-  apply (wp get_object_wp)
-  apply (clarsimp simp: thread_states_def get_tcb_def
-                 elim!: rsubst[where P=P, OF _ ext] split: option.split)
-  done
-
-lemma tcb_domain_map_wellformed_lift:
-  assumes 1: "\<And>P. \<lbrace>\<lambda>s. P (ekheap s)\<rbrace> f \<lbrace>\<lambda>rv s. P (ekheap s)\<rbrace>"
-  shows "\<lbrace>tcb_domain_map_wellformed aag\<rbrace> f \<lbrace>\<lambda>rv. tcb_domain_map_wellformed aag\<rbrace>"
-  by (rule 1)
-
-lemma as_user_pas_refined[wp]:
-  "\<lbrace>pas_refined aag\<rbrace> as_user t f \<lbrace>\<lambda>rv. pas_refined aag\<rbrace>"
-apply (simp add: pas_refined_def state_objs_to_policy_def)
-apply (rule hoare_pre)
- apply wps
- apply wp
-apply simp
-done
-
-(* **************************************** *)
-
-subsection\<open>Random lemmas that belong elsewhere.\<close>
-
-(* FIXME: move *)
-lemma bang_0_in_set:
-  "xs \<noteq> [] \<Longrightarrow> xs ! 0 \<in> set xs"
-  apply(fastforce simp: in_set_conv_nth)
-  done
-
-(* FIXME: move *)
-lemma update_one_strg:
-  "((b \<longrightarrow> P c v) \<and> (\<not> b \<longrightarrow> (\<forall>v'. f c' = Some v' \<longrightarrow> P c v')))
-  \<longrightarrow>
-  ((f(c := if b then Some v else f c')) x = Some y \<and> f x \<noteq> Some y \<longrightarrow> P x y)"
-  by auto
-
-(* FIXME: move *)
-lemma hoare_gen_asm2:
-  assumes a: "P \<Longrightarrow> \<lbrace>\<top>\<rbrace> f \<lbrace>Q\<rbrace>"
-  shows "\<lbrace>K P\<rbrace> f \<lbrace>Q\<rbrace>"
-  using a by (fastforce simp: valid_def)
-
-(* FIXME: move *)
-lemma hoare_vcg_all_liftE:
-  "(\<And>x. \<lbrace>P x\<rbrace> f \<lbrace>Q x\<rbrace>, \<lbrace>Q' x\<rbrace>) \<Longrightarrow> \<lbrace>\<lambda>s. \<forall>x. P x s\<rbrace> f \<lbrace>\<lambda>rv s. \<forall>x. Q x rv s\<rbrace>, \<lbrace>\<lambda>rv s. \<forall>x. Q' x rv s\<rbrace>"
-  unfolding validE_def
-  apply (rule hoare_post_imp [where Q = "\<lambda>v s. \<forall>x. case v of Inl e \<Rightarrow> Q' x e s | Inr r \<Rightarrow> Q x r s"])
-   apply (clarsimp split: sum.splits)
-  apply (erule hoare_vcg_all_lift)
-  done
-
-(* FIXME: eliminate *)
-lemma hoare_weak_lift_impE:
-  "\<lbrace>P\<rbrace> f \<lbrace>Q\<rbrace>, \<lbrace>Q'\<rbrace> \<Longrightarrow> \<lbrace>\<lambda>s. R \<longrightarrow> P s\<rbrace> f \<lbrace>\<lambda>rv s. R \<longrightarrow> Q rv s\<rbrace>, \<lbrace>\<lambda>rv s. R \<longrightarrow> Q' rv s\<rbrace>"
-  by (rule wp_throw_const_impE)
-
-(* FIXME: move *)
-lemma hoare_use_ex_R:
-  "(\<And>x. \<lbrace>P x and Q \<rbrace> f \<lbrace>R\<rbrace>, -) \<Longrightarrow> \<lbrace>\<lambda>s. (\<exists>x. P x s) \<and> Q s \<rbrace> f \<lbrace>R\<rbrace>, -"
-  unfolding validE_R_def validE_def valid_def by fastforce
-
-(* FIXME: move *)
-lemma mapM_x_and_const_wp:
-  assumes f: "\<And>v. \<lbrace>P and K (Q v)\<rbrace> f v \<lbrace>\<lambda>rv. P\<rbrace>"
-  shows "\<lbrace>P and K (\<forall>v \<in> set vs. Q v)\<rbrace> mapM_x f vs \<lbrace>\<lambda>rv. P\<rbrace>"
-  apply (induct vs)
-   apply (simp add: mapM_x_Nil)
-  apply (simp add: mapM_x_Cons)
-  apply (wp f | assumption | simp)+
-  done
-
-(* stronger *)
-(* FIXME: MOVE *)
-lemma ep_queued_st_tcb_at':
-  "\<And>P. \<lbrakk>ko_at (Endpoint ep) ptr s; (t, rt) \<in> ep_q_refs_of ep;
-         valid_objs s; sym_refs (state_refs_of s);
-         \<And>pl pl'. P (Structures_A.BlockedOnSend ptr pl) \<and> P (Structures_A.BlockedOnReceive ptr pl') \<rbrakk>
-    \<Longrightarrow> st_tcb_at P t s"
-  apply (case_tac ep, simp_all)
-  apply (frule(1) sym_refs_ko_atD, clarsimp, erule (1) my_BallE,
-         clarsimp simp: st_tcb_at_def refs_of_rev elim!: obj_at_weakenE)+
-  done
-
-(* Sometimes we only care about one of the queues. *)
-(* FIXME: move *)
-lemma ep_rcv_queued_st_tcb_at:
-  "\<And>P. \<lbrakk>ko_at (Endpoint ep) epptr s; (t, EPRecv) \<in> ep_q_refs_of ep;
-         valid_objs s; sym_refs (state_refs_of s);
-         \<And>pl. P (Structures_A.BlockedOnReceive epptr pl);
-         kheap s' t = kheap s t\<rbrakk>
-    \<Longrightarrow> st_tcb_at P t s'"
-  apply (case_tac ep, simp_all)
-  apply (subgoal_tac "st_tcb_at P t s")
-   apply (simp add: st_tcb_at_def obj_at_def)
-  apply (frule(1) sym_refs_ko_atD, clarsimp, erule (1) my_BallE,
-         clarsimp simp: st_tcb_at_def refs_of_rev elim!: obj_at_weakenE)+
-  done
-
-(* FIXME: move. *)
-lemma ntfn_queued_st_tcb_at':
-  "\<And>P. \<lbrakk>ko_at (Notification ntfn) ntfnptr s; (t, rt) \<in> ntfn_q_refs_of (ntfn_obj ntfn);
-         valid_objs s; sym_refs (state_refs_of s);
-         P (Structures_A.BlockedOnNotification ntfnptr) \<rbrakk>
-   \<Longrightarrow> st_tcb_at P t s"
-  apply (case_tac "ntfn_obj ntfn", simp_all)
-  apply (frule(1) sym_refs_ko_atD)
-  apply (clarsimp)
-  apply (erule_tac y="(t, NTFNSignal)" in my_BallE, clarsimp)
-  apply (clarsimp simp: pred_tcb_at_def refs_of_rev elim!: obj_at_weakenE)+
-  done
-
-(* FIXME: move *)
-lemma case_prod_wp:
-  "(\<And>a b. x = (a, b) \<Longrightarrow> \<lbrace>P a b\<rbrace> f a b \<lbrace>Q\<rbrace>)
-  \<Longrightarrow> \<lbrace>P (fst x) (snd x)\<rbrace> case_prod f x \<lbrace>Q\<rbrace>"
- by (cases x, simp)
-
-(* FIXME: move *)
-lemma case_sum_wp:
-  "\<lbrakk> (\<And>a. x = Inl a \<Longrightarrow> \<lbrace>P a\<rbrace> f a \<lbrace>Q\<rbrace>);
-     (\<And>a. x = Inr a \<Longrightarrow> \<lbrace>P' a\<rbrace> g a \<lbrace>Q\<rbrace>) \<rbrakk>
-  \<Longrightarrow> \<lbrace>\<lambda>s. (\<forall>a. x = Inl a \<longrightarrow> P a s) \<and> (\<forall>a. x = Inr a \<longrightarrow> P' a s)\<rbrace> case_sum f g x \<lbrace>Q\<rbrace>"
-  by (cases x, simp_all)
-
-(* MOVE *)
-crunch arm_asid_table_inv [wp]: store_pte "\<lambda>s. P (arm_asid_table (arch_state s))"
-
-lemma st_tcb_at_to_thread_states:
-  "st_tcb_at P t s \<Longrightarrow> \<exists>st. P st \<and> thread_states s t = tcb_st_to_auth st"
-  by (fastforce simp: st_tcb_def2 thread_states_def tcb_states_of_state_def)
-
-lemma aag_Control_into_owns:
-  "\<lbrakk> aag_has_auth_to aag Control p; pas_refined aag s \<rbrakk> \<Longrightarrow> is_subject aag p"
-  apply (drule (1) pas_refined_Control)
-  apply simp
-  done
-
-lemma aag_has_Control_iff_owns:
-  "pas_refined aag s \<Longrightarrow> (aag_has_auth_to aag Control x) = (is_subject aag x)"
-  apply (rule iffI)
-  apply (erule (1) aag_Control_into_owns)
-  apply (simp add: pas_refined_refl)
-  done
-
-lemma aag_Control_owns_strg:
-  "pas_wellformed aag \<and> is_subject aag v \<longrightarrow> aag_has_auth_to aag Control v"
-  by (clarsimp simp: aag_wellformed_refl)
-
-(* **************************************** *)
-
-subsection \<open>Policy entailments\<close>
-
-lemma owns_ep_owns_receivers:
-  "\<lbrakk>\<forall>auth. aag_has_auth_to aag auth epptr; pas_refined aag s; invs s;
-    ko_at (Endpoint ep) epptr s; (t, EPRecv) \<in> ep_q_refs_of ep\<rbrakk>
-  \<Longrightarrow> is_subject aag t"
-  apply (drule (1) ep_rcv_queued_st_tcb_at [where P = "receive_blocked_on epptr"])
-      apply clarsimp
-     apply clarsimp
-    apply clarsimp
-   apply (rule refl)
-  apply (drule st_tcb_at_to_thread_states)
-  apply (clarsimp simp: receive_blocked_on_def2)
-  apply (drule spec [where x = Grant])
-  apply (frule aag_wellformed_grant_Control_to_recv
-           [OF _ _ pas_refined_wellformed])
-    apply (rule pas_refined_mem [OF sta_ts])
-     apply fastforce
-    apply assumption+
-  apply (erule (1) aag_Control_into_owns)
-  done
-
-(* MOVE *)
-lemma cli_caps_of_state:
-  "\<lbrakk> caps_of_state s slot = Some cap; pas_refined aag s \<rbrakk> \<Longrightarrow> cap_links_irq aag (pasObjectAbs aag (fst slot)) cap"
-apply (clarsimp simp add: cap_links_irq_def pas_refined_def)
-apply (blast dest: state_irqs_to_policy_aux.intros)
-done
-
-(* MOVE *)
-lemma cap_auth_caps_of_state:
-  "\<lbrakk> caps_of_state s p = Some cap; pas_refined aag s \<rbrakk>
-  \<Longrightarrow> aag_cap_auth aag (pasObjectAbs aag (fst p)) cap"
-  unfolding aag_cap_auth_def
-  apply (intro conjI)
-    apply clarsimp
-    apply (drule (2) sta_caps)
-    apply (drule_tac f="pasObjectAbs aag" in auth_graph_map_memI[OF _ refl refl])
-    apply (fastforce simp: pas_refined_def)
-   apply clarsimp
-   apply (drule (2) sta_untyped [THEN pas_refined_mem] )
-   apply simp
-  apply (drule (1) clas_caps_of_state)
-  apply simp
-  apply (drule (1) cli_caps_of_state)
-  apply simp
-  done
-
-lemma cap_cur_auth_caps_of_state:
-  "\<lbrakk> caps_of_state s p = Some cap; pas_refined aag s; is_subject aag (fst p) \<rbrakk>
-  \<Longrightarrow> pas_cap_cur_auth aag cap"
-  by (metis cap_auth_caps_of_state)
-
-subsection \<open>Integrity monotony over subjects\<close>
-
-lemmas new_range_subset' = aligned_range_offset_subset
-lemmas ptr_range_subset = new_range_subset' [folded ptr_range_def]
-
-lemma pbfs_less_wb:
-  "pageBitsForSize x < word_bits"
-  by (cases x, simp_all add: word_bits_def)
-
-lemma ipcframe_subset_page:
-  "\<lbrakk>valid_objs s; get_tcb p s = Some tcb;
-    tcb_ipcframe tcb = cap.ArchObjectCap (arch_cap.PageCap d p' R vms xx);
-    x \<in> ptr_range (p' + (tcb_ipc_buffer tcb && mask (pageBitsForSize vms))) msg_align_bits \<rbrakk>
-  \<Longrightarrow> x \<in> ptr_range p' (pageBitsForSize vms)"
-   apply (frule (1) valid_tcb_objs)
-   apply (clarsimp simp add: valid_tcb_def ran_tcb_cap_cases)
-   apply (erule set_mp[rotated])
-   apply (rule ptr_range_subset)
-     apply (simp add: valid_cap_def cap_aligned_def)
-    apply (simp add: valid_tcb_def valid_ipc_buffer_cap_def is_aligned_andI1 split:bool.splits)
-   apply (rule order_trans [OF _ pbfs_atleast_pageBits])
-   apply (simp add: msg_align_bits pageBits_def)
-  apply (rule and_mask_less')
-  apply (simp add: pbfs_less_wb [unfolded word_bits_conv])
-  done
-
-lemma trm_ipc':
-  "\<lbrakk> pas_refined aag s; valid_objs s; case_option False can_receive_ipc (tcb_states_of_state s p');
-     (tcb_states_of_state s' p') = Some Structures_A.Running;
-     p \<in> auth_ipc_buffers s p' \<rbrakk> \<Longrightarrow>
-    integrity_mem aag subjects p
-          (tcb_states_of_state s) (tcb_states_of_state s') (auth_ipc_buffers s) X
-          (underlying_memory (machine_state s) p)
-          (underlying_memory (machine_state s') p)"
-  apply (cases "pasObjectAbs aag p' \<in> subjects")
-   apply (rule trm_write)
-   apply (clarsimp simp: auth_ipc_buffers_member_def)
-   apply (frule pas_refined_mem[rotated])
-    apply (erule sta_caps, simp)
-     apply (erule(3) ipcframe_subset_page)
-    apply (simp add: cap_auth_conferred_def vspace_cap_rights_to_auth_def
-                     is_page_cap_def)
-    apply fastforce
-   apply fastforce
-  by (rule trm_ipc)
-
-
-lemma tcb_bound_notification_reset_integrity_mono:
-  "\<lbrakk> tcb_bound_notification_reset_integrity ntfn ntfn' S aag ; S \<subseteq> T\<rbrakk>
-   \<Longrightarrow> tcb_bound_notification_reset_integrity ntfn ntfn' T aag"
-  unfolding tcb_bound_notification_reset_integrity_def by blast
-
-lemma reply_cap_deletion_integrity_mono:
-  "\<lbrakk> reply_cap_deletion_integrity S aag cap cap' ; S \<subseteq> T\<rbrakk> \<Longrightarrow> reply_cap_deletion_integrity T aag cap cap'"
-  by (blast intro: reply_cap_deletion_integrity_intros elim: reply_cap_deletion_integrityE)
-
-lemma cnode_integrity_mono:
-  "\<lbrakk> cnode_integrity S aag cont cont' ; S \<subseteq> T\<rbrakk> \<Longrightarrow> cnode_integrity T aag cont cont'"
-  by (blast intro!: cnode_integrityI elim: cnode_integrityE dest:reply_cap_deletion_integrity_mono)
-
-lemma asid_pool_integrity_mono:
-  "\<lbrakk> asid_pool_integrity S aag cont cont' ; S \<subseteq> T\<rbrakk> \<Longrightarrow> asid_pool_integrity T aag cont cont'"
-  unfolding asid_pool_integrity_def by fastforce
-
-lemma cdt_change_allowed_mono:
-  "\<lbrakk>cdt_change_allowed aag S (cdt s) (tcb_states_of_state s) ptr; S \<subseteq> T \<rbrakk> \<Longrightarrow>
-    cdt_change_allowed aag T (cdt s) (tcb_states_of_state s) ptr"
-  unfolding cdt_change_allowed_def cdt_direct_change_allowed.simps direct_call_def by blast
-
-
-
-lemmas rtranclp_monoE = rtranclp_mono[THEN predicate2D,rotated,OF _ predicate2I]
-
-lemma integrity_mono:
-  "\<lbrakk> integrity_subjects S aag activate X s s'; S \<subseteq> T;
-           pas_refined aag s; valid_objs s \<rbrakk>
-     \<Longrightarrow> integrity_subjects T aag activate X s s'"
-  apply (clarsimp simp: integrity_subjects_def simp del:split_paired_All)
-  apply (rule conjI)
-   apply clarsimp
-   apply (drule_tac x=x in spec)+
-   apply (simp only: integrity_obj_def)
-   apply (erule rtranclp_monoE)
-   apply (erule integrity_obj_atomic.cases[OF _ integrity_obj_atomic.intros];
-          auto simp: indirect_send_def direct_send_def direct_call_def direct_reply_def
-               elim: asid_pool_integrity_mono reply_cap_deletion_integrity_mono
-                     cnode_integrity_mono)
-  apply (rule conjI)
-   apply clarsimp
-   apply (drule_tac x=x in spec)+
-   apply (erule integrity_eobj.cases; auto intro: integrity_eobj.intros)
-  apply (rule conjI)
-   apply clarsimp
-   apply (drule_tac x=x in spec, erule integrity_mem.cases;
-          blast intro: integrity_mem.intros trm_ipc')
-  apply (rule conjI)
-   apply clarsimp
-   apply (drule_tac x=x in spec, erule integrity_device.cases;
-          blast intro: integrity_device.intros)
-  apply (rule conjI)
-  apply (intro allI)
-  apply (drule_tac x=x in spec)+
-   apply (erule integrity_cdtE; auto elim: cdt_change_allowed_mono)
-  apply (rule conjI)
-   apply (intro allI)
-   apply (drule_tac x=x in spec)+
-   apply (erule integrity_cdt_listE;
-          auto elim!: weaken_filter_eq' intro: integrity_cdt_list_intros
-               elim: cdt_change_allowed_mono)
-  apply (rule conjI)
-   apply (fastforce simp: integrity_interrupts_def)
-  apply (rule conjI)
-   apply (fastforce simp: integrity_asids_def)
-  apply (clarsimp simp: integrity_ready_queues_def)
-  apply blast
-  done
-
-subsection\<open>Access control do not care about machine_state\<close>
-
-lemma integrity_irq_state_independent[intro!, simp]:
-  "integrity x y z (s\<lparr>machine_state :=
-                              machine_state s\<lparr>irq_state := f (irq_state (machine_state s))\<rparr>\<rparr>)
-   = integrity x y z s"
-  by (simp add: integrity_def)
-
-lemma state_objs_to_policy_irq_state_independent[intro!, simp]:
-  "state_objs_to_policy (s\<lparr>machine_state :=
-                                   machine_state s\<lparr>irq_state := f (irq_state (machine_state s))\<rparr>\<rparr>)
-   = state_objs_to_policy s"
-  by (simp add: state_objs_to_policy_def)
-
-lemma tcb_domain_map_wellformed_independent[intro!, simp]:
-  "tcb_domain_map_wellformed aag (s\<lparr>machine_state :=
-                                  machine_state s\<lparr>irq_state := f (irq_state (machine_state s)) \<rparr> \<rparr>)
-   = tcb_domain_map_wellformed aag s"
-  by (simp add: tcb_domain_map_wellformed_aux_def get_etcb_def)
-
-lemma pas_refined_irq_state_independent[intro!, simp]:
-  "pas_refined x (s\<lparr>machine_state := machine_state s\<lparr>irq_state := f (irq_state (machine_state s))\<rparr>\<rparr>)
-   = pas_refined x s"
-  by (simp add: pas_refined_def)
-
-
-subsection\<open>Transitivity of integrity lemmas and tactics\<close>
-
-lemma integrity_trans_start:
-  "(\<And> s. P s \<Longrightarrow> \<lbrace>(=) s\<rbrace> f \<lbrace>\<lambda>_. integrity aag X s\<rbrace>)
-    \<Longrightarrow> \<lbrace>integrity aag X st and P\<rbrace> f \<lbrace>\<lambda>_. integrity aag X st\<rbrace>"
-  unfolding spec_valid_def valid_def using integrity_trans
-  by simp blast
-
-method integrity_trans_start
-    = ((simp only: and_assoc[symmetric])?, rule integrity_trans_start[rotated])
-
-(* Q should be explicitly supplied, if not, use wp_integrity_clean' *)
-lemma wp_integrity_clean:
-  "\<lbrakk>\<And>s. Q s \<Longrightarrow> integrity aag X s (g s);
-    \<lbrace> P \<rbrace> f \<lbrace>\<lambda>_. integrity aag X st and Q\<rbrace> \<rbrakk> \<Longrightarrow> \<lbrace> P \<rbrace> f \<lbrace>\<lambda>_ s. integrity aag X st (g s) \<rbrace> "
-   by (rule hoare_post_imp[of "\<lambda>_. integrity aag X st and Q"])
-      (fastforce elim: integrity_trans)
-
-lemmas wp_integrity_clean'= wp_integrity_clean[of \<top>, simplified]
-
-
-end
 
 end
