proof/access-control/ARM/ArchAccess.thy
@@ -1,0 +1,287 @@
+(*
+ * Copyright 2020, Data61, CSIRO (ABN 41 687 119 230)
+ *
+ * SPDX-License-Identifier: GPL-2.0-only
+ *)
+
+theory ArchAccess
+imports Types
+begin
+
+context Arch begin global_naming ARM_A
+
+subsection \<open>Arch-specific transformation of caps into authorities\<close>
+
+definition vspace_cap_rights_to_auth :: "cap_rights \<Rightarrow> auth set" where
+  "vspace_cap_rights_to_auth r \<equiv>
+     (if AllowWrite \<in> r then {Write} else {})
+   \<union> (if AllowRead \<in> r then {Read} else {})"
+
+definition arch_cap_auth_conferred where
+  "arch_cap_auth_conferred arch_cap \<equiv>
+     (if is_page_cap arch_cap then vspace_cap_rights_to_auth (acap_rights arch_cap) else {Control})"
+
+subsection \<open>Generating a policy from the current ASID distribution\<close>
+
+definition pte_ref where
+  "pte_ref pte \<equiv> case pte of
+     SmallPagePTE addr atts rights
+       \<Rightarrow> Some (ptrFromPAddr addr, pageBitsForSize ARMSmallPage, vspace_cap_rights_to_auth rights)
+   | LargePagePTE addr atts rights
+       \<Rightarrow> Some (ptrFromPAddr addr, pageBitsForSize ARMLargePage, vspace_cap_rights_to_auth rights)
+   | _ \<Rightarrow> None"
+
+definition pde_ref2 where
+  "pde_ref2 pde \<equiv> case pde of
+     SectionPDE addr atts domain rights
+       \<Rightarrow> Some (ptrFromPAddr addr, pageBitsForSize ARMSection, vspace_cap_rights_to_auth rights)
+   | SuperSectionPDE addr atts rights
+       \<Rightarrow> Some (ptrFromPAddr addr, pageBitsForSize ARMSuperSection, vspace_cap_rights_to_auth rights)
+   | PageTablePDE addr atts domain
+       \<comment> \<open>The 0 is a hack, saying that we own only addr, although 12 would also be OK\<close>
+       \<Rightarrow> Some (ptrFromPAddr addr, 0, {Control})
+   | _ \<Rightarrow> None"
+
+\<comment> \<open>We exclude the global page tables from the authority graph. Alternatively, we could include them
+    and add a wellformedness constraint to policies that requires that every label has the necessary
+    authority to whichever label owns the global page tables, so that when a new page directory is
+    created and references to the global page tables are added to it, no new authority is gained.
+    Note: excluding the references to global page tables in this way brings in some ARM
+          arch-specific VM knowledge here\<close>
+definition vs_refs_no_global_pts :: "kernel_object \<Rightarrow> (obj_ref \<times> obj_ref \<times> aa_type \<times> auth) set"
+  where
+  "vs_refs_no_global_pts \<equiv> \<lambda>ko. case ko of
+     ArchObj (ASIDPool pool) \<Rightarrow> (\<lambda>(r,p). (p, ucast r, AASIDPool, Control)) ` graph_of pool
+   | ArchObj (PageDirectory pd) \<Rightarrow>
+       \<Union>(r,(p, sz, auth)) \<in> graph_of (pde_ref2 o pd) - {(x,y). (ucast (kernel_base >> 20) \<le> x)}.
+         (\<lambda>(p, a). (p, ucast r, APageDirectory, a)) ` (ptr_range p sz \<times> auth)
+   | ArchObj (PageTable pt) \<Rightarrow>
+       \<Union>(r,(p, sz, auth)) \<in> graph_of (pte_ref o pt).
+         (\<lambda>(p, a). (p, ucast r, APageTable, a)) ` (ptr_range p sz \<times> auth)
+   | _ \<Rightarrow> {}"
+
+definition state_vrefs where
+  "state_vrefs s = case_option {} vs_refs_no_global_pts o kheap s"
+
+end
+
+
+context pspace_update_eq begin interpretation Arch .
+
+lemma state_vrefs[iff]: "state_vrefs (f s) = state_vrefs s"
+  by (simp add: state_vrefs_def pspace)
+
+end
+
+
+context Arch begin
+
+primrec aobj_ref' where
+  "aobj_ref' (ASIDPoolCap p as) = {p}"
+| "aobj_ref' ASIDControlCap = {}"
+| "aobj_ref' (PageCap isdev x rs sz as4) = ptr_range x (pageBitsForSize sz)"
+| "aobj_ref' (PageDirectoryCap x as2) = {x}"
+| "aobj_ref' (PageTableCap x as3) = {x}"
+
+fun acap_asid' :: "arch_cap \<Rightarrow> asid set" where
+  "acap_asid' (PageCap _ _ _ _ mapping) = fst ` set_option mapping"
+| "acap_asid' (PageTableCap _ mapping) = fst ` set_option mapping"
+| "acap_asid' (PageDirectoryCap _ asid_opt) = set_option asid_opt"
+| "acap_asid' (ASIDPoolCap _ asid)
+     = {x. asid_high_bits_of x = asid_high_bits_of asid \<and> x \<noteq> 0}"
+| "acap_asid' ASIDControlCap = UNIV"
+
+inductive_set state_asids_to_policy_aux for aag caps asid_tab vrefs where
+  sata_asid:
+    "\<lbrakk> caps ptr = Some (ArchObjectCap acap); asid \<in> acap_asid' acap \<rbrakk>
+       \<Longrightarrow> (pasObjectAbs aag (fst ptr), Control, pasASIDAbs aag asid)
+             \<in> state_asids_to_policy_aux aag caps asid_tab vrefs"
+| sata_asid_lookup:
+    "\<lbrakk> asid_tab (asid_high_bits_of asid) = Some poolptr;
+       (pdptr, asid && mask asid_low_bits, AASIDPool, a) \<in> vrefs poolptr \<rbrakk>
+       \<Longrightarrow> (pasASIDAbs aag asid, a, pasObjectAbs aag pdptr)
+             \<in> state_asids_to_policy_aux aag caps asid_tab vrefs"
+| sata_asidpool:
+    "\<lbrakk> asid_tab (asid_high_bits_of asid) = Some poolptr; asid \<noteq> 0 \<rbrakk>
+       \<Longrightarrow> (pasObjectAbs aag poolptr, AAuth ASIDPoolMapsASID, pasASIDAbs aag asid)
+             \<in> state_asids_to_policy_aux aag caps asid_tab vrefs"
+
+definition
+  "state_asids_to_policy_arch aag caps astate vrefs \<equiv>
+     state_asids_to_policy_aux aag caps (arm_asid_table astate) vrefs"
+declare state_asids_to_policy_arch_def[simp]
+
+section \<open>Arch-specific integrity definition\<close>
+
+subsection \<open>How ASIDs can change\<close>
+
+abbreviation integrity_asids_aux ::
+  "'a PAS \<Rightarrow> 'a set \<Rightarrow> asid \<Rightarrow> obj_ref option \<Rightarrow> obj_ref option \<Rightarrow> bool" where
+  "integrity_asids_aux aag subjects asid pp_opt pp_opt' \<equiv>
+     pp_opt = pp_opt' \<or> (\<forall>asid'. asid' \<noteq> 0 \<and> asid_high_bits_of asid' = asid_high_bits_of asid
+                                 \<longrightarrow> pasASIDAbs aag asid' \<in> subjects)"
+
+definition integrity_asids ::
+  "'a PAS \<Rightarrow> 'a set \<Rightarrow> asid \<Rightarrow> 'y::state_ext state \<Rightarrow> 'z:: state_ext state  \<Rightarrow> bool" where
+  "integrity_asids aag subjects x s s' \<equiv>
+   integrity_asids_aux aag subjects x (asid_table s  (asid_high_bits_of x))
+                                      (asid_table s' (asid_high_bits_of x))"
+
+declare integrity_asids_def[simp]
+
+lemma integrity_asids_trans_state_l[simp]:
+  "integrity_asids aag subjects x (trans_state f st) s =
+   integrity_asids aag subjects x st s"
+  by simp
+
+lemma integrity_asids_trans_state_r[simp]:
+  "integrity_asids aag subjects x st (trans_state f s) =
+   integrity_asids aag subjects x st s"
+  by simp
+
+lemma integrity_asids_cur_thread_update_l[simp]:
+  "integrity_asids aag subjects x (cur_thread_update f st) s =
+   integrity_asids aag subjects x st s"
+  by simp
+
+lemma integrity_asids_cur_thread_update_r[simp]:
+  "integrity_asids aag subjects x st (cur_thread_update f s) =
+   integrity_asids aag subjects x st s"
+  by simp
+
+lemma integrity_asids_kheap_update_l[simp]:
+  "integrity_asids aag subjects x (kheap_update f st) s =
+   integrity_asids aag subjects x st s"
+  by simp
+
+lemma integrity_asids_kheap_update_r[simp]:
+  "integrity_asids aag subjects x st (kheap_update f s) =
+   integrity_asids aag subjects x st s"
+  by simp
+
+lemma integrity_asids_machine_state_update_l[simp]:
+  "integrity_asids aag subjects x (machine_state_update f st) s =
+   integrity_asids aag subjects x st s"
+  by simp
+
+lemma integrity_asids_machine_state_update_r[simp]:
+  "integrity_asids aag subjects x st (machine_state_update f s) =
+   integrity_asids aag subjects x st s"
+  by simp
+
+lemma integrity_asids_cdt_update_l[simp]:
+  "integrity_asids aag subjects x (cdt_update f st) s =
+   integrity_asids aag subjects x st s"
+  by simp
+
+lemma integrity_asids_cdt_update_r[simp]:
+  "integrity_asids aag subjects x st (cdt_update f s) =
+   integrity_asids aag subjects x st s"
+  by simp
+
+lemma integrity_asids_is_original_cap_update_l[simp]:
+  "integrity_asids aag subjects x (is_original_cap_update f st) s =
+   integrity_asids aag subjects x st s"
+  by simp
+
+lemma integrity_asids_is_original_cap_update_r[simp]:
+  "integrity_asids aag subjects x st (is_original_cap_update f s) =
+   integrity_asids aag subjects x st s"
+  by simp
+
+lemma integrity_asids_interrupt_states_update_l[simp]:
+  "integrity_asids aag subjects x (interrupt_states_update f st) s =
+   integrity_asids aag subjects x st s"
+  by simp
+
+lemma integrity_asids_interrupt_states_update_r[simp]:
+  "integrity_asids aag subjects x st (interrupt_states_update f s) =
+   integrity_asids aag subjects x st s"
+  by simp
+
+(* FIXME AC: locale? *)
+lemmas integrity_asids_updates =
+  integrity_asids_trans_state_l
+  integrity_asids_trans_state_r
+  integrity_asids_cur_thread_update_l
+  integrity_asids_cur_thread_update_r
+  integrity_asids_kheap_update_l
+  integrity_asids_kheap_update_r
+  integrity_asids_machine_state_update_l
+  integrity_asids_machine_state_update_r
+  integrity_asids_cdt_update_l
+  integrity_asids_cdt_update_r
+  integrity_asids_is_original_cap_update_l
+  integrity_asids_is_original_cap_update_r
+  integrity_asids_interrupt_states_update_l
+  integrity_asids_interrupt_states_update_r
+
+
+subsection \<open>Misc definitions\<close>
+
+definition ctxt_IP_update where
+  "ctxt_IP_update ctxt \<equiv> ctxt(NextIP := ctxt FaultIP)"
+
+abbreviation arch_IP_update where
+  "arch_IP_update arch \<equiv> arch_tcb_context_set (ctxt_IP_update (arch_tcb_context_get arch)) arch"
+
+definition asid_pool_integrity ::
+  "'a set \<Rightarrow> 'a PAS \<Rightarrow> (asid_low_index \<rightharpoonup> obj_ref) \<Rightarrow> (asid_low_index \<rightharpoonup> obj_ref) \<Rightarrow> bool" where
+  "asid_pool_integrity subjects aag pool pool' \<equiv>
+     \<forall>x. pool' x \<noteq> pool x
+         \<longrightarrow> pool' x = None \<and> aag_subjects_have_auth_to subjects aag Control (the (pool x))"
+
+inductive arch_integrity_obj_atomic ::
+   "'a PAS \<Rightarrow> 'a set \<Rightarrow> 'a \<Rightarrow> arch_kernel_obj \<Rightarrow> arch_kernel_obj \<Rightarrow> bool"
+  for aag subjects l ao ao' where
+  arch_troa_asidpool_clear:
+    "\<lbrakk> ao = ASIDPool pool; ao' = ASIDPool pool';
+       asid_pool_integrity subjects aag pool pool' \<rbrakk>
+       \<Longrightarrow> arch_integrity_obj_atomic aag subjects l ao ao'"
+
+inductive arch_integrity_obj_alt ::
+   "'a PAS \<Rightarrow> 'a set \<Rightarrow> 'a \<Rightarrow> arch_kernel_obj \<Rightarrow> arch_kernel_obj \<Rightarrow> bool"
+  for aag subjects l' ao ao' where
+  arch_tro_alt_asidpool_clear:
+    "\<lbrakk> ao = ASIDPool pool; ao' = ASIDPool pool';
+       asid_pool_integrity subjects aag pool pool'\<rbrakk>
+       \<Longrightarrow> arch_integrity_obj_alt aag subjects l' ao ao'"
+
+definition auth_ipc_buffers :: "'z::state_ext state \<Rightarrow> obj_ref \<Rightarrow> obj_ref set" where
+  "auth_ipc_buffers s \<equiv> \<lambda>p. case (get_tcb p s) of
+     None \<Rightarrow> {}
+   | Some tcb \<Rightarrow>
+     (case tcb_ipcframe tcb of
+        ArchObjectCap (PageCap False p' R vms _) \<Rightarrow>
+          if AllowWrite \<in> R
+          then (ptr_range (p' + (tcb_ipc_buffer tcb && mask (pageBitsForSize vms))) msg_align_bits)
+          else {}
+      | _ \<Rightarrow> {})"
+
+end
+
+
+context begin interpretation Arch .
+
+requalify_consts
+  vspace_cap_rights_to_auth
+  aobj_ref'
+  acap_asid'
+  state_vrefs
+  state_asids_to_policy_arch
+  integrity_asids
+  ctxt_IP_update
+  arch_IP_update
+  arch_cap_auth_conferred
+  arch_integrity_obj_atomic
+  arch_integrity_obj_alt
+  auth_ipc_buffers
+
+requalify_facts
+  integrity_asids_updates
+
+end
+
+declare integrity_asids_updates[simp]
+
+end
