proof/access-control/Types.thy
@@ -1,0 +1,162 @@
+(*
+ * Copyright 2020, Data61, CSIRO (ABN 41 687 119 230)
+ *
+ * SPDX-License-Identifier: GPL-2.0-only
+ *)
+
+theory Types
+imports ArchTypes
+begin
+
+subsection \<open>Policy definition\<close>
+
+text\<open>
+
+The goal is to place limits on what untrusted agents can do while the
+trusted agents are not running. This supports a framing constraint in
+the descriptions (Hoare triples) of syscalls. Roughly the existing
+proofs show the effect of the syscall, and this proof summarises what
+doesn't (or isn't allowed to) change.
+
+The basic intuition is to map all object references to the agent they
+belong to and show that changes to the object reference graph are
+allowed by the policy specified by the user. The policy is a labelled
+graph amongst agents independent of the current state, i.e. a static
+external summary of what should be talking to what and how.
+
+The interesting cases occur between trusted and untrusted components:
+e.g. we assume that it is unsafe for untrusted components (UT)
+to send capabilities to trusted components (T), and so T must ensure
+that all endpoints it shares with UT that it receives on do not have
+the grant bit set.
+
+\<close>
+
+type_synonym 'a agent_map = "obj_ref \<Rightarrow> 'a"
+type_synonym 'a agent_asid_map = "asid \<Rightarrow> 'a"
+type_synonym 'a agent_irq_map = "irq \<Rightarrow> 'a"
+type_synonym 'a agent_domain_map = "domain \<Rightarrow> 'a set"
+
+text\<open>
+
+What one agent can do to another. We allow multiple edges between
+agents in the graph.
+
+Control is special. It implies the ability to do pretty much anything,
+including get access the other rights, create, remove, etc.
+
+DeleteDerived allows you to delete a cap derived from a cap you own
+\<close>
+
+datatype auth = Control | Receive | SyncSend | Notify | Reset | Grant | Call
+                        | Reply | Write | Read | DeleteDerived | AAuth arch_auth
+
+text\<open>
+
+The interesting case is for endpoints.
+
+Consider an EP between T and UT (across a trust boundary). We want to
+be able to say that all EPs and tcbs that T does not expose to UT do
+not change when it is not running. If UT had a direct Send right to T
+then integrity (see below) could not guarantee this, as it doesn't
+know which EP can be changed by UT. Thus we set things up like this
+(all distinct labels):
+
+T -Receive-> EP <-Send- UT
+
+Now UT can interfere with EP and all of T's tcbs blocked for receive on EP,
+but not endpoints internal to T, or tcbs blocked on other (suitably
+labelled) EPs, etc.
+
+\<close>
+
+type_synonym 'a auth_graph = "('a \<times> auth \<times> 'a) set"
+
+text \<open>
+
+Each global namespace will need a labeling function.
+
+We map each scheduling domain to a single label; concretely, each tcb
+in a scheduling domain has to have the same label. We will want to
+weaken this in the future.
+
+The booleans @{text pasMayActivate} and @{text pasMayEditReadyQueues}
+are used to weaken the integrity property. When @{const True},
+@{text pasMayActivate} causes the integrity property to permit
+activation of newly-scheduled threads. Likewise, @{text pasMayEditReadyQueues}
+has the integrity property permit the removal of threads from ready queues,
+as occurs when scheduling a new domain for instance. By setting each of these
+@{const False} we get a more constrained integrity property that is useful for
+establishing some of the proof obligations for the infoflow proofs, particularly
+those over @{const handle_event} that neither activates new threads nor schedules
+new domains.
+
+The @{text pasDomainAbs} relation describes which labels may run in
+a given scheduler domain. This relation is not relevant to integrity
+but will be used in the information flow theory (with additional
+constraints on its structure).
+\<close>
+
+record 'a PAS =
+  pasObjectAbs :: "'a agent_map"
+  pasASIDAbs :: "'a agent_asid_map"
+  pasIRQAbs :: "'a agent_irq_map"
+  pasPolicy :: "'a auth_graph"
+  pasSubject :: "'a"                \<comment> \<open>The active label\<close>
+  pasMayActivate :: "bool"
+  pasMayEditReadyQueues :: "bool"
+  pasMaySendIrqs :: "bool"
+  pasDomainAbs :: "'a agent_domain_map"
+
+text\<open>
+
+Very often we want to say that the agent currently running owns a
+given pointer.
+
+\<close>
+
+abbreviation is_subject :: "'a PAS \<Rightarrow> obj_ref \<Rightarrow> bool" where
+  "is_subject aag ptr \<equiv> pasObjectAbs aag ptr = pasSubject aag"
+
+text\<open>
+
+Also we often want to say the current agent can do something to a
+pointer that he doesn't own but has some authority to.
+
+\<close>
+
+abbreviation(input) abs_has_auth_to :: "'a PAS \<Rightarrow> auth \<Rightarrow> obj_ref \<Rightarrow> obj_ref \<Rightarrow> bool" where
+  "abs_has_auth_to aag auth ptr ptr' \<equiv>
+     (pasObjectAbs aag ptr, auth, pasObjectAbs aag ptr') \<in> pasPolicy aag"
+
+abbreviation(input) aag_has_auth_to :: "'a PAS \<Rightarrow> auth \<Rightarrow> obj_ref \<Rightarrow> bool" where
+  "aag_has_auth_to aag auth ptr \<equiv> (pasSubject aag, auth, pasObjectAbs aag ptr) \<in> pasPolicy aag"
+
+abbreviation aag_subjects_have_auth_to_label :: "'a set \<Rightarrow> 'a PAS \<Rightarrow> auth \<Rightarrow> 'a \<Rightarrow> bool" where
+  "aag_subjects_have_auth_to_label subs aag auth label \<equiv>
+     \<exists>s \<in> subs. (s, auth, label) \<in> pasPolicy aag"
+
+abbreviation aag_subjects_have_auth_to :: "'a set \<Rightarrow> 'a PAS \<Rightarrow> auth \<Rightarrow> obj_ref \<Rightarrow> bool" where
+ "aag_subjects_have_auth_to subs aag auth oref \<equiv>
+    aag_subjects_have_auth_to_label subs aag auth (pasObjectAbs aag oref)"
+
+subsection \<open>Misc. definitions\<close>
+
+definition ptr_range where
+  "ptr_range p sz \<equiv> {p .. p + 2 ^ sz - 1}"
+
+lemma ptr_range_0[simp]: "ptr_range (p :: obj_ref) 0 = {p}"
+  unfolding ptr_range_def by simp
+
+definition tcb_states_of_state where
+  "tcb_states_of_state s \<equiv> \<lambda>p. option_map tcb_state (get_tcb p s)"
+
+fun can_receive_ipc :: "thread_state \<Rightarrow> bool" where
+  "can_receive_ipc (BlockedOnReceive _ _) = True"
+| "can_receive_ipc (BlockedOnSend _ pl)
+     = (sender_is_call pl \<and> (sender_can_grant pl \<or> sender_can_grant_reply pl))"
+| "can_receive_ipc (BlockedOnNotification _) = True"
+| "can_receive_ipc BlockedOnReply = True"
+| "can_receive_ipc _ = False"
+
+end
