spec/abstract/ARM/ArchVSpaceAcc_A.thy
@@ -30,6 +30,9 @@ definition
   asid_high_bits_of :: "asid \<Rightarrow> 7 word" where
   "asid_high_bits_of asid \<equiv> ucast (asid >> asid_low_bits)"
 
+locale_abbrev
+  "asid_table \<equiv> \<lambda>s. arm_asid_table (arch_state s)"
+
 
 section "Kernel Heap Accessors"
 
